Language.v
@@ -3,6 +3,7 @@
      - Expressions
      - Statements **)
 Add LoadPath "vst".
+Require Import CpdtTactics.
 Require Import Arith.
 Require Import List.
 Require Import Subst.
@@ -17,13 +18,36 @@ Inductive var   : Set := V : nat -> var.
 Inductive addr  : Set := A : nat -> addr.
 Inductive pname : Set := P : nat -> pname.
 
-Definition subst_loc (s:subst_t loc loc) (l:loc) := s l.
-Instance Subst_loc_loc : Subst loc loc loc := subst_loc.
+Definition subst_loc (s:subst_t loc loc) (l:loc) := 
+  match s l with 
+    | Some l' => l'
+    | _       => l
+  end.
+
+Instance Subst_loc_loc : Subst loc loc loc := 
+  mkSubst _ _ _ Logic.eq (fun l x => ~ l = x) subst_loc.
+Instance Subst_loc_vars : Subst loc var var := 
+  mkSubst _ _ _ Logic.eq (fun _ _ => True) (fun _ x => x).
+
+Instance FVSubst_loc_loc : SubstFV loc loc loc _ := _.
+Proof. 
+  firstorder. 
+  unfold subst; simpl; unfold subst_loc; simpl.
+  specialize (H e). 
+  destruct (s e).
+  destruct H. discriminate. reflexivity. reflexivity.
+Defined.
+Instance FVSubst_loc_vars : SubstFV loc var var Subst_loc_vars := _.
+Proof. firstorder. Defined.
+
+Instance Eq_eqLoc_loc : Equivalence (@eq loc loc loc Subst_loc_loc) := _.
+Instance Eq_eqLoc_var : Equivalence (@eq loc var var Subst_loc_vars) := _.
+
 Instance EqDec_loc : EqDec loc := _. 
-Proof. hnf. decide equality. apply eq_dec. Qed.
+Proof. hnf; decide equality; apply eq_dec. Defined.
 
 Definition subst_loc_one (l : loc) (l' : loc) : subst_t loc loc  :=
-  fun i => if eq_dec i l then l' else i.
+  fun i => if eq_dec i l then (Some l') else None.
 
 Definition null   := A 0.
 
@@ -53,8 +77,8 @@ Fixpoint fl_expr e :=
     | _ => []
   end.
 
-Definition FV e x := In x (fv_expr e).
-Definition FL e l := In l (fl_expr e).
+Definition NFV e x := ~ In x (fv_expr e).
+Definition NFL e l := ~ In l (fl_expr e).
   
 (* 
 Procedure p(x0 ... xn)
@@ -124,47 +148,146 @@ Proof.
 Qed.
 
 (*** Substitutions ***)
-Definition subst_var (s:subst_t var var) (v:var) := s v.
-Instance Subst_var_var : Subst var var var := subst_var.
+Definition subst_var (s:subst_t var var) (v:var) := 
+  match s v with
+    | Some v' => v'
+    | _       => v
+  end.
+
+Instance Subst_var_var : Subst var var var := 
+  mkSubst _ _ _ Logic.eq (fun v x => v <> x) subst_var.
+Instance FVSubst_var_var : SubstFV var var var _.
+Proof. 
+  constructor.
+  intros. unfold subst; simpl; unfold subst_var; simpl. 
+  specialize (H e).
+  destruct (s e). 
+  destruct H. discriminate. reflexivity. reflexivity.
+Defined.
+Instance Eq_Var_var : Equivalence (@eq var var var Subst_var_var) := _.
 
 Definition subst_var_one (v : var) (v' : var) : subst_t var var  :=
-  fun i => if eq_dec i v then v' else i.
+  fun i => if eq_dec i v then Some v' else None.
 
 Fixpoint subst_expr_var (s:subst_t var var) (e:expr) := 
   match e with 
-    | var_e v => var_e (s v)
+    | var_e v => var_e (subst s v)
     | fun_e p e1 e2 => fun_e p (subst_expr_var s e1) (subst_expr_var s e2)
     | _ => e
   end.
-Instance Subst_var_var_expr : Subst expr var var := fun s v => subst_expr_var s v.
+
+Hint Unfold subst_expr_var NFV fv_expr NFL fl_expr In : subst.
+
+Lemma nonfv_fun :
+  forall f x e1 e2,
+    NFV (fun_e f e1 e2) x -> NFV e1 x /\ NFV e2 x.
+Proof.
+  intros.
+  unfold NFV in *.
+  simpl in H.
+  constructor; intro; apply H; apply in_or_app.
+  left. assumption. right. assumption.
+Qed.
+
+Lemma nonfl_fun :
+  forall f x e1 e2,
+    NFL (fun_e f e1 e2) x -> NFL e1 x /\ NFL e2 x.
+Proof.
+  intros.
+  unfold NFV in *.
+  simpl in H.
+  constructor; intro; apply H; apply in_or_app.
+  left. assumption. right. assumption.
+Qed.
+
+Instance Subst_var_var_expr : Subst expr var var := 
+  mkSubst _ _ _ Logic.eq NFV subst_expr_var.
+Instance FVSubst_var_var_expr : SubstFV expr var var _ := _.
+Proof.
+  constructor.
+  intros.
+  unfold subst. simpl.
+  induction e; try reflexivity.
+  + repeat autounfold with subst in *.
+    rewrite subst_nonfv. reflexivity.
+    repeat intro. specialize (H x). apply H. assumption. rewrite H1.
+    simpl. left. reflexivity.
+  + simpl in *. 
+    pose (nonfv_fun).
+    rewrite IHe1. rewrite IHe2. reflexivity.
+    repeat intro. apply (a p x e1 e2). apply (H x). assumption. assumption.
+    repeat intro. specialize (a p x e1 e2).
+    destruct a. intro. apply (H x). assumption. assumption.
+    apply H2. assumption.
+Defined.
+Instance Eq_Var_expr : Equivalence (@eq expr var var Subst_var_var_expr) := _.
 
 Fixpoint subst_expr (s:subst_t var expr) (e:expr) := 
   match e with 
-    | var_e v => s v
+    | var_e v => match s v with | Some e' => e' | _ => var_e v end
     | fun_e p e1 e2 => fun_e p (subst_expr s e1) (subst_expr s e2)
     | _ => e
   end.
-Instance Subst_var_expr : Subst expr var expr := fun s v => subst_expr s v.
 
-Fixpoint subst_stmt (s:subst_t var var) (st:stmt) :=
-  match st with
-    | proc_s p xs r os ls => proc_s p (subst s xs) (subst s r) (subst s os) ls
-    | assign_s x e => assign_s (subst s x) (subst s e)
-    | _ => st
+Instance Subst_var_expr : Subst expr var expr := 
+  mkSubst _ _ _ Logic.eq NFV subst_expr.
+Instance FVSubst_var_expr : SubstFV expr var expr  _:= _.
+Proof.
+  constructor.
+  intros.
+  induction e; try reflexivity.
+  + specialize (H v). unfold NFV, fv_expr, In in H. intuition. unfold subst; simpl; unfold subst_expr; simpl.
+    destruct (s v).
+    destruct H. intro. inversion H. left. reflexivity. reflexivity.
+  + simpl in *. 
+    rewrite IHe1. rewrite IHe2. reflexivity.
+    repeat intro. apply (nonfv_fun p x e1 e2). apply (H x). assumption. assumption.
+    repeat intro. destruct (nonfv_fun p x e1 e2).
+    intro. apply (H x). assumption. assumption.
+    apply H2. assumption.
+Defined.
+Instance Eq_expr_var_expr : Equivalence (@eq expr var expr Subst_var_expr) := _.
+
+Instance Subst_loc_expr : Subst loc var expr := 
+  mkSubst _ _ _ Logic.eq (fun _ _ => True) (fun _ x => x).
+Instance FVSubst_loc_expr : SubstFV loc var expr _ := _.
+Proof. firstorder. Defined.
+Instance Eq_loc_expr : Equivalence (@eq loc var expr Subst_loc_expr) := _.
+
+Definition subst_var_loc (s : subst_t loc loc) (x : var) : var := x.
+Fixpoint subst_expr_loc (s : subst_t loc loc) (x : expr) : expr := 
+  match x with
+    | locvar_e l => locvar_e (subst s l)
+    | fun_e p e1 e2 => fun_e p (subst_expr_loc s e1) (subst_expr_loc s e2)
+    | _ => x
   end.
+Instance Subst_loc_var : Subst var loc loc := 
+  mkSubst _ _ _ Logic.eq (fun _ _ => True) subst_var_loc.
+Instance FVSubst_loc_var : SubstFV var loc loc _ := _.
+Proof. firstorder. Defined.
+Instance Eq_var_loc_var : Equivalence (@eq var loc loc Subst_loc_var) := _.
 
-Fixpoint subst_stmt_loc (s: subst_t loc loc) (st: stmt) :=
-  match st with 
-    | alloc_s l x e => alloc_s (subst s l) x e
-    | proc_s p xs r os ls => proc_s p xs r os (subst s ls)
-    | _ => st
-  end.
+Instance Subst_expr_loc : Subst expr loc loc := 
+  mkSubst _ _ _ Logic.eq NFL subst_expr_loc.
+Instance FVSubst_expr_loc : SubstFV expr loc loc _ := _.
+Proof.
+  constructor.
+  intros.
+  induction e; try reflexivity.
+  + specialize (H l); unfold NFL, fl_expr, In in *; intuition. 
+    simpl. unfold subst_loc. destruct (s l). 
+    destruct H. intro. inversion H. left. reflexivity. reflexivity.
+  + simpl in *.
+    rewrite IHe1. rewrite IHe2. reflexivity.
+    repeat intro. apply (nonfl_fun p x e1 e2). apply (H x). assumption. assumption.
+    repeat intro. destruct (nonfl_fun p x e1 e2).
+    intro. apply (H x). assumption. assumption.
+    apply H2. assumption.
+Defined.
+Instance Eq_expr_loc_loc : Equivalence (@eq expr loc loc Subst_expr_loc) := _.
 
-Instance Subst_stmt : Subst stmt var var := subst_stmt.
-Instance Subst_stmt_loc : Subst stmt loc loc := subst_stmt_loc.
-
-Definition state := var -> value.
-Definition locmap := loc -> addr.
+Definition state := var -> option value.
+Definition locmap := loc -> option addr.
 Definition heap  := addr -> option value.
 Definition world := ((state * locmap) * heap)%type.
 Definition stk (w : world) : state := fst (fst w).
@@ -175,17 +298,359 @@ Parameter eval_fun : pname -> expr -> expr -> value.
 
 Fixpoint eval s e :=
   match e with
-    | value_e v => v
+    | value_e v => Some v
     | var_e v   => stk s v
-    | locvar_e l => addr_v (runloc s l)
+    | locvar_e l =>  match runloc s l with 
+                       |Some a => Some (addr_v a)
+                       | _     => None
+                     end
     | fun_e f e1 e2 => 
-      let v1 := eval s e1 in
-      let v2 := eval s e2 in
-      eval_fun f v1 v2
+      match (eval s e1, eval s e2) with
+        | (Some v1, Some v2) => Some (eval_fun f v1 v2)
+        | _ => None
+      end
   end.
 
-Definition subst_one (x : var) (e : expr) :=
-  fun i => if eq_dec i x then e else (var_e i).
+Instance Subst_world_var : Subst world var var :=
+  mkSubst _ _ _ Logic.eq (fun w i => stk w i = None) 
+          (fun s w => (fun i => 
+                         match (s i) with
+                           | Some i' => stk w i'
+                           | None => stk w i
+                         end, runloc w, hp w)).
+
+Instance Subst_world_expr : Subst world var expr :=
+  mkSubst _ _ _ Logic.eq (fun w i => stk w i = None) 
+          (fun s w => (fun i => 
+                         match (s i) with
+                           | Some e => eval w e
+                            | None => stk w i
+                         end, runloc w, hp w)).
+
+Instance Subst_world_loc : Subst world loc loc := 
+  mkSubst _ _ _ Logic.eq (fun w i => runloc w i = None)
+          (fun s w => (stk w,
+                       fun l => 
+                         match (s l) with 
+                           | Some l' => runloc w l'
+                           | None => runloc w l
+                         end, hp w)).
+
+(* Class SubstWorld (D R : Type) (S: Subst var D R) `(SW : Subst world D R) := { *)
+(*   subst_world_var : *)
+(*     forall (s : subst_t D R) v w, *)
+(*       stk (subst s w) v = stk w (subst s v) *)
+(* }. *)
+
+(* Instance SubstWorld_var : SubstWorld var var _ _. *)
+(* Proof.  *)
+(*   constructor. *)
+(*   intros. unfold subst. simpl. destruct w. destruct p. *)
+(*   unfold stk. simpl. unfold subst_var. destruct (s v); reflexivity. *)
+(* Qed. *)
+
+(* Instance SubstWorld_loc : SubstWorld loc loc _ _. *)
+(* Proof. constructor; firstorder. Qed. *)
+
+Class SubstExpr (D R : Type) {E : EqDec D} {Sl : Subst loc D R} 
+      `{S : SubstFV expr D R} {SW : Subst world D R} : Type := {
+    subst_fun : 
+      forall (s : subst_t D R) p e1 e2,
+        subst s (fun_e p e1 e2) = fun_e p (subst s e1) (subst s e2)
+   ;
+   subst_value : 
+      forall (s : subst_t D R) v,
+        subst s (value_e v) = value_e v
+   ;
+   subst_locvar :
+     forall (s : subst_t D R) l,
+       locvar_e (subst s l) = subst s (locvar_e l)
+   ;
+   nonfv_eval :
+     forall e (x : D) v w,
+       nonfv e x -> eval w e = eval (subst (subst_one x v) w) e
+   ;
+   nonfv_subst :
+     forall (e e' : expr) (x : D) v,
+       nonfv e x -> nonfv e' x -> nonfv (subst (subst_one v e') e) x
+}.
+
+Instance SubstExpr_var_var : SubstExpr var var. 
+Proof. 
+  firstorder. {
+  unfold nonfv in H. simpl in H. unfold NFV in H.
+  destruct w as [[s ?] ?].
+  induction e; simpl in *; unfold stk; simpl.
+  + reflexivity.
+  + unfold subst_one. destruct (eq_dec x v0). subst. destruct H. left. reflexivity. reflexivity.
+  + reflexivity.
+  + rewrite IHe1. rewrite IHe2. reflexivity. 
+    intro. apply H. apply in_or_app. right. assumption.
+    intro. apply H. apply in_or_app. left. assumption.
+}{ 
+  induction e; intros; simpl in *; unfold stk; simpl. easy.
+  unfold subst_one. destruct (eq_dec v v0). easy. 
+  unfold NFV in *. intro. apply H. easy. easy.
+  unfold NFV in *.
+  simpl.
+  intro.
+  apply in_app_or in H1.
+  simpl in H. 
+  apply H. apply in_or_app. intuition.
+}
+Defined.
+
+Instance SubstExpr_var_expr : SubstExpr var expr. 
+Proof. 
+  firstorder. {
+  unfold nonfv in H. simpl in H. unfold NFV in H.
+  destruct w as [[s ?] ?].
+  induction e; simpl in *; unfold stk; simpl.
+  + reflexivity.
+  + unfold subst_one. destruct (eq_dec x v0). subst. destruct H. left. reflexivity. reflexivity.
+  + reflexivity.
+  + rewrite IHe1. rewrite IHe2. reflexivity. 
+    intro. apply H. apply in_or_app. right. assumption.
+    intro. apply H. apply in_or_app. left. assumption.
+    }{
+    
+  induction e. intros; simpl in *; unfold stk; simpl. easy.
+  unfold subst_one. simpl. destruct (eq_dec v v0). easy. 
+  unfold NFV in *. intro. apply H. easy. easy.
+  simpl in *.
+  intro.
+  simpl in H1. apply in_app_or in H1. apply H. simpl. 
+  unfold NFV in H. simpl in H.
+  unfold NFV in *. simpl in *. intuition.
+}
+Defined.
+
+Instance SubstExpr_loc_loc : SubstExpr loc loc.
+Proof. 
+  firstorder. 
+  {
+  unfold nonfv in H. simpl in H. unfold NFL in H.
+  destruct w as [[s ?] ?].
+  induction e; simpl in *; unfold stk, runloc; simpl.
+  + reflexivity.
+  + reflexivity. 
+  + unfold subst_one. destruct (eq_dec x l0). subst. destruct H. left. reflexivity. reflexivity.
+  + rewrite IHe1. rewrite IHe2. reflexivity. 
+    intro. apply H. apply in_or_app. right. assumption.
+    intro. apply H. apply in_or_app. left. assumption.
+  }
+  {
+    induction e; try easy. 
+    unfold subst_one. simpl. destruct (eq_dec v v0). assumption.
+    unfold NFL. intro. intuition.
+    unfold nonfv in *. simpl in *.
+    unfold NFL in H. simpl in H. intro. simpl in *. intuition.
+    apply H. apply in_or_app. apply in_app_or in H1. unfold NFL in *. intuition.
+  }
+Defined.
+
+Fixpoint subst_stmt {D R : Type} 
+         {S1 : Subst var D R}
+         {S2 : Subst loc D R} 
+         {S3 : Subst expr D R}
+         {E1 : Equivalence (eq (A := var))}
+         {E1 : Equivalence (eq (A := loc))}
+         {E1 : Equivalence (eq (A := expr))}
+         (s:subst_t D R) (st:stmt) :=
+  match st with
+    | pad_s l x => pad_s (subst s l) (subst s x)
+    | alloc_s l v e => alloc_s (subst s l) (subst s v) (subst s e)
+    | assign_s x e => assign_s (subst s x) (subst s e)
+    | proc_s p xs r os ls => proc_s p (subst s xs) (subst s r) (subst s os) (subst s ls)
+    | return_s e => return_s (subst s e)
+    | seq_s s1 s2 => seq_s (subst_stmt s s1) (subst_stmt s s2)
+    | if_s e s1 s2 => if_s (subst s e) (subst_stmt s s1) (subst_stmt s s2)
+    | _ => st
+  end.
+
+Fixpoint nonfv_stmt 
+         {D R : Type} 
+         {S1 : Subst var D R}
+         {S2 : Subst loc D R} 
+         {S3 : Subst expr D R}
+         {E1 : Equivalence (@eq _ _ _ S1)}
+         {E2 : Equivalence (@eq _ _ _ S2)}
+         {E3 : Equivalence (@eq _ _ _ S3)}
+         s (x : D) :=
+  match s with
+    | skip_s => False
+    | pad_s l v => nonfv l x /\ nonfv v x
+    | alloc_s l v e => nonfv l x /\ nonfv v x /\ nonfv e x
+    | assign_s v e => nonfv v x /\ nonfv e x
+    | proc_s p vs v vs' ls => nonfv v x /\ nonfv vs x /\ nonfv vs' x /\ nonfv ls x
+    | seq_s s1 s2 => nonfv_stmt s1 x /\ nonfv_stmt s2 x
+    | if_s e s1 s2 => nonfv e x /\ nonfv_stmt s1 x /\ nonfv_stmt s2 x
+    | return_s e => nonfv e x
+  end.
+
+Fixpoint eq_stmt 
+         {D R : Type} 
+         {S1 : Subst var D R}
+         {S2 : Subst loc D R} 
+         {S3 : Subst expr D R}
+         {E1 : Equivalence (@eq _ _ _ S1)}
+         {E2 : Equivalence (@eq _ _ _ S2)}
+         {E3 : Equivalence (@eq _ _ _ S3)}
+         s1 s2 :=
+  match (s1, s2) with
+    | (skip_s, skip_s) => True
+    | (pad_s l1 x1, pad_s l2 x2) => eq l1 l2 /\ eq x1 x2
+    | (alloc_s l1 x1 e1, alloc_s l2 x2 e2) => eq l1 l2 /\ eq x1 x2 /\ eq e1 e2
+    | (assign_s x1 e1, assign_s x2 e2) => eq x1 x2 /\ eq e1 e2
+    | (proc_s p1 vs1 v1 vs'1 ls1,
+       proc_s p2 vs2 v2 vs'2 ls2) => p1 = p2 /\ eq vs1 vs2 /\ eq v1 v2 /\ eq vs'1 vs'2 /\ eq ls1 ls2
+    | (seq_s s1 t1, seq_s s2 t2) => eq_stmt s1 s2 /\ eq_stmt t1 t2
+    | (if_s e1 s1 t1, if_s e2 s2 t2) => eq e1 e2 /\ eq_stmt s1 s2 /\ eq_stmt t1 t2
+    | (return_s e1, return_s e2) => eq e1 e2
+    | _ => False
+  end.
+
+Instance Equiv_eqStmt 
+         {D R : Type} 
+         {S1 : Subst var D R}
+         {S2 : Subst loc D R} 
+         {S3 : Subst expr D R}
+         {E1 : Equivalence (@eq _ _ _ S1)}
+         {E2 : Equivalence (@eq _ _ _ S2)}
+         {E3 : Equivalence (@eq _ _ _ S3)}
+: Equivalence (@eq_stmt D R _ _ _ _ _ _).
+Proof.
+  constructor.
+  hnf. intros. induction x; try first [ reflexivity
+                                      | repeat constructor; reflexivity
+                                      ].
+  constructor; assumption.
+  repeat constructor; try reflexivity; try assumption.
+  simpl; reflexivity.
+
+  hnf. intro x. induction x; intros; (destruct y; try inversion H).
+  reflexivity.
+  simpl. rewrite H0. rewrite H1. constructor; reflexivity.
+  simpl. rewrite H0. destruct H1. rewrite H1. rewrite H2. repeat constructor; reflexivity.
+  simpl. simpl in H.
+  repeat constructor; first [ rewrite H0; reflexivity | rewrite H1; reflexivity].
+  repeat constructor; simpl in *; symmetry; apply H.
+  constructor. apply IHx1. assumption. apply IHx2. assumption.
+  constructor. symmetry. assumption. constructor. apply IHx1. apply H1. apply IHx2. apply H1.
+  simpl in *. symmetry; assumption.
+
+  hnf.
+  intros x.
+  induction x; intros; destruct y; destruct z; try match goal with | H : eq_stmt _ _ |- _ => solve [inversion H] end;
+  try reflexivity; simpl in *; repeat match goal with 
+                                        | H : _ /\ _ |- _ => destruct H
+                                      end.
+  (constructor; eapply transitivity; eauto).
+  (repeat constructor; eapply transitivity; eauto).
+  (constructor; eapply transitivity; eauto).
+  (repeat constructor); try solve [ eapply transitivity; eauto ].
+  constructor. eapply IHx1; eauto. eapply IHx2; eauto.
+  repeat constructor. eapply transitivity; eauto. eapply IHx1; eauto. eapply IHx2; eauto.
+  eapply transitivity; eauto.
+Qed.
+
+Ltac solve_fv := 
+  (match goal with
+    | |- appcontext[@nonfv _] => unfold nonfv; simpl
+  end;
+  unfold nonfv_stmt;
+  try reflexivity;
+  try assumption;
+  intuition;
+  match goal with
+    | x : ?T, H : (forall _: ?T, _) |- _ => destruct (H x); solve_fv
+    | |- _ \/ _ => first [left; solve_fv | right; solve_fv]
+  end).
+       
+Ltac solve_instance := 
+  first [reflexivity 
+        | repeat constructor;
+          (repeat apply subst_nonfv); 
+          match goal with
+            | |- appcontext[@nonfv _] => solve_fv
+            | _ => firstorder
+          end].
+
+Instance Subst_stmt :
+ Subst stmt var var := mkSubst stmt var var (@eq_stmt var var Subst_var_var _ _ _ _ _) nonfv_stmt subst_stmt.
+Instance FVSubst_stmt : SubstFV stmt var var Subst_stmt.
+Proof.
+ constructor. intros. induction e;
+   match goal with 
+     | |- appcontext [@subst stmt] => 
+       unfold subst, Subst_stmt, subst_stmt 
+   end; solve_instance.
+Defined. 
+
+Definition eq_stmt_v := (eq_stmt (D := var) (R := var)).
+Definition eq_stmt_l := (eq_stmt (D := loc) (R := loc)).
+
+Instance Subst_stmt_var_proper : 
+  Proper (Logic.eq ==> eq_stmt_v ==> eq_stmt_v) subst.
+Proof.
+  pose (Subst_list_proper (A := var) (D := var) (R := var)).
+  pose (Subst_list_proper (A := loc) (D := var) (R := var)).
+  hnf; intros. rewrite H. 
+  hnf; intro. subst y.
+  induction x0; intros y eqh; destruct y;
+  try solve [inversion eqh]; try reflexivity;
+  match goal with | H : eq_stmt_v _ _ |- _ => inversion_clear H end;
+  repeat match goal with 
+           | H : eq _ _ |- _ => inversion_clear H 
+           | H : eq _ _ /\ _ |- _ => decompose [and] H; clear H; subst
+         end; try reflexivity.
+  simpl. 
+  unfold eq_stmt_v. unfold eq_stmt. rewrite H1. rewrite H2. rewrite H5. repeat constructor; reflexivity.
+  unfold eq_stmt_v. hnf. 
+  apply IHx0_1 in H. apply IHx0_2 in H0. constructor; assumption.
+  destruct H0.
+  hnf.
+  apply IHx0_1 in H. apply IHx0_2 in H0. unfold eq_stmt_v in *.
+  repeat constructor; (reflexivity || assumption).
+Qed.
+
+Instance Subst_stmt_loc : Subst stmt loc loc := 
+  mkSubst _ _ _ (@eq_stmt loc loc _ _ _ _ _ _) nonfv_stmt subst_stmt.
+Instance FVSubst_stmt_loc : SubstFV stmt loc loc _ := _.
+Proof.
+ constructor. intros. induction e;
+   try match goal with 
+     | |- appcontext [@subst stmt loc loc] => 
+       unfold subst, Subst_stmt_loc, subst_stmt
+   end; solve_instance.
+Defined.
+
+Instance Subst_stmt_loc_proper :
+  Proper (Logic.eq ==> eq_stmt_l ==> eq_stmt_l) subst.
+Proof.
+  pose (Subst_list_proper (A := var) (D := loc) (R := loc)).
+  pose (Subst_list_proper (A := var) (D := loc) (R := loc)).
+  pose (Subst_list_proper (A := loc) (D := loc) (R := loc)).
+  hnf; intros. rewrite H. 
+  hnf; intro. subst y.
+  induction x0; intros y eqh; destruct y;
+  try solve [inversion eqh]; try reflexivity;
+  match goal with | H : eq_stmt_l _ _ |- _ => inversion_clear H end;
+  repeat match goal with 
+           | H : eq _ _ |- _ => inversion_clear H 
+           | H : eq _ _ /\ _ |- _ => decompose [and] H; clear H; subst
+         end; try reflexivity.
+  hnf. 
+  rewrite H1. rewrite H2. rewrite H5. repeat constructor; reflexivity.
+  unfold eq_stmt_l. hnf. 
+  apply IHx0_1 in H. apply IHx0_2 in H0. constructor; assumption.
+  destruct H0.
+  hnf.
+  apply IHx0_1 in H. apply IHx0_2 in H0. unfold eq_stmt_l in *.
+  repeat constructor; (reflexivity || assumption).
+Qed.
+(* Definition subst_one (x : var) (e : expr) := *)
+(*   fun i => if eq_dec i x then e else (var_e i). *)
 
 Inductive modvars : stmt -> var -> Prop :=
 | mod_alloc : forall l v e, modvars (alloc_s l v e) v
@@ -202,3 +667,7 @@ Inductive modlocs : stmt -> loc -> Prop :=
 | modl_alloc : forall l v e, modlocs (alloc_s l v e) l
 | modl_proc : forall f xs r os ls l,
                 In l ls -> modlocs (proc_s f xs r os ls) l.
+
+(** Dummy instance! **)
+Instance Subst_var_expr_dummy : Subst var var expr :=
+  mkSubst _ _ _ Logic.eq (fun v x => v <> x) (fun s v => v).
