ProgramLogic.v
@@ -10,3 +10,80 @@ Require Export Logic.
 Declare Module Semax : SEMAX.
 Import Semax.
 Export Semax.
+
+Class SubstAssert (D R : Type) `{S : Subst world D R} `{S : Subst assert D R} : Type := mkSubstAssert
+{
+  subst_wld :
+    forall s (P : assert),
+      subst s P = (fun w => P (subst s w))
+  ;
+  subst_andp : 
+    forall P Q (s : subst_t D R),
+      subst s (andp P Q) = andp (subst s P) (subst s Q)
+  ;
+  subst_orp : 
+    forall  P Q (s : subst_t D R),
+      subst s (orp P Q) = orp (subst s P) (subst s Q)
+  ;
+  subst_sepcon : 
+    forall  P Q (s : subst_t D R),
+      subst s (sepcon P Q) = sepcon (subst s P) (subst s Q)
+  ;
+  subst_imp : 
+    forall  P Q (s : subst_t D R),
+      subst s (imp P Q) = imp (subst s P) (subst s Q)
+  ;
+  subst_pure :
+    forall  (P : assert) (s : subst_t D R),
+      pure P -> pure (subst s P)
+  ;
+  nonfv_andp :
+    forall (P Q : assert) (x : D),
+      (nonfv P x) /\ (nonfv Q x) -> nonfv (andp P Q) x
+  ;
+  nonfv_orp :
+    forall (P Q : assert) (x : D),
+      (nonfv P x) /\ (nonfv Q x) -> nonfv (orp P Q) x
+  ;
+  nonfv_imp :
+    forall (P Q : assert) (x : D),
+      (nonfv P x) /\ (nonfv Q x) -> nonfv (imp P Q) x
+  ;
+  nonfv_sepcon :
+    forall (P Q : assert) (x : D),
+      (nonfv P x) /\ (nonfv Q x) -> nonfv (sepcon P Q) x
+  ;
+  nonfv_TT :
+    forall (x : D),
+      nonfv TT x
+  ; nonfv_emp :
+    forall (x : D),
+      nonfv emp x
+}.
+
+Instance SubstAssert_Loc : SubstAssert loc loc := _.
+Proof. 
+  constructor; intros; try firstorder;
+  simpl in *; unfold nonfv_assert in *;  destruct H;
+  intros w va;
+  specialize (H w va); specialize (H0 w va);
+  rewrite H; rewrite H0; reflexivity.
+Defined.
+
+Instance SubstAssert_Var_Expr : SubstAssert var expr := _.
+Proof. 
+  constructor; intros; try firstorder;
+  simpl in *; unfold nonfv_assert in *;  destruct H;
+  intros w va;
+  specialize (H w va); specialize (H0 w va);
+  rewrite H; rewrite H0; reflexivity.
+Defined.
+
+Instance SubstAssert_Var_Var : SubstAssert var var := _.
+Proof. 
+  constructor; intros; try firstorder;
+  simpl in *; unfold nonfv_assert in *;  destruct H;
+  intros w va;
+  specialize (H w va); specialize (H0 w va);
+  rewrite H; rewrite H0; reflexivity.
+Defined.
