Subst.v
@@ -1,33 +1,237 @@
 Add LoadPath "vst".
 
+Require Export Coq.Structures.Equalities.
 Require Import Coq.Unicode.Utf8.
 Require Import msl.eq_dec.
 Require Import List.
 Import ListNotations.
+Require Export Coq.Classes.Morphisms.
+Import ProperNotations.
+Require Import Setoid Morphisms RelationClasses Equivalence.
 
-Definition subst_t (D : Type) (R : Type) := D -> R.
+Definition subst_t (D : Type) (R : Type) := D -> option R.
+
+Definition subst_one {D R : Type} {E: EqDec D} (x : D) (e : R) i := 
+  if eq_dec x i then Some e else None.
+(* Definition subst_one { D R : Type } { E : EqDec D } (d : D) (r : R) : subst_t D R := *)
+(*   fun d' => if eq_dec d d' then Some r else None. *)
 
 (* Definition wf_subst{A : Type} (s : subst_t A) : Prop  := NoDup (fst (split s)). *)
+Class Subst (A D R : Type) := mkSubst {
+  eq : A -> A -> Prop
+  ;
+  nonfv: A -> D -> Prop
+  ;
+  subst: subst_t D R -> A -> A 
+}.
 
-Class Subst (A D R : Type) : Type :=
-  subst: subst_t D R -> A -> A.
+Class SubstFV (A D R : Type) `( S : Subst A D R ) := mkSubstFV {
+  subst_nonfv: 
+    forall (s : subst_t D R) e, 
+      (forall x, s x <> None -> nonfv e x) -> eq (subst s e) e
+}.
 
-Fixpoint subst_prod (A B D R : Type) (SA : Subst A D R) (SB : Subst B D R) (s : subst_t D R) (p : (A * B)) :=
+Definition fv_prod {A B D R : Type} `{SA :Subst A D R} `{SB : Subst B D R} (p : (A * B)) :=
+  fun x => 
+    match p with
+      | (p1, p2) => nonfv p1 x /\ nonfv p2 x
+    end.
+
+Definition subst_prod {A B D R : Type} {SA : Subst A D R} {SB : Subst B D R} (s : subst_t D R) (p : (A * B)) :=
   match p with
     | (p1, p2) => (subst s p1, subst s p2)
   end.
 
-Instance Subst_prod (A B D R : Type) (SA : Subst A D R) (SB : Subst B D R): Subst (A * B) D R := 
-  subst_prod A B D R SA SB.
+Require Import Relation_Definitions.
+Require Import Coq.Classes.RelationClasses.
+
+Definition eq_prod {A B D R : Type} 
+                   {SA : Subst A D R} {SB : Subst B D R} 
+                   (p1 : (A * B)) (p2 : (A * B)) :=
+  let (a, b) := p1 in
+  let (x, y) := p2 in
+  @eq A D R SA a x /\ @eq B D R SB b y.
+
+Instance Eq_eqProd {A B D R : Type} {SA : Subst A D R} {SB : Subst B D R} 
+         {E1 : Equivalence (eq (A := A)) }
+         {E2 : Equivalence (eq (A := B)) }
+: Equivalence (@eq_prod A B D R SA SB).
+Proof.
+  constructor.
+  + hnf; destruct x; unfold eq_prod. 
+    constructor; reflexivity.
+  + hnf. destruct x. destruct y. intros. unfold eq_prod in *. 
+    constructor; symmetry; apply H.
+  + hnf. destruct x. destruct y. destruct z.
+    intros.
+    unfold eq_prod in *.
+    destruct H. destruct H0.
+    constructor.
+    apply (transitivity H H0).
+    apply (transitivity H1 H2).
+Qed.
+
+Instance Subst_prod (A B D R : Type) `{SA : Subst A D R } `{SB : Subst B D R}: Subst (A * B) D R.
+Proof.
+  refine (mkSubst _ _ _ eq_prod fv_prod subst_prod). 
+Defined.
+
+Instance FVSubst_prod {A B D R : Type} `{ SA : SubstFV A D R } `{ SB : SubstFV B D R } 
+          : SubstFV (A * B) D R _ := _.
+Proof.
+  constructor.
+  intros.
+  destruct e.
+  unfold subst; simpl.
+  constructor;
+  apply subst_nonfv; 
+  repeat intro; apply H; intuition.
+Defined.
+
+Instance Subst_prod_proper 
+         {A B D R : Type} 
+         (SA : Subst A D R)
+         (SB : Subst B D R)
+         {E1: Equivalence (eq (A := A))}
+         {E2: Equivalence (eq (A := B))}
+         {P1: Proper (Logic.eq ==> eq (A := A) ==> eq (A := A)) subst }
+         {P2: Proper (Logic.eq ==> eq (A := B) ==> eq (A := B)) subst }
+         : Proper (Logic.eq ==> eq (A := (A * B)) ==> eq (A := (A * B))) subst.
+Proof.
+  hnf.
+  intros s1 s2 ? [x1 y1] [x2 y2] eqxy.
+  subst.
+  inversion eqxy.
+  simpl.
+  rewrite H.
+  rewrite H0.
+  constructor; reflexivity.
+Qed.
 
 Fixpoint subst_list (A D R : Type) (SA : Subst A D R) (s : subst_t D R) (l : list A) :=
   match l with
     | nil => []
     | h :: t => subst s h :: subst_list A D R SA s t
   end.
+
+Fixpoint fv_list {A D R : Type} {SA : Subst A D R} (l : list A) x :=
+  match l with
+    | nil => False
+    | h :: t => @nonfv A D R SA h x /\ @fv_list A D R SA t x
+  end.
+
+Fixpoint eq_list { A D R : Type } { SA : Subst A D R } (l1 : list A) (l2 : list A) :=
+  match (l1, l2) with
+    | ([], []) => True
+    | (h1 :: t1, h2 :: t2) => @eq A D R SA h1 h2 /\ eq_list t1 t2
+    | _ => False
+  end.
+
+Instance Eq_eqList { A D R : Type }{ SA : Subst A D R } { E : Equivalence (eq (A := A)) } 
+: Equivalence (@eq_list A D R SA).
+Proof.
+  constructor.
+  hnf. induction x. reflexivity. simpl. constructor.  reflexivity. assumption.
+  hnf. intro x. induction x; intros; destruct y.
+  constructor. 
+  inversion H.
+  inversion H.
+  simpl in *.
+  constructor.
+  symmetry.
+  apply H.
+  apply IHx. apply H.
+  (** transitivity **)
+  hnf.
+  induction x; intros; destruct y; destruct z; try reflexivity;
+  try match goal with 
+        | H : eq [] ?x |- _ => inversion H
+        | H : eq ?x [] |- _ => inversion H
+        | H : eq_list [] ?x |- _ => inversion H
+        | H : eq_list ?x [] |- _ => inversion H
+      end.
+  inversion H.
+  simpl in *.
+  destruct H. destruct H0.
+  constructor. eapply transitivity; eauto. eapply IHx; eauto.
+Qed.
   
-Instance Subst_list (A D R : Type) (SA : Subst A D R) : Subst (list A) D R := 
-  subst_list A D R SA.
-(* Instance Subst_prod_list (A B D R : Type) (S : Subst A D R) : Subst (list (A * A)) D R := _. *)
-(* Definition wf_subst (X : Type) (s : subst_t X) := *)
-(*   NoDup (fst (split s)). *)
+Instance Subst_list {A D R : Type} {SA : Subst A D R} { E: Equivalence (eq (A := A)) }
+: Subst (list A) D R := 
+  (mkSubst _ _ _ eq_list fv_list (subst_list A D R SA)).
+
+Instance FVSubst_list {A D R : Type} `{SA : SubstFV A D R} { E: Equivalence (eq (A := A)) }
+: SubstFV (list A) D R _.
+Proof.
+  constructor.
+  intros.
+  induction e.
+  + reflexivity.
+  + unfold subst_list; fold subst_list.
+    unfold fv_list in *. fold fv_list in *.
+    simpl; constructor.
+    apply subst_nonfv.
+    repeat intro. apply H. intuition.
+    rewrite IHe.
+    reflexivity.
+    repeat intro. apply H. intuition.
+Defined.
+
+Instance Subst_list_proper 
+  {A D R : Type} {SA : Subst A D R} {E : Equivalence (eq (A := A))} 
+  {P : Proper (Logic.eq ==> eq ==> eq) (subst (A := A))}
+  : Proper (Logic.eq ==> eq ==> eq) (subst (A := list A)).
+Proof.
+  hnf.
+  intros s1 s2 ?. subst.
+  intro l. induction l as [ | h l ]; intros; destruct y.
+  + reflexivity.
+  + inversion H.
+  + inversion H.
+  + simpl. destruct H. rewrite H.
+    constructor. reflexivity. apply IHl. assumption.
+Qed.
+
+Lemma subst_cons :
+  forall { A D R : Type } { S : Subst A D R } { E : Equivalence (@eq _ _ _ S) }
+         (s : subst_t D R) h t,
+    subst s (h :: t) = subst s h :: subst s t.
+Proof. firstorder. Qed.
+
+Lemma subst_app :
+  forall { A D R : Type } { S : Subst A D R } {E : Equivalence (@eq _ _ _ S) }
+         (s : subst_t D R) l1 l2,
+    subst s (l1 ++ l2) = subst s l1 ++ subst s l2.
+Proof.
+  intros.
+  induction l1.
+  reflexivity.
+  rewrite subst_cons.
+  simpl. f_equal. apply IHl1.
+Qed.
+
+Lemma subst_pair :
+  forall { X Y D R : Type } { SX : Subst X D R } {SY : Subst Y D R} 
+         (x : X) (y : Y) (s : subst_t D R),
+    subst s (x, y) = (subst s x, subst s y).
+Proof. reflexivity. Qed.
+
+Lemma subst_rev :
+  forall { A D R : Type } { S : Subst A D R } { E : Equivalence (@eq _ _ _ S) }
+         s l,
+    subst s (rev l) = rev (subst s l).
+Proof.
+  induction l; eauto.
+  rewrite subst_cons.
+  simpl.
+  setoid_rewrite subst_app.
+  rewrite IHl.
+  reflexivity.
+Qed.
+
+Ltac step_subst := 
+  try first [ rewrite subst_pair
+            | rewrite subst_cons
+            | rewrite subst_app
+            | rewrite subst_rev
+            ].
