Translation.v
@@ -6,22 +6,25 @@ Require Import Language.
 Require Export ProgramLogic.
 Require Import Subst.
 Require Import List.
+Require Import ListSet.
 Import ListNotations.
 Require Import Coq.Unicode.Utf8.
 Require Import msl.eq_dec.
-
-Instance EQ_EQUIVALENCE : Equivalence (@eq assert) := _.
 
 Set Implicit Arguments.
 
 Open Scope logic.
 
+Definition OkRef x l s :=
+(!!(eval s x = eval s (locvar_e l))
+                        && !!(eval s x <> Some null_v)
+                        && !!(eval s x <> None)).
+
 Definition sep_base (x:expr) (t:base_type) : assert :=
   match t with 
     | int_t   => (EX n : nat, eval_to x (int_v n))
-    | ref_t l => (fun s => !!(eval s x = eval s (locvar_e l))
-                        && !!(eval s x <> null_v))
-    | null_t  => (fun s => !!(eval s x = null_v))
+    | ref_t l => OkRef x l
+    | null_t  => eval_to x null_v
   end && emp.
 
 Fixpoint sep_pred (p:reft_prop) : assert :=
@@ -45,10 +48,9 @@ Fixpoint sep_env (Γ : type_env) : assert :=
   end && emp.
 
 Definition sep_heap_bind l (xt : type_binding) : assert :=
-  let (x, t) := xt in
-      (eval_to (locvar_e l) null_v) 
-        || (emapsto (locvar_e l) (var_e x)
-            * sep_ty (var_e x) t).
+  (eval_to (locvar_e l) null_v) 
+    || (emapsto (locvar_e l) (var_e (fst xt))
+        * sep_ty (var_e (fst xt)) (snd xt)).
 
 Fixpoint sep_heap' es :=
   match es with
@@ -70,10 +72,27 @@ Fixpoint sep_guards (Δ : guards) : assert :=
     | p :: Δ' => sep_pred p && sep_guards Δ'
   end && emp.
 
+Definition binds (h : heap_env) :=
+  fold (fun _ xt bs => set_add eq_dec (fst xt) bs) h [].
+
+Definition locs (h : heap_env) :=
+  fold (fun l _ bs => set_add eq_dec l bs) h [].
+
+Definition mod_vars S :=
+  let h1s := binds (s_heap_in S)  in
+  let h2s := binds (s_heap_out S) in
+  set_diff eq_dec h2s h1s.
+
+Definition mod_locs S :=
+  let h1s := locs (s_heap_in S)  in
+  let h2s := locs (s_heap_out S) in
+  set_diff eq_dec h2s h1s.
+  
+
 Definition sep_schema (f:pname) (s:stmt) (S:proc_schema) : procspec := 
   match S with
     | mkSchema xs ts hi ho (x, t) =>
-      (f, mkProc xs x [] [] s, 
+      (f, mkProc xs x (mod_vars S) (mod_locs S) s, 
           sep_env (combine xs ts) * sep_heap hi,
           sep_ty (var_e x) t * sep_heap ho)
   end.
@@ -86,6 +105,137 @@ Fixpoint sep_proc_env (Φ : proc_env) : procspecs :=
 
 Definition disj_subst Γ (θ : var -> expr) :=
   θ ν = (var_e ν) /\ forall x, var_in x Γ -> θ x = (var_e x).
+
+Lemma help_in_rev :
+  forall l L, (exists (e : type_binding), InA (eq_key_elt (elt := type_binding)) (l,e) L)
+                       <-> (exists (e : type_binding), InA (eq_key_elt (elt := type_binding)) (l, e) (rev L)).
+Proof.
+  intros.
+  split; intros; destruct H; exists x; apply InA_rev; eauto using HE_Props.eqke_equiv.
+Qed.
+
+Lemma help_in_rev' :
+  forall b L, (exists l (e : reft_type), InA (eq_key_elt (elt := type_binding)) (l,(b,e)) L)
+                       <-> (exists l (e : reft_type), InA (eq_key_elt (elt := type_binding)) (l, (b, e)) (rev L)).
+Proof.
+  intros.
+  split; intros; destruct H; destruct H; exists x, x0; apply InA_rev; eauto using HE_Props.eqke_equiv.
+Qed.
+
+Lemma locs_in_heap :
+  forall h l,
+    loc_in l h <-> In l (locs h).
+Proof.
+  intros.
+  unfold loc_in.
+  unfold locs.
+  rewrite <- HE_Props.F.in_find_iff.
+  rewrite HE_Props.F.elements_in_iff.
+  rewrite HE_Props.fold_spec_right.
+  split. intros.
+  destruct H.
+  rewrite <- InA_rev in H.
+  induction (rev (elements h)).
+  inv H.
+  unfold HE_Props.uncurry in *.
+  inv H.
+  apply set_add_intro2. apply H1.
+  apply set_add_intro1; apply IHl0. easy.
+  apply HE_Props.eqke_equiv.
+  intros. 
+  rewrite help_in_rev.
+  induction (rev (elements h)).
+  inv H.
+  unfold HE_Props.uncurry in *.
+  unfold fold_right in H. fold fold_right in H.
+  apply set_add_elim in H. destruct H.
+  rewrite H. exists (snd a). left. destruct a. reflexivity.
+  apply IHl0 in H. destruct H. exists x. right. assumption.
+Qed.
+
+Lemma ack_foo :
+  forall L b,
+     b ∈ fold_right
+          (HE_Props.uncurry
+             (λ (_ : key) (xt : var * reft_type) (bs : set var),
+              set_add eq_dec (fst xt) bs)) []
+         L  ->
+   exists (l : key) (e : reft_type),
+     InA (eq_key_elt (elt:=type_binding)) (l, (b, e)) L.
+Proof.
+  intros.
+  induction L. inv H.
+  simpl in H. unfold HE_Props.uncurry in *.
+  apply set_add_elim in H.
+  destruct H.
+  rewrite H.
+  exists (fst a). exists (snd (snd a)). left. destruct a. destruct p. reflexivity.
+  apply IHL in H. destruct H. destruct H. exists x, x0.
+  right. assumption.
+Qed.
+
+Lemma binds_in_heap :
+  forall (h : heap_env) (b : var),
+    bind_in b h <-> In b (binds h).
+Proof.
+  intros.
+  unfold bind_in.
+  unfold binds.
+  setoid_rewrite <- HE_Props.F.find_mapsto_iff.
+  setoid_rewrite HE_Props.F.elements_mapsto_iff.
+  rewrite HE_Props.fold_spec_right.
+  split. intros.
+  destruct H. destruct H. rewrite <- InA_rev in H.
+  induction (rev ((elements (elt := var * reft_type)) h)). inv H.
+  unfold fold_right; fold fold_right. unfold HE_Props.uncurry in *.
+  inv H.
+  apply set_add_intro2. destruct a. destruct p. inv H1. simpl in *. congruence.
+  apply set_add_intro1. apply IHl. easy.
+  apply HE_Props.eqke_equiv.
+  intro.
+  rewrite help_in_rev'.
+  eauto using ack_foo.
+Qed.
+
+Lemma new_mod_locs_schema :
+  forall S l,
+    In l (mod_locs S) <-> (loc_in l (s_heap_out S) /\ ~ loc_in l (s_heap_in S)).
+Proof.
+  intros. destruct S as [xs ts hi ho rt]. simpl.
+  split; intros.
+  unfold mod_locs in *.
+  split.
+  apply locs_in_heap.
+  simpl in *.
+  apply set_diff_elim1 in H. easy.
+  rewrite locs_in_heap.
+  eapply set_diff_elim2; eauto.
+  destruct H.
+  unfold mod_locs.
+  apply set_diff_intro.
+  apply locs_in_heap. apply H.
+  rewrite locs_in_heap in H0. apply H0.
+Qed.
+
+Lemma new_mod_vars_schema :
+  forall S v,
+    In v (mod_vars S) <-> (bind_in v (s_heap_out S) /\ ~ bind_in v (s_heap_in S)).
+Proof.
+  intros. destruct S as [xs ts hi ho rt]. simpl.
+  split; intros.
+  unfold mod_vars in *.
+  split.
+  apply binds_in_heap.
+  simpl in *.
+  apply set_diff_elim1 in H. easy.
+  rewrite binds_in_heap.
+  eapply set_diff_elim2; eauto.
+  destruct H.
+  unfold mod_vars.
+  apply set_diff_intro.
+  apply binds_in_heap. apply H.
+  rewrite binds_in_heap in H0. apply H0.
+Qed.
 
 Lemma sep_base_pure : 
   forall x t, 
@@ -141,13 +291,6 @@ Proof.
   normalize.
   apply andp_left2.
   apply derives_refl.
-Qed.
-
-Lemma subst_pure :
-  forall s P,
-    pure P -> pure (subst_pred s P).
-Proof.
-  firstorder.
 Qed.
 
 Lemma pure_andp_1 :
@@ -334,11 +477,802 @@ Proof.
   assert (sep_heap H1 * sep_heap H2 = fold f H1 (fold f H2 emp)).
   apply sep_heap_split''.
   rewrite H3.
-  apply (Partition_fold (eqA := eq)).
-  apply EQ_EQUIVALENCE.
+  apply (Partition_fold (eqA := Logic.eq)).
+  apply eq_equivalence.
   solve_proper.
   hnf. intros. extensionality. 
   repeat rewrite <- sepcon_assoc. 
   rewrite sepcon_comm with (P := sep_heap_bind k e). reflexivity.
   assumption.
 Qed.
+
+Class SubstBase ( D R : Type )
+  `{SL : Subst loc D R} `{SB : @Subst base_type D R}
+  `{SE : SubstExpr D R} `{SA : SubstAssert D R}
+  `{S  : @SubstFV base_type D R SB} : Type := {
+  subst_int_t : 
+    forall (s : subst_t D R), subst s int_t = int_t
+  ;
+  subst_null_t : 
+    forall (s : subst_t D R), subst s null_t = null_t
+  ;
+  subst_ref_t : 
+    forall l (s : subst_t D R), subst s (ref_t l) = ref_t (subst s l)
+  ;
+  nonfv_base_t :
+    forall bt e (x : D),
+      nonfv e x ->
+      nonfv bt x -> nonfv (sep_base e bt) x
+  }.
+
+Ltac f_equalize :=
+  match goal with
+    | |- (fun _ => _) = (fun _ => _) => extensionality
+    | |- (_ && _) _ = (_ && _) _ => f_equal; f_equalize
+    | |- (_ && _) = (_ && _) => f_equal; f_equalize
+    | |- EX _:_, _ = EX _:_, _ => f_equal; f_equalize
+    | _ => idtac
+  end.
+
+Lemma SubstProp_var :
+  forall p (x : var),
+    nonfv p x -> nonfv (sep_pred p) x.
+Proof.
+  intros.
+  induction p; try easy.
+  + unfold sep_pred. apply nonfv_andp.
+    simpl. split.
+    simpl in H.
+    unfold nonfv_assert. intros. f_equalize.
+    repeat rewrite <- nonfv_eval. reflexivity. easy. easy. easy.
+  + unfold sep_pred. fold sep_pred. apply nonfv_andp.
+    split.
+    apply nonfv_imp. split.
+    apply IHp. apply H. easy. easy.
+  + unfold sep_pred; fold sep_pred; apply nonfv_andp. split.
+    apply nonfv_andp. split.
+    apply IHp1. apply H. apply IHp2. apply H. easy.
+  + unfold sep_pred; fold sep_pred; apply nonfv_andp. split.
+    apply nonfv_orp. split.
+    apply IHp1. apply H. apply IHp2. apply H. easy.
+Qed.
+
+Ltac nonfv_base_simp := match goal with
+                          | |- nonfv (_ && _) _ => apply nonfv_andp; split; nonfv_base_simp
+                          | |- nonfv ?f _ => unfold f; nonfv_base_simp
+                          | |- nonfv (?f _) _ => unfold f; nonfv_base_simp
+                          | |- nonfv (?f _ _) _ => unfold f; nonfv_base_simp
+                          | b : base_type |- appcontext[match ?b with _ => _ end]   =>
+                            destruct b; unfold eval_to; nonfv_base_simp
+                          | _ => idtac
+                        end.
+
+Ltac crush_substbase := 
+  constructor; try firstorder;
+  intros;
+  nonfv_base_simp;
+  simpl; unfold nonfv_assert; intros; f_equalize; try rewrite <- nonfv_eval; easy.
+
+Instance SepBase_var_var : @SubstBase var var _ _ _ _ _ _ _ _ _ _ _ _ := _.
+Proof. crush_substbase. Defined.
+
+Instance SepBase_var_expr : @SubstBase var expr _ _ _ _ _ _ _ _ _ _ _ _  := _.
+Proof.  crush_substbase. Defined.
+
+Instance SepBase_loc_loc : @SubstBase loc loc _ _ _ _ _ _ _ _ _ _ _ _  := _.
+Proof. 
+  constructor; try firstorder; intros; nonfv_base_simp.
+  simpl. unfold nonfv_assert. intros. f_equalize. rewrite <- nonfv_eval; easy.
+  simpl. unfold nonfv_assert. intros. f_equalize. rewrite <- nonfv_eval; easy. easy.
+  simpl. unfold nonfv_assert. intros. f_equalize. f_equal. f_equal. rewrite <- nonfv_eval; easy.
+  unfold subst, subst_one. simpl. unfold runloc. simpl.
+  destruct (eq_dec.eq_dec x l). compute in H0. subst x. congruence. easy.
+  rewrite <- nonfv_eval; easy.
+  rewrite <- nonfv_eval; easy.
+  easy.
+Defined.
+
+Lemma SubstTy_var :
+  forall e t (x : var),
+    nonfv e x -> nonfv t x -> nonfv (sep_ty e t) x.
+Proof.
+  intros. destruct t0.
+  unfold sep_ty.
+  apply nonfv_andp. split.
+  apply nonfv_andp. split.
+  apply nonfv_base_t. easy. destruct reft_base; firstorder.
+  apply SubstProp_var.
+  eauto.
+  induction reft_r; try easy.
+  simpl. split.
+  simpl in H0. unfold nonfv_reft_t in H0. destruct H0. simpl in H1. 
+  pose nonfv_subst. apply n. clear n. apply H1. apply H.
+  pose nonfv_subst. apply n. clear n. apply H0. apply H.
+  simpl. apply IHreft_r. assumption.
+  simpl. simpl in H0. unfold nonfv_reft_t in H0.  simpl in H0. destruct H0.
+  split. 
+  apply IHreft_r1; split; easy. 
+  apply IHreft_r2; split; easy. 
+  simpl. simpl in H0. unfold nonfv_reft_t in H0.  simpl in H0. destruct H0. split.
+  apply IHreft_r1; split; easy. 
+  apply IHreft_r2; split; easy. 
+  easy.
+Qed.
+
+Lemma foo :  forall (P Q : assert), (fun w => (P w && Q w)) = ((fun w => P w) && (fun w => Q w)).
+  firstorder.
+Qed.
+
+Class SubstPull ( D R : Type )  {S1 : Subst world D R} `{S2 : Subst expr D R} : Type 
+:=
+   subst_eval : 
+     forall (w : world) (s : subst_t D R) (x : expr),
+       eval w (subst s x) = eval (subst s w) x .
+
+Instance SubstPull_var : @SubstPull var var _ _.
+Proof.
+  hnf.
+    unfold subst. simpl.
+    induction x.
+    + reflexivity.
+    + simpl. unfold subst_var. unfold stk. destruct w. destruct p. simpl.
+      destruct (s v). reflexivity. reflexivity.
+    + reflexivity.
+    + simpl. rewrite IHx1. rewrite IHx2. reflexivity. 
+Qed.
+
+Instance SubstPull_expr : @SubstPull var expr _ _.
+Proof.
+  hnf.
+    unfold subst. simpl.
+    induction x.
+    + reflexivity.
+    + simpl.
+      unfold stk. destruct w. destruct p. simpl.
+      destruct (s v). reflexivity. reflexivity.
+    + reflexivity.
+    + simpl. rewrite IHx1. rewrite IHx2. reflexivity.
+Qed.
+
+Instance SubstPull_loc : @SubstPull loc loc _ _.
+Proof.
+  hnf.
+    unfold subst. simpl.
+    induction x.
+    + reflexivity.
+    + reflexivity. 
+    + simpl. destruct w. destruct p. unfold runloc. simpl. unfold subst_loc. simpl.
+      destruct (s l). destruct (l0 l1); reflexivity.
+      destruct (l0 l); reflexivity.
+    + simpl. rewrite IHx1. rewrite IHx2. reflexivity.
+Qed.
+
+Section Subst.
+
+  (** Base Assumptions **)
+  Context { D R : Type}.
+  Context { EqDecD : EqDec D}.
+  Context {Sub_Loc : Subst loc D R}.
+  Context {Sub_LocFV : SubstFV loc D R Sub_Loc}.
+  Context {Sub_Var : Subst var D R}.
+  Context {Sub_Expr : Subst expr D R}.
+  Context {Sub_ExprFV : SubstFV expr D R Sub_Expr}.
+  Context {Sub_Wld : Subst world D R}.
+  (* Context {SubWld : SubstWorld D R Sub_Var Sub_Wld}. *)
+  Context {Sub_Assrt : Subst assert D R}.
+  Context {SubAssrt : @SubstAssert D R Sub_Wld Sub_Assrt}.
+  Definition eq_loc  := @eq _ _ _ Sub_Loc.
+  Definition eq_var  := @eq _ _ _ Sub_Var.
+  Definition eq_expr := @eq _ _ _ Sub_Expr.
+  Context { Eq_eq_loc : Equivalence eq_loc}.
+  Context { Eq_eq_var : Equivalence eq_var}.
+  Context { Eq_eq_expr : Equivalence eq_expr}.
+
+  Context { SubExpr : @SubstExpr D R EqDecD Sub_Loc Sub_Expr Sub_ExprFV Sub_Wld}.
+
+  (** Base Types **)
+  Instance Sub_Base : Subst base_type D R :=  @Subst_base D R Sub_Loc Eq_eq_loc.
+  Instance Sub_BaseFV : SubstFV base_type D R Sub_Base := 
+    @FVSubst_base D R Sub_Loc Sub_LocFV Eq_eq_loc.
+  Context { SubBase : (@SubstBase D R Sub_Loc Sub_Base EqDecD Sub_Loc
+                                  Sub_Expr Sub_ExprFV Sub_Wld SubExpr Sub_Wld Sub_Assrt 
+                                  SubAssrt Sub_BaseFV)}.
+  Instance Eq_eq_base : Equivalence (@eq base_type D R Sub_Base) :=
+    @Eq_eqBase D R Sub_Loc Eq_eq_loc.
+ 
+  (** Props **)
+  Instance Sub_Prop : Subst reft_prop D R := @Subst_prop D R Sub_Expr.
+  Instance Eq_eq_Prop : Equivalence (@eq reft_prop D R Sub_Prop) :=
+    @Eq_eqProp D R Sub_Expr Eq_eq_expr.
+
+  (** Reft Types **)
+  Instance Sub_Type : Subst reft_type D R := @Subst_reft D R Sub_Base Sub_Prop.
+  Instance Eq_eq_Type : Equivalence (@eq reft_type D R Sub_Type) :=
+    @Eq_eq_reft_r D R Sub_Base Sub_Prop Eq_eq_base Eq_eq_Prop.
+
+  Instance Sub_TyBi : Subst type_binding D R := 
+    @Subst_prod var reft_type D R Sub_Var Sub_Type.
+  Instance Eq_eq_TyBi : Equivalence (@eq type_binding D R Sub_TyBi) :=
+    @Eq_eqProd var reft_type D R Sub_Var Sub_Type Eq_eq_var Eq_eq_Type.
+
+  Instance Sub_Ctx  : Subst type_env D R := 
+    @Subst_list type_binding D R Sub_TyBi Eq_eq_TyBi.
+  Instance Sub_Heap : Subst heap_env D R :=
+    @Subst_heap D R Sub_Loc Sub_TyBi Eq_eq_loc Eq_eq_TyBi.
+  Instance Sub_HeapBinds : Subst (list (loc * type_binding)) D R :=
+    @Subst_list (loc * type_binding) D R (@Subst_prod loc type_binding D R Sub_Loc Sub_TyBi)
+    (@Eq_eqProd loc type_binding D R Sub_Loc Sub_TyBi Eq_eq_loc Eq_eq_TyBi).
+  
+  (** Pulling **) 
+  Context { Sub_Pull_Expr : @SubstPull D R Sub_Wld Sub_Expr}.
+
+Lemma sep_base_subst :
+  forall (s : subst_t D R) x b,
+    sep_base (subst s x) (subst s b) = subst s (sep_base x b).
+Proof.
+  intros.
+  unfold sep_base.
+  destruct b;
+  first [rewrite subst_int_t | rewrite subst_null_t | rewrite subst_ref_t].
+  simpl. rewrite subst_wld. extensionality.
+  f_equal. f_equal. extensionality.
+  unfold eval_to. simpl. rewrite subst_eval. reflexivity.
+  unfold eval_to. extensionality. rewrite subst_wld.
+  simpl. f_equal. f_equal. f_equal.
+  f_equal. rewrite subst_eval. reflexivity.
+  rewrite subst_andp.
+  f_equal.
+  rewrite subst_wld. extensionality w.
+  unfold OkRef.
+  rewrite subst_eval. f_equal. f_equal.
+  f_equal. f_equal.
+  rewrite <- subst_eval.
+  f_equal. f_equal. 
+  rewrite <- subst_locvar.
+  reflexivity.
+  simpl.
+  rewrite subst_wld. reflexivity.
+Qed.
+
+Lemma sep_pred_subst :
+  (* forall { D R : Type }  *)
+  (*        `{Sl : Subst loc D R}  *)
+  (*        `{SFV : SubstFV expr D R} *)
+  (*        `{SFVB : SubstFV base_type D R} *)
+  (*        { E : EqDec D } *)
+  (*        {SW : Subst world D R} *)
+  (*        {S : SubstExpr D R (Sl := Sl)}  *)
+  (*        `{S' : SubstBase D R (SL := Sl)}  *)
+  (*        {SW : Subst world D R}  *)
+  (*        {SA : Subst assert D R} *)
+  (*        `{S'''' : (@SubstPull D R SW _)}  *)
+  (*        `{S : @SubstAssert D R SW _} *)
+         forall (s : subst_t D R) x,
+    sep_pred (subst s x) = subst s (sep_pred x).
+Proof.
+  intros.
+  induction x.
+  + simpl; rewrite subst_wld; reflexivity.
+  + simpl. rewrite subst_wld. extensionality. f_equal. do 2 rewrite subst_eval. reflexivity.
+  + unfold sep_pred. 
+    simpl subst at 1. unfold subst_prop; fold subst_prop.
+    rewrite subst_andp. f_equal.
+    rewrite subst_imp. f_equal. apply IHx.
+    rewrite subst_wld. reflexivity.
+    rewrite subst_wld. reflexivity.
+  + simpl subst at 1. unfold subst_prop; fold subst_prop. 
+    unfold sep_pred.
+    rewrite subst_andp. rewrite subst_andp.
+    fold sep_pred.
+    f_equal. f_equal. assumption. assumption. rewrite subst_wld. reflexivity.
+  + simpl subst at 1. unfold subst_prop. fold subst_prop. 
+    unfold sep_pred.
+    rewrite subst_andp. rewrite subst_orp.
+    fold sep_pred.
+    f_equal. f_equal. assumption. assumption. rewrite subst_wld. reflexivity.
+Qed.
+
+Lemma subst_ty_base_pred :
+  forall {D R : Type} {S : Subst assert D R } (s : subst_t D R) v b p,
+    subst s (sep_ty v { ν : b | p }) =
+    subst s (sep_base v b && sep_pred (subst (subst_one ν v) p) && emp).
+Proof.
+  firstorder.
+Qed.
+
+Lemma commuting_subst :
+  forall (s : subst_t D R) x (e : expr),
+    (subst s (var_e ν) = var_e ν) ->
+    (forall (x : expr), (nonfv x ν) -> nonfv (subst s x) ν) ->
+    subst (subst_one ν (subst s x)) (subst s e) = subst s (subst (subst_one ν x) e).
+Proof.
+  intros.
+  induction e.
+  simpl. rewrite subst_value. reflexivity.
+  compare ν v.
+  intro.
+  subst v. 
+  rewrite H. simpl subst at 4. unfold subst_expr. unfold subst_one. simpl.
+  destruct (eq_dec.eq_dec ν ν). reflexivity. congruence.
+
+  intros.
+  assert (subst (subst_one ν (subst s x)) (subst s (var_e v)) = subst s (var_e v)).
+  pose (subst_nonfv (subst_one ν (subst s x)) (subst s (var_e v))).
+  rewrite e. reflexivity.
+  intro v'.
+  unfold subst_one.
+  intro.
+  destruct (eq_dec.eq_dec ν v'). subst v'. apply H0. intro. inversion H2. congruence. inv H3.
+  congruence.
+
+  rewrite H1.
+  pose (subst_nonfv (subst_one ν x) (var_e v)).
+  rewrite e. reflexivity. 
+  intro v'. unfold subst_one. destruct (eq_dec.eq_dec ν v'). intro. subst v'. unfold nonfv. simpl.
+  unfold NFV. simpl. intro. destruct H3; congruence.
+  congruence.
+  decide equality.
+
+  repeat rewrite <- subst_locvar. simpl.
+  rewrite subst_locvar. reflexivity.
+  
+  repeat rewrite subst_fun.
+  rewrite IHe1.
+  rewrite IHe2. 
+ reflexivity.
+Qed.
+  
+Lemma boo :
+  forall  (s : subst_t D R) x p,
+    (subst s (var_e ν) = var_e ν) ->
+    (forall (x : expr), (nonfv x ν) -> nonfv (subst s x) ν) ->
+   sep_pred (subst_prop (subst_one ν (subst s x)) (subst_prop s p)) =
+   subst s (sep_pred (subst_prop (subst_one ν x) p)) .
+Proof.
+  intros.
+  rewrite <- sep_pred_subst.
+  f_equal.
+  simpl.
+  induction p.
+  + reflexivity.
+  + simpl.
+    repeat rewrite commuting_subst; easy.
+  + simpl. rewrite IHp. reflexivity.
+  + simpl. rewrite IHp1. rewrite IHp2. reflexivity.
+  + simpl. rewrite IHp1. rewrite IHp2. reflexivity.
+Qed.
+
+Lemma sep_ty_subst :
+  forall (s : subst_t D R) x b p,
+    (subst s (var_e ν) = var_e ν) ->
+    (forall (x : expr), nonfv x ν -> nonfv (subst s x) ν) ->
+    sep_ty (@subst _ _ _ Sub_Expr s x) (@subst _ _ _ Sub_Type s {ν : b | p}) = @subst _ _ _ Sub_Assrt s (sep_ty x {ν : b | p}).
+Proof.
+  intros.
+  rewrite subst_ty_base_pred.
+  unfold sep_ty.
+  simpl subst at 1.
+  unfold subst_r.
+  extensionality.
+  simpl reft_base.
+  rewrite sep_base_subst.
+  rewrite subst_andp.
+  rewrite subst_andp.
+  (* rewrite subst_wld. *)
+  (* rewrite subst_wld. *)
+  (* rewrite subst_wld. *)
+  f_equal.
+  f_equal.
+  cut (
+        sep_pred (subst (subst_one ν (subst s x)) (subst s p)) =
+        subst s (sep_pred (subst (subst_one ν x) p))
+  ). 
+  intro.
+  simpl reft_r.
+  rewrite H1. reflexivity.
+  pose (boo s x p).
+  simpl subst at 1.
+  simpl subst at 2. 
+  simpl subst at 3.
+  rewrite e; easy. 
+  extensionality. simpl. rewrite subst_wld. reflexivity.
+Qed.
+
+Lemma subst_prod :
+  forall s x y,
+    subst s (x, y) = (subst s x, subst s y).
+Proof.
+  reflexivity.
+Qed.
+
+Definition var_2_var (θ : subst_t D R) :=
+  forall x, var_e (subst θ x) = subst θ (var_e x).
+
+Lemma sep_env_subst :
+  forall (s : subst_t D R) xts,
+    var_2_var s ->
+    (subst s (var_e ν) = var_e ν) ->
+    (forall (x : expr), nonfv x ν -> nonfv (subst s x) ν) ->
+    sep_env (subst s xts) = subst s (sep_env xts).
+Proof.
+  intros.
+  induction xts as [| [x t]].
+  - rewrite subst_wld. reflexivity.
+  - setoid_rewrite subst_cons. 
+    unfold sep_env. fold sep_env.
+    setoid_rewrite subst_prod.
+    do 2 setoid_rewrite subst_andp.
+    f_equal. f_equal.
+    rewrite H.
+    destruct t as [b p].
+    rewrite <- sep_ty_subst.
+    reflexivity.
+    assumption.
+    assumption.
+    intuition.
+    rewrite subst_wld.
+    reflexivity.
+Qed.
+
+Lemma sep_guards_subst :
+  forall (s : subst_t D R) g,
+    sep_guards (subst s g) = subst s (sep_guards g).
+Proof.
+  intros.
+  induction g as [| φ ].
+  + rewrite subst_wld. reflexivity.
+  + setoid_rewrite subst_cons.
+    unfold sep_guards. fold sep_guards.
+    rewrite subst_andp.
+    rewrite subst_andp.
+    rewrite <- IHg.
+    f_equal. f_equal. rewrite sep_pred_subst. reflexivity. 
+    rewrite subst_wld. reflexivity.
+Qed.
+
+  Ltac push n := rewrite subst_prod at n.
+  
+  (* Lemma lift_fun : *)
+  (*   forall (P : mpred) w, *)
+  (*     ((fun (x : world) => P x) && emp)  *)
+  (*     ((fun (x : world) => P) && (@emp (world -> mpred) _ _)) w = fun (x : world) => (P && (@emp mpred _ _)). *)
+  (* Proof. *)
+  (*   firstorder. *)
+  (* Qed. *)
+  
+
+  Lemma sep_heap_bind_subst :
+    forall (s : subst_t D R) l xt,
+      var_2_var s ->
+      (subst s (var_e ν) = var_e ν) ->
+      (forall (x : expr), nonfv x ν -> nonfv (subst s x) ν) ->
+      sep_heap_bind (subst s l) (subst s xt) = subst s (sep_heap_bind l xt).
+  Proof.
+    intros s l [x t]. intros.
+    unfold sep_heap_bind.
+    rewrite subst_prod.
+    unfold snd. unfold fst.
+    rewrite subst_orp.
+    f_equal.
+    unfold eval_to.
+    rewrite subst_andp.
+    f_equal.
+    rewrite subst_wld.
+    extensionality w.
+    rewrite subst_locvar.
+    rewrite subst_eval.
+    reflexivity.
+    rewrite subst_wld. 
+    reflexivity.
+    rewrite H.
+    rewrite subst_sepcon.
+    f_equal.
+    rewrite subst_locvar.
+    unfold emapsto. 
+    rewrite subst_wld.
+    simpl. extensionality w. f_equal. extensionality addr. f_equal. extensionality v.
+    f_equal. f_equal.
+    unfold eval_to.
+    simpl.
+    rewrite subst_eval.
+    reflexivity.
+    unfold eval_to.
+    simpl andp. cbv beta.
+    f_equal.
+    f_equal.
+    rewrite subst_eval.
+    reflexivity.
+    destruct t as [b p].
+    rewrite <- sep_ty_subst.
+    reflexivity.
+    easy.
+    easy.
+  Qed.
+
+Ltac push_subst :=
+  (repeat (first [ rewrite subst_andp 
+                 | rewrite subst_orp 
+                 | rewrite subst_sepcon 
+                 | rewrite subst_imp
+                 ])).
+
+Definition eqk := @eq_key type_binding.
+
+Lemma thingie' :
+  forall (s : subst_t D R) (x y : loc * type_binding),
+    (forall (l m : loc), (subst s l) = (subst s m) -> l = m) ->
+    eqk (subst s x) (subst s y) -> eqk x y.
+Proof.
+  intros.
+  destruct x as [l xt].
+  destruct y as [m yt].
+  inv H0.
+  specialize (H l m).
+  unfold eqk.
+  apply H. easy.
+Qed.
+
+Lemma thingie :
+  forall (s : subst_t D R) (e : (loc * type_binding)) l,
+    (forall (l m : loc), (subst s l) = (subst s m) -> l = m) ->
+    InA eqk (subst s e) (subst s l) -> InA eqk e l.
+Proof.
+  intros.
+  induction l.
+  + inv H0.
+  + simpl subst at 2 in H0.
+    unfold subst_list in H0. fold subst_list in H0.
+    inv H0.
+    left.
+    apply (thingie' s). 
+    assumption.
+    apply H2.
+    right.
+    apply IHl.
+    assumption.
+Qed.
+
+Lemma transpose_sep_heap_bind :
+   transpose_neqkey Logic.eq
+     (λ (l : key) (xt : type_binding) (a : assert), sep_heap_bind l xt * a).
+Proof.
+  hnf. intros.
+  extensionality. rewrite sepcon_comm. rewrite sepcon_comm with (P := sep_heap_bind k e).
+  rewrite sepcon_assoc. reflexivity.
+Qed.
+
+Definition NonUnifyingSub (θ : subst_t D R) (h : heap_env) :=
+  (forall (l1 l2 : loc), l1 <> l2 -> subst θ l1 <> subst θ l2) /\
+  forall l x t,
+    MapsTo l (x, t) h <-> MapsTo (subst θ l) (subst θ x, subst θ t) (subst θ h).
+
+Lemma push_sep_heap_subst_1 : 
+  forall s h,
+       subst s (sep_heap h) 
+       = fold (fun l xt a => subst s (sep_heap_bind l xt) * a) h emp.
+Proof.
+  intros.
+  unfold sep_heap.
+  rewrite subst_wld.
+  extensionality w.
+  apply fold_rel with (R := fun (A B : assert) => A (subst s w) = B w).
+  reflexivity.
+  intros.
+  simpl. rewrite H0.
+  rewrite subst_wld. reflexivity.
+Qed.
+
+Lemma subst_heap_bindings :
+  forall s l (h : heap_env),
+    (forall (l1 l2 : loc), l1 <> l2 -> subst s l1 <> subst s l2) ->
+    ~ HE.In l (fold (add (elt := type_binding)) h heap_emp) -> ~ HE.In (subst s l) (subst s h).
+  simpl subst at 2.
+  unfold subst_heap.
+  intros until h. intro Hyp.
+  apply fold_rel with (R := fun A B => ~ HE.In l A -> ~ HE.In (subst s l) B); intros.
+  + intro. apply H. apply empty_in_iff in H0. intuition.
+  + simpl in *.
+    intro.
+    apply H1.
+    apply add_in_iff in H2.
+    apply add_in_iff.
+    destruct H2. 
+    left.
+    compare k l. tauto.
+    intro. apply Hyp in n. exfalso. apply n. apply H2. decide equality.
+    right.
+    apply H0 in H2. inv H2. 
+    intro. apply H1. apply add_in_iff. 
+    compare k l. tauto. intro. right. assumption.
+    decide equality.
+Qed.
+
+Lemma transpose_neqkey_add :
+  forall s, 
+    (forall (l1 l2 : loc), l1 <> l2 -> subst s l1 <> subst s l2) ->
+    transpose_neqkey Equal
+                     (λ (l0 : key) (xt0 : type_binding) (m0 : t type_binding),
+                      add (subst s l0) (subst s xt0) m0).
+Proof.
+  intros; hnf; intros.
+  simpl.
+  rewrite Equal_mapsto_iff. intros.
+  repeat rewrite add_mapsto_iff.
+  split. intros. decompose [and or] H1; clear H1.
+  right. split. rewrite <- H3. apply H. intuition. 
+  left. intuition.
+  left. intuition.
+  right. intuition.
+  intros. decompose [and or] H1; clear H1.
+  right. split. rewrite <- H3. apply H. intuition.
+  left. intuition.
+  left. intuition.
+  right. intuition.
+Qed.
+
+Lemma subst_heap_eq : 
+  forall s h h',
+    (∀ l1 l2 : loc, l1 ≠ l2 → subst s l1 ≠ subst s l2) ->
+    Equal h h' -> 
+    Equal (subst_heap s h) (subst_heap s h').
+Proof.
+  intros.
+  unfold subst_heap.
+  apply fold_Equal. apply Equal_ST.
+  solve_proper.
+  apply transpose_neqkey_add.
+  assumption.
+  assumption.
+Qed.
+
+Lemma subst_heap_add : forall s k e m,
+    (forall (l1 l2 : loc), l1 <> l2 -> subst s l1 <> subst s l2) ->
+       ¬HE.In (elt:=type_binding) k m ->
+       Equal (subst_heap s (add k e m)) (add (subst s k) (subst s e) (subst_heap s m)).
+Proof.
+  intros.
+  rewrite Equal_mapsto_iff.
+  intros l xt.
+  rewrite add_mapsto_iff.
+  split. intro.
+  unfold subst_heap in H1.
+  rewrite fold_add in H1.
+  rewrite add_mapsto_iff in H1. decompose [and or] H1; clear H1.
+  left. intuition. right.  intuition.
+  apply Equal_ST. solve_proper.
+  apply transpose_neqkey_add. apply H. assumption.
+  unfold subst_heap.
+  rewrite fold_add.
+  rewrite add_mapsto_iff. 
+  intros. decompose [and or] H1; clear H1.
+  left. intuition.
+  right. intuition.
+  apply Equal_ST.
+  solve_proper.
+  apply transpose_neqkey_add. apply H. 
+  assumption.
+Qed.
+
+Lemma subst_heap_add_step : 
+  forall k e h,
+    ~ HE.In k h ->
+    sep_heap (add k e h) = 
+    sep_heap_bind k e * sep_heap h.
+Proof.
+  intros.
+  unfold sep_heap.
+  rewrite fold_add. reflexivity. apply eq_equivalence. solve_proper. 
+  hnf. intros. simpl. extensionality. rewrite sepcon_comm. rewrite sepcon_comm with (P := sep_heap_bind k0 e0 x).
+  rewrite sepcon_assoc. normalize.
+  assumption.
+Qed.
+                             
+Lemma push_sep_heap_subst_2 :
+  forall s h,
+    NonUnifyingSub s h ->
+    sep_heap (subst s h) = fold (fun l xt a => (sep_heap_bind (subst s l) (subst s xt)) * a) h emp.
+Proof.
+  intros.
+  unfold sep_heap.
+  simpl subst at 1.
+  apply fold_rec_bis with (P := fun M A => 
+                                  fold (fun l xt a => sep_heap_bind l xt * a) (subst_heap s M) emp 
+                                  = A).
+  intros.
+  rewrite <- H1.
+  apply fold_Equal.
+  apply eq_equivalence. solve_proper. apply transpose_sep_heap_bind. apply subst_heap_eq. apply H.
+  symmetry. assumption.
+  compute. reflexivity.
+  intros.
+  assert (Equal (subst_heap s (add k e m')) (add (subst s k) (subst s e) (subst_heap s m'))).
+  apply subst_heap_add. apply H. apply H1.
+  assert (fold (fun l xt a => sep_heap_bind l xt * a) (subst_heap s (add k e m')) emp
+          = fold (fun l xt a => sep_heap_bind l xt * a) (add (subst s k) (subst s e) (subst_heap s m')) emp).
+  apply fold_Equal. apply eq_equivalence. solve_proper. apply transpose_sep_heap_bind. easy.
+  rewrite H4.
+  pose (@subst_heap_add_step (subst s k) (subst s e) (subst_heap s m')).
+  rewrite <- H2.
+  unfold sep_heap in e0.
+  rewrite e0.
+  reflexivity.
+  apply subst_heap_bindings.
+  apply H.
+  intro.
+  apply H1.
+  rewrite In_m. apply H5. reflexivity. symmetry. apply fold_identity.
+Qed.
+
+(* Lemma goo :  *)
+(*   forall (s : subst_t D R) h l xt, *)
+(*     (forall (l m : loc), (subst s l) = (subst s m) -> l = m) -> *)
+(*     (MapsTo l xt (fold (add (elt := type_binding)) h heap_emp) -> *)
+(*     MapsTo (subst s l) (subst s xt) (subst s h)). *)
+(* Proof. *)
+(*   intros until xt. intro OkSub. *)
+(*   simpl subst at 3. *)
+(*   unfold subst_heap. *)
+(*   apply fold_rel with  *)
+(*   (R := fun A B => MapsTo l xt A -> MapsTo (subst s l) (subst s xt) B). *)
+(*   + rewrite empty_mapsto_iff. intuition. *)
+(*   + repeat setoid_rewrite add_mapsto_iff. *)
+(*     intros. *)
+(*     destruct H1. destruct H1; subst. left. split; reflexivity. *)
+(*     right. destruct H1. split. *)
+(*     intro. apply OkSub in H3. congruence. auto. *)
+(* Qed. *)
+  
+Lemma sep_heap_subst :
+  forall (s : subst_t D R) h,
+      var_2_var s ->
+      (subst s (var_e ν) = var_e ν) ->
+      (forall (x : expr), nonfv x ν -> nonfv (subst s x) ν) ->
+      NonUnifyingSub s h ->
+    sep_heap (subst s h) = subst s (sep_heap h).
+Proof.
+    intros.
+    rewrite push_sep_heap_subst_1.
+    rewrite push_sep_heap_subst_2; try easy.
+    apply fold_rel. reflexivity.
+    intros. subst.
+    rewrite sep_heap_bind_subst; easy.
+Qed.
+
+End Subst.
+   
+Corollary sep_base_subst_var :
+  forall (s : subst_t var var) x b, subst s (sep_base x b) = sep_base (subst s x) (subst s b).
+Proof.
+  intros; exact (eq_sym (sep_base_subst s x b)).
+Qed.
+
+Corollary sep_base_subst_expr :
+  forall (s : subst_t var expr) x b, subst s (sep_base x b) = sep_base (subst s x) (subst s b).
+Proof.
+  intros; exact (eq_sym (sep_base_subst s x b)).
+Qed.
+
+Corollary sep_base_subst_loc :
+  forall (s : subst_t loc loc) x b, subst s (sep_base x b) = sep_base (subst s x) (subst s b).
+Proof.
+  intros; exact (eq_sym (sep_base_subst s x b)).
+Qed.
+
+Corollary sep_pred_subst_expr :
+  forall (θ : subst_t var expr) φ,
+    subst θ (sep_pred φ) = sep_pred (subst θ φ).
+Proof.
+  intros.
+  exact (eq_sym (sep_pred_subst θ φ)).
+Qed.
+
+Definition lift_var_subst (s : subst_t var var) :=
+  fun i => match s i with
+             | Some v => Some (var_e v)
+             | None => None
+           end.
+(** wf G (H1 * H2) (H1 * H2) 
+    x ∈ H2 ==> x ∉ H1
+    wf (H0 * H1) G ==> x ∉ H1
+    modvar x ==> x ∉ H0 **)
+  
