TranslationLemmas.v
@@ -38,12 +38,12 @@ Import ListNotations.
 (*   assumption. *)
 (* Qed. *)
 
-Lemma subst_emp_id :
-  forall s,
-    subst_pred s emp = emp.
-Proof.
-  normalize.
-Qed.
+(* Lemma subst_emp_id : *)
+(*   forall {A D R : Type} {s : subst_t A D R}, *)
+(*     subst s emp = emp. *)
+(* Proof. *)
+(*   normalize. *)
+(* Qed. *)
 
 Lemma combine_cons :
   forall A B (a:A) (b:B) xs ys,
@@ -73,7 +73,10 @@ Qed.
 (* Qed. *)
 
 Lemma subst_combine :
-  forall (A B D R : Type) (SA : Subst A D R) (SB : Subst B D R)
+  forall {A B D R : Type} {SA : Subst A D R} {SB : Subst B D R} 
+         {EA: Equivalence (@eq _ _ _ SA)}
+         {EB : Equivalence (@eq _ _ _ SB)}
+         {EB' : Equivalence (@eq _ _ _ (Subst_prod A B D R))}
          (xs : list A) (ys : list B) (θ : subst_t D R),
     length xs = length ys ->
     subst θ (combine xs ys) = combine (subst θ xs) (subst θ ys).
@@ -93,8 +96,7 @@ Proof.
     unfold subst at 1.
     unfold subst_list at 1.
     fold subst_list.
-    unfold subst at 1.
-    unfold Subst_prod at 1. unfold subst_prod.
+    simpl subst at 1. unfold Subst.subst_prod.
     inversion H.
     specialize (IHxs ys θ H1).
     unfold subst at 2 3 in IHxs. unfold Subst_list in IHxs.
@@ -102,36 +104,33 @@ Proof.
     reflexivity.
 Qed.
 
-Hint Resolve subst_emp_id : subst.
+(* Hint Resolve subst_emp_id : subst. *)
 
 Lemma vv_not_fv :
   forall G Gr H e T,
-    wf_env H G -> expr_type G H Gr e T -> ~ FV e ν.
+    wf_env H G -> expr_type G H Gr e T -> NFV e ν.
 Proof.
   intros.
   induction H1; eauto with datatypes.
+  + unfold NFV. intro. inv H.
+  + unfold NFV. intro. inv H.
   + induction Γ.
     contradiction H.
     apply in_inv in H.
     destruct a as [x' [b' p']].
     destruct H. inversion H. subst.
     inversion H0. subst.
-    unfold FV.
+    unfold NFV.
     unfold fv_expr.
     intro.
-    inversion H1. subst x. apply H5. reflexivity. contradiction.
-    apply IHΓ. inversion H0. assumption. assumption.
+    inversion H1. subst.  unfold fresh in H5. destruct H5. apply H2. reflexivity. inv H2.
+    apply IHΓ. inv H0. assumption. assumption.
 Qed.
 
 Lemma fresh_var_cons :
   forall G H xt x, fresh x (xt :: G) H -> fresh x G H.
 Proof. 
   firstorder. 
-  unfold var_not_in in *.
-  rewrite Forall_forall in *.
-  intros.
-  apply H1.
-  eauto with datatypes.
 Qed.
 
 Lemma bind_not_in_cons :
@@ -162,26 +161,44 @@ Proof.
   apply H1.
 Qed.
 
-Lemma fresh_var_cons_hp :
-  forall G H l xt x, ~ In l H -> fresh x G (add l xt H) -> fresh x G H.
-Proof.
-  intros.
-  unfold fresh in *.
-  decompose [and] H1.
-  repeat split; try assumption.
-  eapply bind_not_in_cons; eauto.
-Qed.
+(* Lemma fresh_var_cons_hp : *)
+(*   forall G H l xt x, nonfv x H -> fresh x G (add l xt H) -> fresh x G H. *)
+(* Proof. *)
+(*   intros. *)
+(*   unfold fresh in *. *)
+(*   decompose [and] H1. clear H1. *)
+(*   repeat split. assumption. assumption. *)
+(*   repeat split; try assumption. *)
+(*   eapply bind_not_in_cons; eauto. *)
+(* Qed. *)
   
 Lemma fresh_var_nonmem_env :
-  forall G H x, fresh x G H -> var_not_in x G.
+  forall G H (x : var), fresh x G H -> var_not_in x G.
 Proof.
-  firstorder.
+  unfold fresh. unfold var_not_in.
+  intros.
+  rewrite Forall_forall.
+  intros.
+  decompose [and] H0. clear H0.
+  destruct x0. simpl.
+  unfold nonfv in H4. simpl in *.
+  induction G as [| [x' t']].
+  + inv H1.
+  + inv H1. inv H0. inv H4. apply H0.
+    apply IHG. assumption. inv H4. assumption.
 Qed.
 
 Lemma fresh_var_nonmem_heap :
   forall G H x, fresh x G H -> bind_not_in x H.
 Proof.
-  firstorder.
+  unfold fresh. unfold bind_not_in.
+  intros.
+  decompose [and] H0. clear H0. unfold nonfv in *; simpl in *.
+  unfold nonfv_heap in H4.
+  specialize (H4 l (x, t0)).
+  intro.
+  rewrite <- HE_Props.F.find_mapsto_iff in H0.
+  apply H4 in H0. destruct H0. apply H2. reflexivity.
 Qed.
 
 Lemma var_not_in_not_eq :
@@ -210,13 +227,31 @@ Proof.
 Qed.
 
 Lemma var_not_in_and_in :
-  forall G x, var_not_in x G -> ~ (var_in x G).
+  forall G x, var_not_in x G <-> ~ (var_in x G).
 Proof.
   unfold var_not_in.
   unfold var_in.
   intros.
   rewrite Forall_forall in *.
   firstorder.
+  destruct x0.
+  intro.
+  apply (H r).
+  inv H1. apply H0.
+Qed.
+
+Lemma fresh_var_not_in :
+  forall G H x, fresh x G H -> ~ (var_in x G).
+Proof.
+  intros.
+  induction G as [| [x' t']].
+  + intro. inv H1. intuition.
+  + intro. inv H1. inv H2. inv H1.
+    apply H0. reflexivity.
+    inv H0. unfold nonfv in H3. simpl in *.
+    decompose [and] H3.
+    apply IHG. constructor. assumption.
+    constructor. assumption. assumption. exists x0. assumption.
 Qed.
 
 Lemma bind_not_in_and_in :
@@ -246,94 +281,101 @@ Hint Resolve
      bind_not_in_and_in
      bind_in_and_not_in_eq
      fresh_var_cons
-     fresh_var_cons_hp
+     fresh_var_not_in
+     (* fresh_var_cons_hp *)
      vv_not_fv
 : var.
 
-Lemma subst_dist_sepcon :
-  forall P Q (s : var -> expr),
-    subst_pred s (P * Q) = subst_pred s P * subst_pred s Q.
-Proof.
-  firstorder.
-Qed.
+(* Lemma subst_dist_sepcon_loc : *)
+(*   forall P Q (s : loc -> loc), *)
+(*     subst_pred_loc s (P * Q) = subst_pred_loc s P * subst_pred_loc s Q. *)
+(* Proof. *)
+(*   firstorder. *)
+(* Qed. *)
 
-Lemma subst_dist_andp :
-  forall P Q (s : var -> expr),
-    subst_pred s (P && Q) = subst_pred s P && subst_pred s Q.
-Proof.
-  firstorder.
-Qed.
+(* Lemma subst_dist_sepcon : *)
+(*   forall P Q (s : var -> expr), *)
+(*     subst_pred s (P * Q) = subst_pred s P * subst_pred s Q. *)
+(* Proof. *)
+(*   firstorder. *)
+(* Qed. *)
 
-Lemma subst_dist_andp_loc :
-  forall P Q (s : loc -> loc),
-    subst_pred_loc s (P && Q) = subst_pred_loc s P && subst_pred_loc s Q.
-Proof.
-  firstorder.
-Qed.
+(* Lemma subst_dist_andp : *)
+(*   forall P Q (s : var -> expr), *)
+(*     subst_pred s (P && Q) = subst_pred s P && subst_pred s Q. *)
+(* Proof. *)
+(*   firstorder. *)
+(* Qed. *)
 
-Lemma subst_dist_sepcon_loc :
-  forall P Q (s : loc -> loc),
-    subst_pred_loc s (P * Q) = subst_pred_loc s P * subst_pred_loc s Q.
-Proof.
-  firstorder.
-Qed.
+(* Lemma subst_dist_andp_loc : *)
+(*   forall P Q (s : loc -> loc), *)
+(*     subst_pred_loc s (P && Q) = subst_pred_loc s P && subst_pred_loc s Q. *)
+(* Proof. *)
+(*   firstorder. *)
+(* Qed. *)
 
-Lemma subst_dist_orp :
-  forall P Q (s : var -> expr),
-    subst_pred s (P || Q) = subst_pred s P || subst_pred s Q.
-Proof.
-  firstorder.
-Qed.
+(* Lemma subst_dist_sepcon_loc : *)
+(*   forall P Q (s : loc -> loc), *)
+(*     subst_pred_loc s (P * Q) = subst_pred_loc s P * subst_pred_loc s Q. *)
+(* Proof. *)
+(*   firstorder. *)
+(* Qed. *)
 
-Lemma subst_dist_imp :
-  forall P Q (s : var -> expr),
-    subst_pred s (P --> Q) = subst_pred s P --> subst_pred s Q.
-Proof.
-  firstorder.
-Qed.
+(* Lemma subst_dist_orp : *)
+(*   forall P Q (s : var -> expr), *)
+(*     subst_pred s (P || Q) = subst_pred s P || subst_pred s Q. *)
+(* Proof. *)
+(*   firstorder. *)
+(* Qed. *)
 
-Lemma subst_cons :
-  forall { A D R : Type } { S : Subst A D R }
-         s h t,
-    subst s (h :: t) = subst s h :: subst s t.
-Proof. firstorder. Qed.
-
-Ltac push_subst :=
-  (repeat (first [ rewrite subst_dist_andp 
-                 | rewrite subst_dist_andp_loc
-                 | rewrite subst_dist_sepcon_loc
-                 | rewrite subst_dist_orp 
-                 | rewrite subst_cons
-                 | rewrite subst_dist_sepcon ])).
-
+(* Lemma subst_dist_imp : *)
+(*   forall P Q (s : var -> expr), *)
+(*     subst_pred s (P --> Q) = subst_pred s P --> subst_pred s Q. *)
+(* Proof. *)
+(*   firstorder. *)
+(* Qed. *)
 Lemma fresh_var_expr_fv :
   forall G H e x, 
-    fresh x G H -> wf_expr G H e -> FV e x -> False.
+    fresh x G H -> wf_expr G H e -> nonfv e x.
 Proof.
   induction e.
   + firstorder.
   + firstorder.
-    inversion H1; subst.
-    inversion H1; subst. 
-      eapply var_not_in_and_in; eauto.
-      apply bind_not_in_and_in in H4. congruence.
-      congruence.
-      apply bind_not_in_and_in in H4. congruence.
-      congruence.
-  + firstorder.
-  + intro x.
-    unfold FV in *.
-    intros.
-    simpl in *.
-    apply in_app_or in H2.
-    inversion H1; subst.
-    destruct H2.
-    eapply IHe1; eauto.
-    eapply IHe2; eauto.
+    inv H1;
+    unfold nonfv; simpl; intro; simpl in H1; destruct H1; intuition; subst x.
+    * apply var_not_in_and_in in H7. contradiction.
+      rewrite var_not_in_and_in. eapply fresh_var_not_in. unfold fresh. 
+      split. easy. split. easy. eauto.
+    * apply bind_not_in_and_in in H7. contradiction.
+      eapply fresh_var_nonmem_heap. unfold fresh; eauto.
+  + easy.
+  + intros.
+    unfold fresh in *.
+    inv H1.
+    simpl.
+    unfold NFV. intro. simpl in H1. apply in_app_or in H1.
+    destruct H1. 
+    simpl in *. 
+    apply (IHe1 x); easy.
+    apply (IHe2 x); easy.
+Qed.
+
+Lemma fresh_var_pred_fv :
+  forall G H p x,
+    fresh x G H -> wf_prop G H p -> nonfv p x.
+Proof.
+  intros.
+  induction p; try easy; match goal with 
+                           | H : wf_prop _ _ _ |- _ => inv H end.
+  + split; eauto using fresh_var_expr_fv.
+  + intuition.
+  + simpl. intuition.
+  + simpl. intuition.
 Qed.
 
 Hint Transparent stk hp runloc fst snd.
 
+(** 
 Lemma nonfree_var_expr_eval :
   forall e e' x,
     (FV e x -> False) ->
@@ -357,59 +399,155 @@ Proof.
     intro. apply H. simpl. apply in_or_app. right. assumption.
     intro. apply H. simpl. apply in_or_app. left. assumption.
 Qed.
+**)
+
+Lemma nonfree_var_expr_eval :
+  forall G H e e' x,
+    fresh x G H ->
+    wf_expr G H e ->
+    forall w,
+   eval w e = eval (λ i : var, if eq_dec x i then e' else stk w i, runloc w, hp w) e.
+Proof.
+  induction e; intros.
+  * reflexivity.
+    * pose (fresh_var_expr_fv G H (var_e v)).
+      simpl in n. unfold NFV in n. simpl in n.
+      simpl. unfold stk. simpl.
+      destruct (eq_dec x v).
+      destruct (n x). assumption. assumption. left. congruence. reflexivity.
+    * reflexivity.
+    * simpl. erewrite IHe1. erewrite IHe2. reflexivity. 
+      assumption. inv H1; assumption.
+      assumption. inv H1; assumption.
+Qed.
+
+Lemma nonfv_not_r :
+  forall p (x : var),
+    nonfv (sep_pred p) x -> nonfv (sep_pred (not_r p)) x.
+Proof.
+  intros.
+  simpl.
+  unfold nonfv_assert.
+  intros;
+  specialize (H w v).
+  f_equal; f_equal; apply H.
+Qed.
+
+Lemma nonfv_and_r :
+  forall p1 p2 (x : var),
+    nonfv (sep_pred p1) x -> nonfv (sep_pred p2) x -> nonfv (sep_pred (and_r p1 p2)) x.
+Proof.
+  intros.
+  simpl.
+  unfold nonfv_assert.
+  intros;
+  specialize (H w v);
+  specialize (H0 w v).
+  do 2 f_equal. apply H.  apply H0.
+Qed.
+
+Lemma nonfv_or_r :
+  forall p1 p2 (x : var),
+    nonfv (sep_pred p1) x -> nonfv (sep_pred p2) x -> nonfv (sep_pred (or_r p1 p2)) x.
+Proof.
+  intros.
+  simpl.
+  unfold nonfv_assert.
+  intros;
+  specialize (H w v);
+  specialize (H0 w v).
+  do 2 f_equal. apply H.  apply H0.
+Qed.
 
 Lemma fresh_var_nonfree_pred :
   forall G H p x,
-    fresh x G H -> wf_prop G H p -> nonfreevars (sep_pred p) x.
+    fresh x G H -> wf_prop G H p -> nonfv (sep_pred p) x.
 Proof.
   intros.
-  induction p.
-  + firstorder.
-  + inversion H1; subst.
-    unfold nonfreevars.
-    intro e'.
-    unfold subst_pred.
-    simpl. extensionality w.
-    f_equal.
-    f_equal.
-    repeat rewrite nonfree_var_expr_eval.
-    reflexivity.
-    eauto using fresh_var_expr_fv.
-    eauto using fresh_var_expr_fv.
-  + unfold sep_pred; fold sep_pred.
-    unfold nonfreevars in *.
-    intro e.
-    rewrite subst_dist_andp.
-    rewrite subst_dist_imp.
-    f_equal.
-    rewrite <- IHp with (v := e).
-    apply  pred_ext.
-    apply derives_refl.
-    apply derives_refl.
-    inversion H1; auto.
-  + unfold sep_pred; fold sep_pred.
-    unfold nonfreevars in *.
-    intro e.
-    inversion H1.
-    repeat rewrite subst_dist_andp.
-    repeat f_equal.
-    auto.
-    auto.
-  + unfold sep_pred; fold sep_pred.
-    unfold nonfreevars in *.
-    intro e.
-    inversion H1.
-    repeat rewrite subst_dist_andp.
-    repeat rewrite subst_dist_orp.
-    repeat f_equal.
-    auto.
-    auto.
+  apply SubstProp_var. 
+  induction p; try easy.
+  inv H1. split; eauto using fresh_var_expr_fv.
+  simpl. apply IHp. inv H1; easy.
+  simpl. inv H1. split; intuition.
+  simpl. inv H1. split; intuition.
 Qed.
 
+Lemma wf_expr_nonfree_locs :
+  forall G H e, 
+    wf_expr G H e -> (forall (l : loc), nonfv e l).
+Proof.
+  intros.
+  induction e; try easy.
+  inv H0.
+  simpl.
+  unfold NFL.
+  simpl.
+  intro.
+  apply in_app_or in H0. intuition.
+Qed.
+
+Lemma wf_prop_nonfree_locs :
+  forall G H p,
+    wf_prop G H p -> (forall (l : loc), nonfv p l).
+Proof.
+  intros. simpl. unfold nonfv_prop.
+  induction H0; eauto using wf_expr_nonfree_locs. 
+Qed.
+
+Lemma wf_type_nonfree_locs :
+  forall G H t,
+    wf_type G H t -> (forall (l : loc), nonfv (reft_r t) l).
+Proof.
+  intros.
+  inv H0.
+  eauto using wf_prop_nonfree_locs.
+Qed.
+
+Hint Resolve wf_expr_nonfree_locs wf_prop_nonfree_locs wf_type_nonfree_locs : wf.
+
+Lemma wf_heap_nonfree_locs :
+  forall G H,
+    wf_heap G H H ->
+    (forall l x t, MapsTo l (x,t) H -> (forall (l : loc), nonfv (reft_r t) l)).
+Proof.
+  intros.
+  induction H0.
+  assert (elements Σ' = []).
+  apply HE_Props.elements_Empty; assumption.
+  rewrite HE_Props.F.elements_mapsto_iff with (elt := type_binding) in H1.
+  rewrite H2 in H1.
+  inv H1.
+  + (* compare l l0; intros. *)
+    unfold HE_Props.Add in *.
+    specialize (H6 l).
+    rewrite HE_Props.F.find_mapsto_iff in *.
+    rewrite H6 in *.
+    rewrite <- HE_Props.F.find_mapsto_iff in H1.
+    apply HE_Props.F.add_mapsto_iff in H1. 
+    destruct H1. 
+    inv H1. inv H8. eauto with wf.
+    apply IHwf_heap. destruct H1. 
+    apply HE_Props.F.find_mapsto_iff.
+    apply H7.
+Qed.
+
+Lemma wf_ctx_nonfree_locs :
+  forall G H,
+    wf_env H G -> 
+    Forall (fun xt => (forall (l : loc), nonfv (reft_r (snd xt)) l)) G.
+Proof.
+  intros.
+  rewrite Forall_forall.
+  induction H0; intros.
+  + inversion H.
+  + inv H2;
+    eauto with wf.
+Qed.
+
+Hint Resolve wf_ctx_nonfree_locs wf_heap_nonfree_locs : wf.
 Hint Resolve fresh_var_nonfree_pred : wf var.
 Hint Rewrite fresh_var_nonfree_pred : wf.
 Hint Constructors wf_expr wf_prop wf_type wf_env wf_heap : wf.
-
 
 Lemma wf_expr_cons :
   forall G H xt e,
@@ -479,13 +617,7 @@ Qed.
 
 Hint Resolve wf_prop_from_ty : wf.
 
-Ltac split_subst_var :=
-  match goal with 
-    | |- appcontext[_ (subst_one ?x _) (var_e ?v)] =>
-      unfold subst; unfold subst_one; simpl;
-      destruct (eq_dec v x); subst
-  end.
-
+(**
 Lemma subst_expr_fun :
   forall (s : var -> expr) f e1 e2,
     subst s (fun_e f e1 e2) = fun_e f (subst s e1) (subst s e2).
@@ -513,6 +645,7 @@ Lemma subst_prop_or :
     subst s (or_r p1 p2) = or_r (subst s p1) (subst s p2).
 Proof. firstorder. Qed.
 
+**)
 Lemma wf_prop_not :
   forall G H p, wf_prop G H p -> wf_prop G H (not_r p).
 Proof. firstorder. Qed.
@@ -527,13 +660,20 @@ Lemma wf_prop_or :
     wf_prop G H p1 -> wf_prop G H p2 -> wf_prop G H (or_r p1 p2).
 Proof. firstorder. Qed.
 
-Hint Rewrite 
-     subst_prop_rel subst_expr_fun subst_prop_and subst_prop_or subst_prop_not 
-: wf.
+(* Hint Rewrite  *)
+(*      subst_prop_rel subst_expr_fun subst_prop_and subst_prop_or subst_prop_not  *)
+(* : wf. *)
 Hint Resolve 
-     subst_prop_rel subst_expr_fun subst_prop_and subst_prop_or subst_prop_not 
+     (* subst_prop_rel subst_expr_fun subst_prop_and subst_prop_or subst_prop_not  *)
      wf_prop_and wf_prop_or wf_prop_not 
 : wf.
+
+Ltac split_subst_var :=
+  match goal with 
+    | |- appcontext[_ (subst_one ?x _) (var_e ?v)] =>
+      unfold subst; unfold subst_one; simpl;
+      destruct (eq_dec x v); subst
+  end.
 
 Lemma wf_subst_vv_expr :
   forall G H e e',
@@ -543,9 +683,9 @@ Proof.
   intros.
   induction e.
   + eauto with wf.
-  + inversion H0; split_subst_var; eauto with wf.
+  + inv H0; split_subst_var; eauto with wf.
   + inversion H0.
-  + inversion H0; rewrite subst_expr_fun; eauto with wf.
+  + inversion H0; rewrite subst_fun; eauto with wf.
 Qed.
 
 Lemma wf_expr_mem :
@@ -579,7 +719,7 @@ Lemma wf_subst_vv_pred :
     wf_prop G H (subst (subst_one ν e) p).
 Proof.
   intros.
-  induction p; inversion H1; autorewrite with wf; eauto with wf.
+  induction p; inv H1; rw_subst_reft; eauto with wf.
 Qed.
   
 Hint Resolve wf_subst_vv_pred : wf.
@@ -589,241 +729,45 @@ Lemma fresh_var_nonfree_ty :
     x <> v ->
     fresh v G H -> 
     var_in x G \/ bind_in x H -> 
-    wf_type G H t -> nonfreevars (sep_ty (var_e x) t) v.
+    wf_type G H t -> nonfv (sep_ty (var_e x) t) v.
 Proof.
+  Hint Transparent NFV.
   intros.
-  unfold nonfreevars.
-  intro e.
-  unfold sep_ty. 
-  destruct t0 as [ b p ].
-  push_subst.
-  f_equal.
-  f_equal.
-  + unfold sep_base.
-    destruct b;
-      push_subst; repeat (extensionality; f_equal); 
-      unfold eval_to, subst_one, subst_pred; simpl; unfold stk; simpl;
-      destruct (eq_dec x v); try first [contradiction | reflexivity ].
-  + erewrite <- fresh_var_nonfree_pred. reflexivity. eauto with wf. apply wf_subst_vv_pred; eauto with wf var.
-    match goal with 
-      | H: (var_in _ _  \/ bind_in _ _) |- _ =>
-        destruct H; eauto with wf
-    end.
+  apply SubstTy_var.
+  simpl. 
+  firstorder.
+  simpl.
+  unfold nonfv_reft_t.
+  split. destruct (reft_base t0); easy. 
+  inv H3.
+  eapply fresh_var_pred_fv; eauto.
 Qed.
 
 Lemma var_nonmem_free_ctx :
-  forall G H x, fresh x G H -> wf_env H G -> nonfreevars (sep_env G) x.
+  forall G H x, fresh x G H -> wf_env H G -> nonfv (sep_env G) x.
 Proof.
   intros G H x fr wf.
   induction G as [| (x',t')].
-  + unfold nonfreevars. normalize.
+  + unfold nonfv. simpl. unfold nonfv_assert. normalize.
   + destruct t' as [b p]. 
     assert (x' <> x).
       apply var_not_in_not_eq with (G := G) (t := { ν : b | p }). 
-      apply fr.
-    unfold nonfreevars in *. 
-    intros.
-    unfold sep_env; fold sep_env.
-    repeat rewrite subst_dist_andp.
-    f_equal.
-    f_equal.
-    unfold sep_ty. 
-    repeat rewrite subst_dist_andp.
-    repeat f_equal.
-    unfold sep_base, subst_pred, subst_one.
-    destruct b; unfold eval_to; simpl; repeat (f_equal; extensionality);
-    unfold stk; simpl;
-      try match goal with
-          | |- appcontext[eq_dec ?x ?y] => destruct (eq_dec x y); (contradiction || reflexivity)
-          end.
-    inversion wf. subst.
-    inversion H7. subst.
-    rewrite <- fresh_var_nonfree_pred. reflexivity.
-    eauto.
-    apply wf_subst_vv_pred. 
-    constructor. exists ({ ν : b | p }). left. reflexivity. (* Should automate this *)
-    assumption.
-    apply IHG; inversion wf; eauto with var wf.
+      eauto with var.
+    unfold sep_env. fold sep_env.
+    apply nonfv_andp. split.
+    apply nonfv_andp. split.
+    eapply fresh_var_nonfree_ty; eauto.
+    left. unfold var_in. exists { ν : b | p}. left. reflexivity.
+    inv wf. easy.
+    apply IHG. eauto with var. inv wf. easy. easy.
 Qed.
-
-(* 
-Lemma wf_heap_loc_fresh :
-  forall G H l x t,
-    wf_heap G (add l (x, t) H) (add l (x, t) H) ->
-    fresh_loc l G H.
-Proof.
-  intros.
-  inv H0.
-  rewrite (@HE_Props.elements_Empty (var * reft_type)) in H1.
-  pose (HE_Props.F.elements_mapsto_iff (add l (x, t0) H) l (x, t0)).
-  destruct i. 
-  rewrite H1 in H0.
-  assert (MapsTo l (x, t0) (add l (x, t0) H)).
-  apply HE_Props.F.find_mapsto_iff.
-  rewrite HE_Props.F.add_eq_o. reflexivity. reflexivity.
-  apply H0 in H3.
-  inv H3.
-  constructor.
-
-  pose (@HE_Props.F.empty_o type_binding l).
-  pose (@find (type_binding) l (HE.empty type_binding) = @find type_binding l (add l (x, t0) H)).
-  Set Printing All. idtac.
-  rewrite e in P.
-  unfold fresh_loc in *.
-  apply H8.
-Qed.
-
-Lemma wf_heap_fresh_trans :
-  forall G H H' x,
-    wf_heap G H H' -> fresh x G H -> fresh x G H'.
-Proof.
-  intros until x.
-  induction H' as [| [l [x' t']]].
-  + firstorder. unfold bind_not_in. eauto with datatypes.
-  + intros.
-    inv H0.
-    destruct (IHH' H12).
-    auto.
-    unfold fresh.
-    destruct H2.
-    repeat (split; try assumption). 
-    assert (x' <> x).
-      eauto with wf var.
-    unfold bind_not_in.
-    eauto with wf var.
-Qed.
-
-Hint Resolve wf_heap_loc_fresh : var wf.
-*)
 
 Lemma sep_heap_emp :
   sep_heap (empty type_binding) = emp.
 Proof.
   reflexivity.
 Qed.
-(*
-Lemma MapsTo_sepheap :
-  forall H l xt,
-    InA (eq_key_elt (elt := type_binding)) (l,xt) H -> 
-    exists H1 H2,
-      (H = H1 ++ (l, xt) :: H2)
-      /\ (sep_heap' H |-- sep_heap' H1 * sep_heap_bind l xt * sep_heap' H2).
-Proof.
-  intros.
-  induction H as [| [l' xt']]. 
-    * inversion H0.
-    * destruct (InA_split H0) as [H' [[l'' xt''] [H'']]]. 
-      destruct H1. inv H1. simpl in H3. simpl in H4. subst.
-      inv H0.
-      inv H3. simpl in H0. simpl in H1. subst.
-      exists []. exists H.
-      split. reflexivity.
-      unfold sep_heap'; fold sep_heap'.
-      rewrite sepcon_assoc.
-      rewrite sepcon_comm with (P := emp).
-      rewrite sepcon_emp.
-      apply derives_refl.
-      apply IHlist in H3.
-      destruct H3 as [H1'].
-      destruct H0 as [H1''].
-      destruct H0.
-      exists ((l',xt') :: H1'). exists H1''.
-      split. 
-      simpl.
-      rewrite H0. reflexivity.
-      unfold sep_heap'; fold sep_heap'.
-      rewrite sepcon_comm with (Q := sep_heap' H1').
-      rewrite sepcon_comm with (Q := sep_heap_bind l'' xt'').
-      rewrite sepcon_assoc.
-      rewrite sepcon_comm with (Q := sep_heap' H1'').
-      rewrite <- sepcon_assoc.
-      rewrite <- sepcon_assoc.
-      rewrite sepcon_comm with (Q := sep_heap' H).
-      apply sepcon_derives.
-      rewrite sepcon_comm.
-      rewrite <- sepcon_assoc.
-      apply H1.
-      apply derives_refl.
-Qed.
 
-Lemma sep_heap_app :
-  forall H1 H2,
-    sep_heap' (H1 ++ H2) = sep_heap' H1 * sep_heap' H2.
-Proof.
-  induction H1 as [| [l xt]]; intros.
-  rewrite app_nil_l.
-  apply pred_ext.
-  rewrite <- sepcon_emp at 1. rewrite sepcon_comm.
-  apply derives_refl. 
-  rewrite <- sepcon_emp. rewrite sepcon_comm.
-  apply derives_refl.
-  rewrite <- app_comm_cons.
-  unfold sep_heap'; fold sep_heap'.
-  rewrite IHlist.
-  rewrite sepcon_assoc.
-  reflexivity.
-Qed.
-*)
-
-Definition eqA := eq_key_elt (elt := type_binding).
-
-(*
-Lemma In_app_sub :
-  forall p p' H H' H'',
-    (InA eqA p (p' :: H) ↔ InA eqA p (H' ++ p' :: H''))
-    ->
-    (eqA p p' \/ (InA eqA p H ↔ InA eqA p (H' ++ H''))).
-Proof.
-  intros until p'.
-  destruct (eq_dec p p').
-  subst. left. reflexivity.
-  intro H.
-  induction H; intros. 
-  right.
-  destruct H.
-  constructor; intro. 
-   * inv H1.
-   * apply InA_app in H1.
-     destruct H1.
-     cut (InA eqA p (H' ++ p' :: H'')).
-     intro. apply H0 in H2. inv H2. inv H4. destruct p. destruct p'. simpl in H2, H3. subst.
-     congruence. assumption.
-     apply InA_app_iff.
-     apply HE_Props.eqke_equiv.
-       left. apply H1.
-     cut (InA eqA p (H' ++ p' :: H'')).
-     intro. apply H0 in H2. inv H2. inv H4. destruct p. destruct p'. simpl in H2, H3. subst.
-     congruence. assumption.
-     apply InA_app_iff.
-       apply HE_Props.eqke_equiv.
-       right.
-       apply InA_cons. right. assumption.
-       apply HE_Props.eqke_equiv.
-  * destruct H0.
-    destruct (eq_dec p p').
-    left. inv e. reflexivity.
-    right.
-    constructor; intro.
-    + cut (InA eqA p (p' :: a :: H)).
-      intro.
-      apply H0 in H3.
-      apply InA_app_iff. apply HE_Props.eqke_equiv.
-      apply InA_app in H3.
-      destruct H3. left. assumption.
-      inv H3. inv H5. destruct p. destruct p'. simpl in *. subst. congruence.
-      right. assumption. apply HE_Props.eqke_equiv.
-      apply InA_cons. right. assumption.
-    + cut (InA eqA p (H' ++ p' :: H'')).
-      intro IN.
-      apply H1 in IN. inv IN.
-      inv H4. destruct p; destruct p'; simpl in *; subst; congruence.
-      assumption.
-      apply InA_app_iff. apply HE_Props.eqke_equiv.
-      apply InA_app in H2.
-      destruct H2. left. assumption. right. apply InA_cons. right. assumption.
-      apply HE_Props.eqke_equiv.
-Qed.
-*)
 
 Lemma EqMapsTo :
   forall H H',
@@ -832,7 +776,7 @@ Proof.
   unfold sep_heap.
   intros.
   apply HE_Props.fold_Equal.
-  apply EQ_EQUIVALENCE.
+  apply eq_equivalence.
   repeat (hnf; intros; subst).
   reflexivity.
   hnf.
@@ -863,7 +807,7 @@ Proof.
   unfold sep_heap.
   set (f := fun l xt a => sep_heap_bind l xt * a).
   assert (eq (fold f (add l xt H) emp) (f l xt (fold f H emp))).
-  apply HE_Props.fold_add. apply EQ_EQUIVALENCE.
+  apply HE_Props.fold_add. apply eq_equivalence.
   solve_proper.
   repeat (hnf; intros; subst). unfold f.
   rewrite sepcon_comm. rewrite sepcon_assoc. rewrite sepcon_comm with (P := a).
@@ -876,65 +820,136 @@ Lemma sep_heap_Emp :
   forall H, Empty H -> sep_heap H = emp.
 Proof.
   intros.
-  unfold sep_heap. rewrite HE_Props.fold_Empty. reflexivity. apply EQ_EQUIVALENCE.
+  unfold sep_heap. rewrite HE_Props.fold_Empty. reflexivity. apply eq_equivalence.
   assumption.
 Qed.
 
 Lemma fresh_loc_not_In :
-  forall l G H, fresh_loc l G H -> ~ In l H.
+  forall l G H, fresh_loc l G H -> nonfv H l.
+Proof.
+  firstorder.
+Qed.
+
+Lemma fv_var_sep_heap_bind :
+  forall k e (x : var),
+  @nonfv loc var var _ k x -> 
+  @nonfv type_binding var var _ e x ->
+   @nonfv assert var var _  (sep_heap_bind k e) x.
+Proof.
+  intros. destruct e.
+  unfold sep_heap_bind.
+  apply nonfv_orp. split.
+  unfold eval_to. unfold eval. 
+  simpl. unfold nonfv_assert. simpl. intros.
+  f_equal.
+  apply nonfv_sepcon. split.
+  unfold emapsto. simpl. unfold nonfv_assert. intros.
+  f_equalize. f_equal. extensionality. f_equalize.
+  unfold eval_to. simpl. f_equalize. f_equal. f_equal.
+  unfold subst_one. unfold stk. simpl. destruct (eq_dec x v). 
+  subst x. inv H0. simpl in *. congruence. reflexivity.
+  apply SubstTy_var. inv H0. unfold nonfv in H1. simpl in *.
+  intro. simpl in *. intuition.
+  inv H0. 
+  simpl in *. unfold nonfv_reft_t in *.
+  destruct H2. split.
+  assumption. 
+  induction (reft_r r); simpl in *; intuition.
+Qed.
+
+Lemma fv_var_sep_heap :
+  forall (H : heap_env) (x : var), nonfv H x -> nonfv (sep_heap H) x.
 Proof.
   intros.
-  unfold fresh_loc in *.
-  decompose [and] H0.
-  apply HE_Props.F.not_find_in_iff.
-  apply H0.
+  unfold sep_heap.
+  apply HE_Props.fold_rec_bis.
+  intros. assumption. easy.
+  intros. apply nonfv_sepcon. constructor.
+  unfold nonfv in H0. simpl in H0.
+  unfold nonfv_heap in H0. specialize (H0 k e). apply H0 in H1.
+  apply fv_var_sep_heap_bind; easy.
+  easy.
 Qed.
 
 Lemma var_nonmem_free_heap :
-  forall G H H' x, fresh x G H -> wf_heap G H H' -> nonfreevars (sep_heap H') x.
+  forall G H x, fresh x G H -> wf_heap G H H -> nonfv (sep_heap H) x.
 Proof.
   intros.
-  induction H1.
-  + unfold nonfreevars. intro e.
-    rewrite sep_heap_Emp; easy. 
-  + assert (x0 <> x).
-      eauto with wf var.
-    unfold nonfreevars in *.
-    rewrite sep_heap_add.
-    intro e.
-    push_subst.
-    f_equal.
-    unfold sep_heap_bind.
-    push_subst.
-    f_equal.
-    f_equal.
-    unfold emapsto, eval_to; simpl.
-    unfold subst_pred, subst_one; simpl.
-    unfold stk, runloc; simpl.
-    destruct (eq_dec x0 x).
-    contradiction. reflexivity.
-    rewrite <- fresh_var_nonfree_ty; eauto.
-    eauto.
-    eapply fresh_loc_not_In; eauto.
- Qed.
+  apply fv_var_sep_heap.
+  apply H0.
+Qed.
+
+(* Lemma var_nonmem_free_heap : *)
+(*   forall G H H' x, fresh x G H -> wf_heap G H H' -> nonfv (sep_heap H') x. *)
+(* Proof. *)
+(*   intros. *)
+(*   apply fv_var_sep_heap. *)
+(*   induction H1. simpl nonfv. repeat intro. *)
+(*   rewrite HE_Props.F.elements_mapsto_iff in *. *)
+(*   rewrite HE_Props.elements_Empty in *. *)
+(*   rewrite H in *. inv H1. *)
+
+(*   (* apply IHwf_heap in H0. *) *)
+(*   (* simpl nonfv in H0. unfold nonfv_heap in *. *) *)
+(*   repeat intro. *)
+(*   unfold HE_Props.Add in *. *)
+(*   unfold nonfv. simpl. unfold nonfv_heap. *)
+(*   rewrite  HE_Props.F.find_mapsto_iff in *. *)
+(*   specialize (H5 l0). unfold type_binding in *. rewrite H5 in H6. *)
+(*   rewrite <- HE_Props.F.find_mapsto_iff in *. *)
+(*   rewrite HE_Props.F.add_mapsto_iff in *. *)
+(*   decompose [and or] H6; clear H6. destruct xt. inv H9. *)
+(*   split. easy. *)
+(*   simpl. *)
+(*   (* apply fresh_var_nonmem_heap in H0. *) *)
+(*   compare v x.  *)
+(*   intro. subst. exfalso. apply bind_not_in_and_in in H2. contradiction.  *)
+(*   eapply fresh_var_nonmem_heap. eauto. *)
+(*   intro. split. easy. unfold nonfv_reft_t.  *)
+(*   split. simpl nonfv. destruct r. simpl. destruct reft_base; easy. *)
+(*   simpl nonfv. destruct r. simpl. eauto with var. *)
+(*   induction reft_r; try easy.  *)
+(*   + simpl. *)
+
+(*   admit. decide equality. *)
+(*   simpl nonfv in IHwf_heap. unfold nonfv_heap in IHwf_heap.  *)
+(*   simpl nonfv in IHwf_heap. eapply IHwf_heap; eauto. *)
+(*  Qed. *)
+
+Ltac step :=
+  match goal with
+      | |- appcontext[?f (cons _ _)] => unfold f; fold f
+  end.
+
+Lemma wf_expr_empty_heap :
+  forall G e, wf_expr G heap_emp e -> forall H, wf_expr G H e.
+Proof.
+  intros.
+  dependent induction H; eauto with wf var.
+    unfold bind_in in *. destruct H. destruct H.
+    rewrite HE_Props.F.empty_o in *. discriminate H.
+Qed.
+
+Lemma wf_prop_empty_heap :
+  forall G p, wf_prop G heap_emp p -> forall H, wf_prop G H p.
+Proof.
+  intros.
+  dependent induction H; eauto using wf_expr_empty_heap with wf.
+Qed.
 
 Lemma var_nonmem_free_grd :
   forall G H g x, 
-    fresh x G H -> wf_env H G -> wf_guards G H g -> 
-    nonfreevars (sep_guards g) x.
+    fresh x G H -> wf_env H G -> wf_guards G g -> 
+    nonfv (sep_guards g) x.
 Proof.
   intros.
   induction g as [| g'].
-  + unfold nonfreevars. normalize.
-  + unfold sep_guards; fold sep_guards.
-    unfold nonfreevars. 
-    intros.
-    repeat rewrite subst_dist_andp.
-    repeat f_equal.
-    rewrite <- fresh_var_nonfree_pred.
-      reflexivity. eauto. inversion H2. unfold wf_guard in H5.
-      apply H5.
-      apply IHg. inversion H2. auto.
+  + easy.
+  + step. apply nonfv_andp. split. apply nonfv_andp. split.
+    apply SubstProp_var. inv H2.
+    destruct H5.
+    eapply fresh_var_pred_fv; eauto. apply wf_prop_empty_heap. easy.
+    apply IHg. inv H2. apply H6. easy.
 Qed.
 
 Hint Constructors value.
@@ -943,7 +958,7 @@ Lemma var_val :
   forall Γ x b φ, 
     (x,{ ν : b | φ}) ∈ Γ ->
     sep_env Γ |-- (EX v : value,
-                          (fun s => !!(eval s (var_e x) =  v))).
+                          (fun s => !!(eval s (var_e x) = Some v))).
 Proof.
   induction Γ. 
   intuition.
@@ -957,21 +972,78 @@ Proof.
     destruct b0.
       * rewrite exp_andp1; apply exp_left; intros; eapply exp_right.
         apply andp_left1. simpl.
-        intro w. unfold eval_to. apply andp_left1. normalize.
-      * intro w. simpl. eapply exp_right. normalize. 
-      * simpl. intro w. repeat apply andp_left1. eapply exp_right.
-        normalize.
+        intro w. unfold eval_to. 
+        simpl. apply andp_left1. normalize.
+      * intro w. simpl. eapply exp_right. instantiate (1 := null_v).
+        unfold eval_to. simpl. apply andp_left1. apply andp_left1. normalize.
+      * unfold OkRef. simpl. intro. 
+        apply (exp_right (match (runloc x0 l) with 
+                            | Some a => addr_v a 
+                            | None => addr_v (A 0)
+                          end)).
+        destruct (runloc x0 l).
+        repeat apply andp_left1. apply derives_refl.
+        apply andp_left1. rewrite andp_comm. rewrite <- andp_assoc.
+        apply andp_left1.
+        apply derives_extract_prop; intros.
+        apply prop_left. intro. congruence.
   + apply andp_left1. apply andp_left2.
     eauto.
 Qed.
 
+
+Lemma lift_derives :
+  forall (P Q : assert) x,
+    P |-- Q -> P x |-- Q x.
+Proof.
+  firstorder.
+Qed.
+
+Lemma lift_andp :
+  forall (P Q : assert) x,
+    (P && Q) x = P x && Q x.
+Proof. easy. Qed.
+
+Lemma lift_sepconp :
+  forall (P Q : assert) x,
+    (P * Q) x = P x * Q x.
+Proof. easy. Qed.
+
+Lemma lift_emp :
+  forall (x : world),
+    emp = emp x.
+Proof. easy. Qed.
+
+Ltac fix_assert_help :=
+  repeat first [ rewrite <- lift_andp
+               | rewrite <- lift_sepconp
+               | erewrite lift_emp 
+               | apply lift_derives
+               ].
+
+Ltac fix_assert :=
+  let x := fresh "ρ" in
+  match goal with 
+    | |- appcontext[fun ρ : world  => _] => intro x; fix_assert_help; clear x
+    | _ => idtac
+  end.
+
 Lemma var_eval :
-  forall Γ x b φ, 
+  forall Γ x b φ w, 
     (x, { ν : b | φ }) ∈ Γ -> 
-    sep_env Γ |-- (EX v : value, (fun s => !!(eval s (var_e x) = v))).
+    sep_env Γ w |-- (EX v : value, eval_to (var_e x) v w).
 Proof.
   intros.
-  eauto using var_val.
+  unfold eval_to.
+  simpl.
+  rewrite <- exp_andp1.
+  apply andp_right.
+  apply var_val in H. simpl in H.
+  specialize (H w).
+  eapply derives_trans.
+  apply H.
+  normalize.
+  apply sep_env_pure.
 Qed.
 
 Lemma expr_eval :
@@ -980,12 +1052,15 @@ Lemma expr_eval :
     sep_env Γ |-- (EX v : value, eval_to e v).
 Proof.
   intros.
-  unfold eval_to.
-  simpl. intros. rewrite <- exp_andp1.
-  apply andp_right.
-  2: apply sep_env_pure.
-  induction H; eauto using exp_right, var_eval;
-  eapply exp_right; simpl; eauto using prop_right.
+  simpl.
+  intros.
+  induction H.
+  + eapply exp_right. unfold eval_to; simpl. apply andp_right. apply prop_right. reflexivity.
+    apply sep_env_pure.
+  + eapply exp_right. unfold eval_to; simpl. apply andp_right. apply prop_right. reflexivity.
+    apply sep_env_pure.
+  + eapply var_eval. apply H.
+  + eauto using exp_right, var_eval.
 Qed.
 
 Lemma exfalso_etype_fun :
@@ -1013,41 +1088,27 @@ Proof.
   dependent induction H;
     simpl in *.
     intro w.
-    apply exp_right with (x := n). unfold eval_to.
+    apply exp_right with (x := n). unfold eval_to; simpl.
     apply andp_right.
     normalize.
     apply sep_env_pure.
 
-    intro w. apply prop_right. reflexivity.
+    intro w. unfold eval_to; simpl. apply andp_right. apply prop_right. reflexivity.
+    apply sep_env_pure.
 
     intro w. induction Γ as [| (x', t')]. contradiction.
       apply in_inv in H. destruct H. inv H. simpl.
       apply andp_left1. apply andp_left1. 
       unfold sep_ty. simpl. apply andp_left1. apply andp_left1.
       unfold sep_base. simpl. apply andp_left1. apply derives_refl.
-      unfold sep_env. fold sep_env.
+      step.
       simpl.
       apply andp_left1. apply andp_left2. apply IHΓ. assumption.
 
       inv H1. eauto.
 Qed.
 
-(* Lemma expr_eval_ty : *)
-(*   forall Γ Σ Ξ e b φ, *)
-(*     expr_type Γ Σ Ξ e { ν : b | φ } -> *)
-(*     sep_env Γ |--  *)
-(*       (EX v : base_of_type b , (fun s => !!(eval s e = val_of_base b v))). *)
-(* Proof. *)
-(*   intros. *)
-(*   apply derives_trans with *)
-(*     (Q := sep_base e (reft_base { ν : b | φ })). *)
-(*   eapply expr_eval_ty'; eauto. *)
-(*   unfold sep_base.  *)
-(*   rewrite <- exp_andp1. apply andp_left1. normalize. *)
-(* Qed. *)
-
 Hint Resolve 
-     (* expr_eval_ty *)
      exfalso_etype_fun
      expr_eval_ty'
      expr_eval
@@ -1056,13 +1117,14 @@ Hint Resolve
 : eval.
 
 Lemma subst_ty_base_pred :
-  forall v s b p,
-    subst_pred s (sep_ty (var_e v) { ν : b | p }) =
-    subst_pred s (sep_base (var_e v) b && sep_pred (subst (subst_one ν (var_e v)) p) && emp).
+  forall {D R : Type} {S : Subst assert D R } (s : subst_t D R) v b p,
+    subst s (sep_ty (var_e v) { ν : b | p }) =
+    subst s (sep_base (var_e v) b && sep_pred (subst (subst_one ν (var_e v)) p) && emp).
 Proof.
   firstorder.
 Qed.
 
+(**
 Lemma subst_convert_expr :
   forall v w e e',
    ~ (FV e v) ->
@@ -1122,41 +1184,99 @@ Proof.
     eauto with datatypes.
     eauto with datatypes.
 Qed.
+**)
 
-Lemma subst_assign_eq_true :
-  forall v b e,
-    ~ (FV e ν) ->
-    ~ (FV e v) ->
-    sep_base e b
-             |-- subst_pred (subst_one v e) (sep_ty (var_e v) {ν : b | var_e ν .= e}).
+(* Definition F P  *)
+
+Instance Proper_sep_ty :
+    Proper (Logic.eq ==> (@eq reft_type var expr _) 
+                     ==> (Logic.eq ( A := assert)) ) sep_ty.
+Proof.
+  hnf.
+  intros. subst x.
+  hnf.
+  intros t1 t2. intros equ. 
+  inv equ.
+  unfold eq in *. simpl in *.
+  destruct t1. destruct t2. simpl in *.
+  unfold eq_base in *. 
+  assert (reft_base = reft_base0).
+  destruct reft_base; destruct reft_base0; try easy. inv H. easy.
+  subst reft_base0.
+  unfold sep_ty. f_equal. f_equal.
+  clear H.
+  generalize H0. clear H0. generalize reft_r0. clear reft_r0.
+  induction reft_r; destruct reft_r0; intros; try easy.
+  inv H0. rewrite H. rewrite H1. reflexivity.
+  simpl in H0. simpl. extensionality. f_equal. f_equal. 
+  unfold subst in IHreft_r. simpl in *. erewrite IHreft_r. eauto. easy.
+  simpl in H0.
+  simpl in *. rewrite (IHreft_r1 reft_r0_1). rewrite (IHreft_r2 reft_r0_2).
+  reflexivity. easy. easy.
+  simpl in *. rewrite (IHreft_r1 reft_r0_1). rewrite (IHreft_r2 reft_r0_2).
+  reflexivity. easy. easy.
+Qed.
+
+Lemma subst_help :
+  forall (v : var) (e x : expr) ,
+    nonfv e ν ->
+    nonfv x ν -> nonfv (subst (subst_one v e) x) ν.
 Proof.
   intros.
-  rewrite subst_ty_base_pred.
-  repeat rewrite subst_dist_andp.
-  repeat apply andp_right. 
-    unfold subst_one, subst_pred.
-    unfold sep_base. simpl.
-    intro w. 
-    apply andp_derives.
-    destruct b; unfold eval_to, eval, stk; simpl; destruct (eq_dec v v) eqn:?X;
-      try (apply derives_refl || congruence).
-    apply derives_refl.
-  rewrite subst_prop_rel.
-  rewrite subst_expr_non_fv with (e := e).
-  unfold subst, Subst_var_expr, subst_one. simpl.
-  unfold subst_pred, eval, stk.
-  destruct (eq_dec ν ν). 
-  simpl.
-  destruct (eq_dec v v).
+  unfold subst_one. unfold subst. simpl.
+  unfold NFV.
+  induction x; simpl.
+  + easy. 
+  + destruct (eq_dec v v0); simpl. subst v.
+    intuition.
+    compute in H0. intuition.
+  + easy.
+  + intro. apply in_app_or in H1.
+    simpl in H0. unfold NFV in H0. simpl in H0. 
+    assert (nonfv x1 ν).
+    intro.
+    apply H0. apply in_or_app. left. easy.
+    assert (nonfv x2 ν). 
+    intro.
+    apply H0. apply in_or_app. right. easy.
+    intuition.
+Qed.
+
+Lemma subst_assign_eq_true :
+  forall (v : var) b (e : expr),
+    (v <> ν) -> nonfv e ν -> nonfv e v -> 
+    sep_base e b
+             |-- subst (subst_one v e) (sep_ty (var_e v) {ν : b | var_e ν .= e}).
+Proof.
+  intros.
+  rewrite <- sep_ty_subst.
+  setoid_rewrite subst_nonfv at 2.
+  unfold subst_one. unfold subst. simpl. destruct (eq_dec v v).
   intro w.
-  rewrite subst_help with (v := v) (e' := e).
+  destruct ({ν : b | var_e ν .= e}) eqn: FOO.
+  inv FOO.
+  unfold sep_ty.
+  simpl. apply andp_right. apply andp_right.
   normalize.
+  pose (subst_nonfv (subst_one ν e) e).
+  setoid_rewrite e1. apply andp_right. apply prop_right.
+  unfold subst_one. destruct (eq_dec ν ν). reflexivity. congruence.
   apply sep_base_pure.
-  assumption.
+  intros v' X. intro. simpl in H0. unfold NFV in H0. 
+  unfold subst_one in X. destruct (eq_dec ν v'). subst v'. congruence.
   congruence.
-  congruence.
-  assumption.
   apply sep_base_pure.
+  congruence.
+  intro v'. intro X.
+  unfold nonfv. simpl. unfold nonfv_reft_t. split.
+  unfold nonfv. simpl. destruct b; easy. 
+  split. intro. unfold subst_one in X. destruct (eq_dec v v'). subst v'.
+  unfold fv_expr in *. inv H2. congruence. inv H3. congruence.
+  unfold subst_one in X. destruct (eq_dec v v'). subst v'. easy. congruence.
+  unfold subst. simpl. unfold subst_one. destruct (eq_dec v ν).
+  subst v. congruence. reflexivity.
+  intros e' X.
+  apply subst_help; easy.
 Qed.
 
 Lemma expr_type_wf :
@@ -1168,14 +1288,6 @@ Proof.
   exists {ν : τ | φ}. eauto.
 Qed.
 
-Ltac nfv_env := 
-  match goal with
-    | H : nonfreevars _ ?v |- appcontext[subst_one ?v _] =>
-      unfold nonfreevars in H; erewrite <- H; simpl; eauto using andp_left1, andp_left2, derives_refl
-    | |- _ |-- subst_pred (subst_one ?v _) ?P =>
-      assert (nonfreevars P v); eauto using var_nonmem_free_ctx, var_nonmem_free_grd; nfv_env
-  end.
-
 Lemma sep_base_eval :
   forall e τ φ,
     sep_base e (reft_base {ν : τ | φ}) |-- exp (eval_to e).
@@ -1183,9 +1295,25 @@ Proof.
   intros.
   unfold sep_base.
   destruct τ;
-    simpl; intro w; try rewrite exp_andp1; try apply exp_left; try eapply exp_right; unfold eval_to; normalize.
+    simpl; intro w; try rewrite exp_andp1; try apply exp_left. 
+    try eapply exp_right; unfold eval_to; normalize.
   intros.
-  eapply exp_right. apply andp_right. rewrite H. apply prop_right. reflexivity. normalize.
+  eapply exp_right. simpl. apply andp_right. rewrite H. apply prop_right. reflexivity. normalize.
+  try eapply exp_right; unfold eval_to; simpl; normalize.
+  unfold OkRef.
+  unfold eval_to.
+  simpl.
+  rewrite <- exp_andp1.
+  apply andp_right.
+  apply andp_left1.
+  rewrite andp_assoc.
+  apply derives_extract_prop. intro.
+  apply derives_extract_prop. intro.
+  apply prop_left. intro.
+  simpl in *.
+  destruct (runloc w l). apply (exp_right (addr_v a)). normalize.
+  congruence.
+  repeat apply (andp_left2). easy.
 Qed.
 
 Lemma sep_schema_in_env :
@@ -1374,227 +1502,243 @@ Proof.
   do_pure.
 Qed.
 
-Lemma subst_loc_expr :
-  forall (s : loc -> loc) (e : expr),
-    fl_expr e = [] ->
-    subst s e = e.
-Proof.
-  intros.
-  unfold subst. 
-  simpl.
-  induction e; simpl in *; try first [reflexivity | congruence].
-  apply app_eq_nil in H.
-  rewrite IHe1; repeat (reflexivity || rewrite IHe2 || intuition).
-Qed.
+(* Lemma subst_loc_expr : *)
+(*   forall (s : subst_t loc loc) (e : expr), *)
+(*     fl_expr e = [] -> *)
+(*     subst s e = e. *)
+(* Proof. *)
+(*   intros. *)
+(*   unfold subst.  *)
+(*   simpl. *)
+(*   induction e; simpl in *; try first [reflexivity | congruence]. *)
+(*   apply app_eq_nil in H. *)
+(*   rewrite IHe1; repeat (reflexivity || rewrite IHe2 || intuition). *)
+(* Qed. *)
 
-Lemma wf_expr_not_loc :
-  forall (s : loc -> loc) e,
-    fl_expr e = [] -> 
-    forall w, eval w e = eval (stk w, fun l => runloc w (s l), hp w) e.
-Proof.
-  intros.
-  induction e; eauto.
-  inv H.
-  simpl in *.
-  apply app_eq_nil in H.
-  intuition.
-  rewrite H.
-  rewrite H2.
-  reflexivity.
-Qed.
+(* Lemma wf_expr_not_loc : *)
+(*   forall (s : subst_t loc loc) e, *)
+(*     fl_expr e = [] ->  *)
+(*     forall w, eval w e = eval (subst s w) (* (stk w, fun l => runloc w (s l), hp w) *) e. *)
+(* Proof. *)
+(*   intros. *)
+(*   induction e; eauto. *)
+(*   inv H. *)
+(*   simpl in *. *)
+(*   apply app_eq_nil in H. *)
+(*   intuition. *)
+(*   rewrite H. *)
+(*   rewrite H2. *)
+(*   reflexivity. *)
+(* Qed. *)
 
-Lemma subst_loc_pred_prop' :
-  forall  (s : loc -> loc) (p : reft_prop),
-    fl_prop p = [] ->
-    forall x, sep_pred p x = subst_pred_loc s (sep_pred p) x.
-Proof.
-  intros until p.
-  induction p; intro; eauto. 
-  +  intro w.
-     unfold sep_pred.
-     unfold fl_prop in *.
-     apply app_eq_nil in H.
-     unfold subst_pred_loc.
-     simpl.
-     f_equal.
-     intuition; repeat erewrite <- wf_expr_not_loc; eauto.
-  + intro w.
-    unfold subst_pred_loc in *.
-    simpl.
-    rewrite <- IHp.
-    reflexivity.
-    assumption.
-  + intro w.
-    unfold subst_pred_loc in *.
-    simpl in *.
-    apply app_eq_nil in H.
-    rewrite <- IHp1; try solve [intuition; eauto].
-    rewrite <- IHp2; intuition; eauto.
-  + intro w.
-    unfold subst_pred_loc in *.
-    simpl in *.
-    apply app_eq_nil in H.
-    rewrite <- IHp1; try solve [intuition; eauto].
-    rewrite <- IHp2; intuition; eauto.
-Qed.
+(* Lemma subst_loc_pred_prop' : *)
+(*   forall (s : subst_t loc loc) (p : reft_prop), *)
+(*     fl_prop p = [] -> *)
+(*     forall x, sep_pred p x = subst s (sep_pred p) x. *)
+(* Proof. *)
+(*   intros until p. *)
+(*   induction p; intro; eauto.  *)
+(*   +  intro w. *)
+(*      unfold sep_pred. *)
+(*      unfold fl_prop in *. *)
+(*      apply app_eq_nil in H. *)
+(*      unfold subst_pred_loc. *)
+(*      simpl. *)
+(*      f_equal. *)
+(*      intuition; repeat erewrite <- wf_expr_not_loc; eauto. *)
+(*   + intro w. *)
+(*     unfold subst_pred_loc in *. *)
+(*     simpl. *)
+(*     rewrite <- IHp. *)
+(*     reflexivity. *)
+(*     assumption. *)
+(*   + intro w. *)
+(*     unfold subst_pred_loc in *. *)
+(*     simpl in *. *)
+(*     apply app_eq_nil in H. *)
+(*     rewrite <- IHp1; try solve [intuition; eauto]. *)
+(*     rewrite <- IHp2; intuition; eauto. *)
+(*   + intro w. *)
+(*     unfold subst_pred_loc in *. *)
+(*     simpl in *. *)
+(*     apply app_eq_nil in H. *)
+(*     rewrite <- IHp1; try solve [intuition; eauto]. *)
+(*     rewrite <- IHp2; intuition; eauto. *)
+(* Qed. *)
 
-Lemma subst_loc_pred_prop :
-  forall (s : loc -> loc) p,
-    fl_prop p = [] ->
-    sep_pred (subst s p) = subst_pred_loc s (sep_pred p).
-Proof.
-  intros.
-  unfold subst, Subst_prop_loc, subst_prop_loc.
-  extensionality.
-  erewrite <- subst_loc_pred_prop'; eauto.
-Qed.
+(* Lemma subst_pred_expr : *)
+(*   forall {D R : Type}  *)
+(*          {SE : Subst expr D R} *)
+(*          {SA : Subst assert D R} *)
+(*          {SAA : SubstAssert D R} *)
+(*          (s : subst_t D R) e v, *)
+(*     subst s e  *)
 
-Lemma subst_base_loc :
-  forall (s : loc -> loc) e b,
-    fl_expr e = [] -> 
-    sep_base (subst s e) (subst s b) = subst_pred_loc s (sep_base e b).
-Proof.
-  intros.
-  unfold sep_base; destruct b; simpl; erewrite subst_loc_expr; eauto; unfold subst_pred_loc; extensionality.
-  + f_equal.
-    f_equal.
-    extensionality.
-    unfold eval_to.
-    erewrite <- wf_expr_not_loc; eauto.
-  + f_equal.
-    f_equal.
-    erewrite <- wf_expr_not_loc; eauto.
-  + f_equal.
-    f_equal.
-    erewrite <- wf_expr_not_loc; eauto.
-    erewrite <- wf_expr_not_loc; eauto.
-Qed.
+(* Lemma subst_loc_pred_prop : *)
+(*   forall {D R : Type}  *)
+(*          {S : Subst reft_prop D R}  *)
+(*          {SE : Subst expr D R} *)
+(*          {SR : SubstReft D R} *)
+(*          {SA : Subst assert D R} *)
+(*          {SAA : SubstAssert D R} *)
+(*          (s : subst_t D R) p,  *)
+(*     fl_prop p = [] -> *)
+(*     sep_pred (subst s p) = subst s (sep_pred p). *)
+(* Proof. *)
+(*   Hint Transparent sep_pred. *)
+(*   intros. *)
+(*   induction p; intros. *)
+(*   { *)
+(*   rewrite subst_tt_r. *)
+(*   unfold sep_pred; push_subst. *)
+(*      admit.  *)
+(*   } *)
+(*   { *)
+(*   rewrite subst_rel_r. *)
+(*   unfold sep_pred; push_subst. *)
+(*   simpl. *)
+(*   extensionality. *)
+(*   f_equal. *)
+(* Qed. *)
 
-Lemma subst_prop_loc_var_comm :
-  forall (p : reft_prop) (s1 : subst_t var expr) (s2 : subst_t loc loc),
-    subst s1 (subst s2 p) = subst s2 (subst s1 p).
-Proof.
-  firstorder.
-Qed.
+(*   intros. *)
+(*   unfold subst, Subst_prop_loc, subst_prop_loc. *)
+(*   extensionality. *)
+(*   erewrite <- subst_loc_pred_prop'; eauto. *)
+(* Qed. *)
 
-Lemma subst_fl_closed_expr :
-  forall v x e,
-    fl_expr x = [] ->
-    fl_expr e = [] ->
-    fl_expr (subst (subst_one v x) e) = [].
-Proof.
-  intros;
-  induction e; try reflexivity.
-  + unfold subst, subst_one. simpl.
-    destruct (eq_dec v0 v); assumption. 
-  + inv H0.
-  + simpl in *.
-    apply app_eq_nil in H0.
-    destruct H0.
-    unfold subst in IHe1.
-    unfold subst in IHe2.
-    rewrite IHe1.
-    rewrite IHe2.
-    reflexivity.
-    assumption.
-    assumption.
-Qed.
+(* Lemma subst_base_loc : *)
+(*   forall (s : loc -> loc) e b, *)
+(*     fl_expr e = [] ->  *)
+(*     sep_base (subst s e) (subst s b) = subst_pred_loc s (sep_base e b). *)
+(* Proof. *)
+(*   intros. *)
+(*   unfold sep_base; destruct b; simpl; erewrite subst_loc_expr; eauto; unfold subst_pred_loc; extensionality. *)
+(*   + f_equal. *)
+(*     f_equal. *)
+(*     extensionality. *)
+(*     unfold eval_to. *)
+(*     erewrite <- wf_expr_not_loc; eauto. *)
+(*   + f_equal. *)
+(*     f_equal. *)
+(*     erewrite <- wf_expr_not_loc; eauto. *)
+(*   + f_equal. *)
+(*     f_equal. *)
+(*     erewrite <- wf_expr_not_loc; eauto. *)
+(*     erewrite <- wf_expr_not_loc; eauto. *)
+(* Qed. *)
 
-Lemma subst_fl_closed_prop :
-  forall v x p,
-    fl_expr x = [] ->
-    fl_prop p = [] ->
-    fl_prop (subst (subst_one v x) p ) = [].
-Proof.
-  intros.
-  induction p.
-  + reflexivity.
-  + simpl in *.
-    unfold subst.
-    apply app_eq_nil in H0.
-    repeat rewrite subst_fl_closed_expr; try (reflexivity || apply H || apply H0).
-  + auto.
-  + simpl in *.
-    apply app_eq_nil in H0.
-    unfold subst in *.
-    rewrite IHp1.
-    rewrite IHp2.
-    reflexivity.
-    apply H0.
-    apply H0.
-  + simpl in *.
-    apply app_eq_nil in H0.
-    unfold subst in *.
-    rewrite IHp1.
-    rewrite IHp2.
-    reflexivity.
-    apply H0.
-    apply H0.
-Qed.
+(* Lemma subst_prop_loc_var_comm : *)
+(*   forall (p : reft_prop) (s1 : subst_t var expr) (s2 : subst_t loc loc), *)
+(*     subst s1 (subst s2 p) = subst s2 (subst s1 p). *)
+(* Proof. *)
+(*   intros. *)
+(*   rewrite subst_nonfv. *)
+(* Qed. *)
+
+(* Lemma subst_fl_closed_expr : *)
+(*   forall v x e, *)
+(*     fl_expr x = [] -> *)
+(*     fl_expr e = [] -> *)
+(*     fl_expr (subst (subst_one v x) e) = []. *)
+(* Proof. *)
+(*   intros; *)
+(*   induction e; try reflexivity. *)
+(*   + unfold subst, subst_one. simpl. *)
+(*     destruct (eq_dec v0 v); assumption.  *)
+(*   + inv H0. *)
+(*   + simpl in *. *)
+(*     apply app_eq_nil in H0. *)
+(*     destruct H0. *)
+(*     unfold subst in IHe1. *)
+(*     unfold subst in IHe2. *)
+(*     rewrite IHe1. *)
+(*     rewrite IHe2. *)
+(*     reflexivity. *)
+(*     assumption. *)
+(*     assumption. *)
+(* Qed. *)
+
+(* Lemma subst_fl_closed_prop : *)
+(*   forall v x p, *)
+(*     fl_expr x = [] -> *)
+(*     fl_prop p = [] -> *)
+(*     fl_prop (subst (subst_one v x) p ) = []. *)
+(* Proof. *)
+(*   intros. *)
+(*   induction p. *)
+(*   + reflexivity. *)
+(*   + simpl in *. *)
+(*     unfold subst. *)
+(*     apply app_eq_nil in H0. *)
+(*     repeat rewrite subst_fl_closed_expr; try (reflexivity || apply H || apply H0). *)
+(*   + auto. *)
+(*   + simpl in *. *)
+(*     apply app_eq_nil in H0. *)
+(*     unfold subst in *. *)
+(*     rewrite IHp1. *)
+(*     rewrite IHp2. *)
+(*     reflexivity. *)
+(*     apply H0. *)
+(*     apply H0. *)
+(*   + simpl in *. *)
+(*     apply app_eq_nil in H0. *)
+(*     unfold subst in *. *)
+(*     rewrite IHp1. *)
+(*     rewrite IHp2. *)
+(*     reflexivity. *)
+(*     apply H0. *)
+(*     apply H0. *)
+(* Qed. *)
+
+(**
 
 Lemma subst_ty_loc :
-  forall (s : loc -> loc) x T,
-    fl_expr x = [] ->
-    fl_prop (reft_r T) = [] ->
-    sep_ty (subst s x) (subst s T) = subst_pred_loc s (sep_ty x T).
+  (* forall {D R : Type} {S : Subst assert D R} {Sa : SubstAssert D R} {St : Subst reft_type D R} {Sp : Subst reft_prop D R} {Se : Subst expr D R} (s : subst_t D R) x T, *)
+  forall x T (s : subst_t loc loc),
+  (forall (l : loc), nonfv x l) ->
+  (forall (l : loc), nonfv (reft_r T) l) ->
+  (forall (x : expr), nonfv x ν -> nonfv (subst s x) ν) ->
+    sep_ty (subst s x) (subst s T) = subst s (sep_ty x T).
 Proof.
   intros.
-  destruct T.
-  simpl in * |- .
-  unfold sep_ty at 2.
-  push_subst.
-  erewrite <- subst_base_loc; eauto.
-  erewrite <- subst_loc_pred_prop; eauto.
-  unfold sep_ty.
-  unfold subst at 1. simpl. extensionality. f_equal. f_equal. f_equal.
-  rewrite <- subst_prop_loc_var_comm.
-  erewrite subst_loc_expr; eauto.
-  apply subst_fl_closed_prop; assumption.
-Qed.
-
-Lemma subst_heap_loc' :
-  forall (s : loc -> loc) H,
-    fold (fun l xt a => (subst s (sep_heap_bind l xt)) * a) H emp 
-    = subst s (fold (fun l xt a => sep_heap_bind l xt * a) H emp).
-Proof.
-  intros.
-  apply HE_Props.fold_rel with
-    (R := fun a b => a = subst s b).
-  + reflexivity.
-  + intros.
-    push_subst.
-    f_equal. assumption.
+  destruct T as [b p].
+  setoid_rewrite sep_ty_subst.
+  reflexivity.
+  unfold subst. simpl. reflexivity.
+  intros. 
+  apply H1.
+  easy.
 Qed.
 
 Lemma subst_heap_loc'' :
-  forall s L,
-    subst_pred_loc s
+  forall (s : subst_t loc loc) L,
+    Forall (fun lxt => (forall (l : loc), nonfv (reft_r (snd (snd lxt))) l)) L ->
+    (subst s
       (fold_right (fun lxt a => sep_heap_bind (fst lxt) (snd lxt) * a) emp L)
-   = fold_right (fun lxt a => sep_heap_bind (fst lxt) (snd lxt) * a) emp (subst s L).
+   = fold_right (fun lxt a => sep_heap_bind (fst lxt) (snd lxt) * a) emp (subst s L)).
 Proof.
   intros.
   induction L as [ | [l [x t]]].
   reflexivity.
-  unfold subst. unfold Subst_list, subst_list. fold subst_list.
-  unfold fold_right at 2. 
-  fold fold_right.
-  unfold subst in IHL.
+  push_subst.
+  unfold fold_right at 2.
   unfold fold_right at 2 in IHL.
-  unfold Subst_list, subst_list in IHL. fold subst_list in IHL.
   rewrite <- IHL.
-  unfold fold_right. push_subst.
+  unfold fold_right.
+  push_subst.
   f_equal.
   unfold fst, snd.
-  unfold subst_pred_loc.
   unfold sep_heap_bind. 
-  unfold subst. unfold Subst_prod. unfold subst_prod.
-  unfold subst, Subst_prod, subst_prod, Subst_binding_loc, Subst_loc_loc, subst_loc.
   extensionality w.
-  unfold subst. simpl. 
+  push_subst.
   f_equal. f_equal.
-  Admitted.
-
-Definition eqk := @eq_key type_binding.
+  rewrite (subst_ty_loc s (var_e x)).
+  reflexivity.
+  reflexivity.
+  inv H. eauto with datatypes.
+  inv H; assumption.
+Qed.
 
 Lemma helper :
   forall l1 l2,
@@ -1619,25 +1763,24 @@ Proof.
 Qed.
 
 Lemma thingie' :
-  forall (s : loc -> loc) (x y : loc * type_binding),
-    (forall l m, s l = s m -> l = m) ->
+  forall {D R : Type} {Sl : Subst loc D R} {St : Subst type_binding D R } 
+         s (x y : loc * type_binding),
+    (forall (l m : loc), subst s l = subst s m -> l = m) ->
     eqk (subst s x) (subst s y) -> eqk x y.
 Proof.
   intros.
   destruct x as [l xt].
   destruct y as [m yt].
-  unfold eqk in H0.
-  unfold subst in H0.
-  unfold eq_key in H0.
   inv H0.
-  apply H in H2. 
-  rewrite H2.
+  apply H in H2.
+  subst.
   reflexivity.
 Qed.
 
 Lemma thingie :
-  forall (s : loc -> loc) (e : loc * type_binding) l,
-    (forall l m, s l = s m -> l = m) ->
+  forall {D R : Type} {S : Subst loc D R } {S' : Subst type_binding D R} 
+         (s : subst_t D R) (e : (loc * type_binding)) l,
+    (forall (l m : loc), subst s l = subst s m -> l = m) ->
     InA eqk (subst s e) (subst s l) -> InA eqk e l.
 Proof.
   intros.
@@ -1646,7 +1789,7 @@ Proof.
   + rewrite subst_cons in H0.
     inv H0.
     left.
-    apply thingie' with (s := s).
+    apply (thingie' s). 
     assumption.
     apply H2.
     right.
@@ -1655,8 +1798,9 @@ Proof.
 Qed.
 
 Lemma NoDupA_subst_heap_binds :
-  forall (s : loc -> loc) (L : list (loc * type_binding)),
-    (forall l m, s l = s m -> l = m) ->
+  forall {D R : Type} {S : Subst loc D R } {S' : Subst type_binding D R } 
+         s (L : list (loc * type_binding)),
+    (forall (l m : loc), subst s l = subst s m -> l = m) ->
     NoDupA eqk L ->
     NoDupA eqk (subst s L).
 Proof.
@@ -1668,7 +1812,7 @@ Proof.
     intro.
     inv H0.
     apply H4.
-    apply thingie with (s := s). 
+    apply (thingie s).
     assumption.
     assumption.
     apply IHL.
@@ -1676,8 +1820,8 @@ Proof.
 Qed.
 
 Lemma NoDup_Heap :
-  forall s H,
-    (forall l m, s l = s m -> l = m) ->
+  forall {D R : Type} {S : Subst loc D R} {S' : Subst type_binding D R} s H,
+    (forall (l m : loc), s l = s m -> l = m) ->
     (forall lxt, InA eqA lxt (elements (subst s H)) <-> 
                 InA eqA lxt (subst s (elements H))).
 Proof.
@@ -1700,75 +1844,144 @@ Proof.
   assumption.
 Qed.
 
-Lemma subst_heap_loc :
-  forall (s : loc -> loc) H,
-    (forall lxt,
-      List.In lxt (elements (subst s H))
-      <-> List.In lxt (subst s (elements H))) ->
-    sep_heap (subst s H) = subst_pred_loc s (sep_heap H).
+Lemma subst_eq_heaps :
+  forall {D R : Type} {S : Subst loc D R} {S' : Subst type_binding D R} s H,
+    (forall (l m : loc), s l = s m -> l = m) ->
+    Equal (subst s H) (HE_Props.of_list (subst s (elements H))).
 Proof.
   intros.
-  (* unfold sep_heap. *)
-  (* unfold subst, Subst_heap_loc, subst_heap_loc. *)
-  (* rewrite HE_Props.fold_spec_right. *)
-  (* rewrite HE_Props.fold_spec_right. *)
-  (* rewrite HE_Props.fold_spec_right. *)
+  assert (forall lxt, InA eqA lxt (elements (subst s H)) <-> InA eqA lxt (subst s (elements H)))
+  by (apply NoDup_Heap; assumption).
+  assert (Equal (HE_Props.of_list (elements (subst s H))) (HE_Props.of_list (subst s (elements H)))).
+  apply helper.
+  apply elements_3w.
+  apply NoDupA_subst_heap_binds.
+  assumption.
+  apply elements_3w.
+  apply H1.
+  rewrite HE_Props.of_list_3 in H2.
+  assumption.
+Qed.  
+
+Instance EQA_EQUIVALENCE : Equivalence eqA := _.
+Instance EQK_EQUIVALENCE : Equivalence eqk := _.
+
+Lemma heap_equiv_elements_subst :
+  forall {D R : Type} {S : Subst loc D R} {S' : Subst type_binding D R} H s,
+    (forall (l m : loc), s l = s m -> l = m) ->
+    equivlistA
+      eqA
+      (rev (elements (HE_Props.of_list (subst s (elements H)))))
+      (subst s (rev (elements H))).
+Proof.
+  intros.
+  push_subst.
+  pose (@HE_Props.of_list_2 type_binding).
+  cut (forall l l', equivlistA eqA l l' -> equivlistA eqA (rev l) (rev l')).
+  intros.
+  symmetry.
+  apply H1.
+  apply HE_Props.of_list_2.
+  apply NoDupA_subst_heap_binds.
+  assumption.
+  apply elements_3w.
+  intros.
+  intro. destruct H1 with (x := x).
+  constructor; intros; apply InA_rev; try apply EQA_EQUIVALENCE;
+  [ apply H2 | apply H3]; apply InA_rev; try apply EQA_EQUIVALENCE; assumption.
+Qed.
+
+Lemma heap_free_locs :
+  forall (h : heap_env),
+    (forall l x t, MapsTo l (x,t) h -> fl_prop (reft_r t) = []) ->
+    (forall l x t, List.In (l,(x,t)) (elements h) -> fl_prop (reft_r t) = []).
+Proof.
+  intros.
+  apply H with (l := l) (x := x).
+  apply In_InA with (eqA := eqA) in H0.
+  apply HE_Facts.elements_mapsto_iff.
+  apply H0.
+  apply EQA_EQUIVALENCE.
+Qed.
+
+Lemma subst_heap_loc :
+  forall {D R : Type} {S : Subst loc D R} {S' : Subst type_binding D R} {SA: Subst assert D R}
+         (s : subst_t D R) H,
+    (forall l x t, MapsTo l (x,t) H -> fl_prop (reft_r t) = []) ->
+    (forall (l m : loc), subst s l = subst s m -> l = m) ->
+    sep_heap (subst s H) = subst s (sep_heap H).
+Proof.
+  intros.
   unfold sep_heap at 2.
   rewrite HE_Props.fold_spec_right.
   rewrite subst_heap_loc''.
   unfold sep_heap.
+  rewrite HE_Props.fold_Equal with (m1 := subst s H) (m2 := HE_Props.of_list (subst s (elements H))).
   rewrite fold_1.
-  unfold subst.
-  unfold Subst_list.
-  assert (subst_list (loc * type_binding) _ _ _ s (rev (elements H)) = (rev (subst s (elements H)))) by admit.
-  rewrite H1.
-  rewrite fold_left_rev_right.
-  rewrite <- 
-
-  unfold subst.
-  unfold subst in H1. rewrite H1.
-  Set Printing All.
-  idtac.
-  rewrite  H1.
-  rewrite <- H0.
-
-  apply HE_Props.fold_rel with 
-  (R := fun m b => fold (fun l xt a => sep_heap_bind l xt * a) m emp = b).
-  reflexivity.
-  intros.
-  rewrite HE_Props.fold_add.
-  admit. admit. admit. admit.
-  rewrite fold_1.
-  reflexivity.
-  intros.
-  rewrite H2.
-  admit.
-  apply EQ_EQUIVALENCE.
-  solve_proper.
-  admit.
-  
-  rewrite HE_Props.fold_Empty.
-
-Lemma subst_ctx_loc :
-  forall G H s,
-    subst_pred_loc s (sep_env G) 
-    = sep_env (@subst _ _ _ (Subst_list (var * reft_type) loc loc (Subst_prod _ _ _ _ _ _)) s G).
-Proof.
-  intros.
-  induction G as [ | [x t]].
-  + reflexivity.
-  + unfold subst, Subst_list, subst_list. fold subst_list.
-    unfold sep_env; fold sep_env.
-    push_subst.
-    simpl.
-    extensionality.
-    repeat f_equal.
-    pose (subst_ty_loc ((x,t) :: G) H s (var_e x) t).
-    elim e. reflexivity. 
-    inv H0. constructor. unfold var_in. exists t. left. reflexivity.
-    inv H0; eauto.
-    rewrite IHG. reflexivity. inv H0; eauto.
+  rewrite <- fold_left_rev_right.
+  rewrite 
+    (fold_right_equivlistA).
+    auto.
+    apply HE_Props.eqke_equiv.
+    apply EQ_EQUIVALENCE.
+    destruct x. destruct y.
+    intros. inv H2. simpl in *. subst. reflexivity.
+    hnf. intros. 
+    simpl. extensionality ρ. 
+    do 2 rewrite <- sepcon_assoc.
+    rewrite sepcon_comm with (P := sep_heap_bind (fst x) (snd x) (ρ)).
+    reflexivity.
+    apply NoDupA_rev. apply EQA_EQUIVALENCE. 
+    apply HE_Props.NoDupA_eqk_eqke.
+    apply elements_3w.
+    apply HE_Props.NoDupA_eqk_eqke.
+    apply NoDupA_subst_heap_binds.
+    assumption.
+    apply NoDupA_rev. 
+    apply EQK_EQUIVALENCE.
+    apply elements_3w.
+    apply heap_equiv_elements_subst.
+    assumption.
+    apply EQ_EQUIVALENCE.
+    solve_proper.
+    hnf. intros. 
+    simpl. extensionality ρ. 
+    do 2 rewrite <- sepcon_assoc.
+    rewrite sepcon_comm with (P := sep_heap_bind k e (ρ)).
+    reflexivity.
+    apply subst_eq_heaps.
+    assumption.
+    rewrite Forall_forall.
+    intros.
+    rewrite <- in_rev in H2.
+    destruct x as [l [x t]].
+    eapply heap_free_locs; eauto.
 Qed.
+**)
+
+(* Lemma subst_ctx_loc : *)
+(*   forall G s, *)
+(*     (Forall (fun xt => fl_prop (reft_r (snd xt)) = []) G) -> *)
+(*     sep_env (@subst _ _ _ (Subst_list (var * reft_type) loc loc (Subst_prod _ _ _ _ _ _)) s G) *)
+(*     = subst s (sep_env G). *)
+(* Proof. *)
+(*   intros. *)
+(*   induction G as [ | [x t]]. *)
+(*   + reflexivity. *)
+(*   + push_subst. *)
+(*     unfold sep_env; fold sep_env. *)
+(*     simpl. *)
+(*     extensionality w. *)
+(*     unfold subst, Subst_pred_loc, subst_pred_loc. *)
+(*     f_equal. f_equal. *)
+(*     rewrite (subst_ty_loc s (var_e x)). *)
+(*     reflexivity. *)
+(*     reflexivity. *)
+(*     rewrite Forall_forall in *. specialize (H (x, t)). apply H. left. reflexivity. *)
+(*     unfold subst in IHG. *)
+(*     rewrite IHG. reflexivity.  *)
+(*     inv H. assumption. *)
+(* Qed. *)
 
 Ltac lift_apply l :=
   let X := fresh "X" in
@@ -1794,56 +2007,480 @@ Proof.
   (* lift_apply types_interp; eauto. *)
   (* lift_apply heap_subtype_interp; eauto. *)
 Admitted.
+Notation "S · T" := (subst S T) (right associativity, at level 60).
+(* Lemma loc_sub_proc_call : *)
+(*   forall (θ : subst_t loc loc) f xs x mxs mls, *)
+(*     (θ·proc_s f xs x mxs mls) = proc_s f xs x mxs (θ·mls). *)
+(* Proof. *)
+(*   Admitted. *)
 
-Lemma lift_derives :
-  forall (P Q : assert) x,
-    P |-- Q -> P x |-- Q x.
+Lemma loc_sub_var2var :
+  forall (θ : subst_t loc loc), var_2_var θ.
 Proof.
   firstorder.
 Qed.
 
-Lemma lift_andp :
-  forall (P Q : assert) x,
-    (P && Q) x = P x && Q x.
-Proof. easy. Qed.
+Lemma var_sub_var2var :
+  forall (θ : subst_t var var), var_2_var θ.
+Proof.
+  firstorder.
+Qed.
 
-Lemma lift_sepconp :
-  forall (P Q : assert) x,
-    (P * Q) x = P x * Q x.
-Proof. easy. Qed.
+Lemma wf_subst_vv_nonfv :
+  forall (θ : subst_t var var),
+    wf_subst θ  ->
+    ∀ x0 : expr, nonfv x0 ν → nonfv (θ · x0) ν.
+Proof.
+  intros. unfold wf_subst in *.
+  induction x0; simpl nonfv in *; unfold NFV in *; simpl fv_expr in *.
+  + trivial.
+  + destruct (H v). intuition. simpl subst in *.
+    destruct H3; intuition.
+  + trivial.
+  + intro. apply in_app_or in H1. destruct H1; intuition.
+Qed.
 
-Lemma lift_emp :
-  forall (x : world),
-    emp = emp x.
-Proof. easy. Qed.
+Lemma loc_subst_vv_nonfv :
+  forall (θ : subst_t loc loc), 
+    forall (e : expr), nonfv e ν -> nonfv (θ · e) ν.
+Proof.
+  intros.
+  induction e; simpl nonfv in *; unfold NFV in *; simpl fv_expr in *; trivial.
+  intro. apply in_app_or in H0. destruct H0; intuition.
+Qed.
+(**
+Lemma MapsToSubst' :
+  forall (θ : subst_t loc loc) h l x t,
+    (MapsTo l (x, t) (θ · h) ->
+    (exists (l' : loc) x' t', (l = θ · l') /\ (x = θ · x') /\ (t = θ · t') /\ MapsTo (θ · l') (θ · x', θ · t') (θ · h))).
+Proof.
+  intros until t0.
+  simpl subst at 1 8.
+  unfold subst_heap.
+  (* unfold NonUnifyingSub. *)
+  apply HE_Props.fold_rel with 
+  (f := fun l xt a => add (θ · l) (θ·xt) a)
+  (g := fun l xt a => add (θ · l) (θ·xt) a)
+  (R := fun A B => 
+          MapsTo l (x, t0) A -> 
+          (exists l' x' t', (l = θ · l') /\ (x = θ · x') /\ (t0 = θ · t') /\ MapsTo (θ · l') (θ · x', θ · t') B)).
+  intros. inv H.
+  intros.
+  rewrite HE_Props.F.add_mapsto_iff in H1.
+  decompose [and or] H1; clear H1.
+  destruct e.
+  simpl subst in H4. unfold Subst.subst_prod in H4. inv H4.
+  setoid_rewrite HE_Props.F.add_mapsto_iff.
+  exists k. exists v. exists r. repeat split. left. intuition.
+  apply H0 in H4. destruct H4. destruct H1. destruct H1. decompose [and] H1. clear H1.
+  exists x0. exists x1. exists x2. repeat split. easy. easy. easy.
+  apply HE_Props.F.add_mapsto_iff.
+  right. subst l. intuition.
+Qed.
 
-Ltac fix_assert_help :=
-  repeat first [ rewrite <- lift_andp
-               | rewrite <- lift_sepconp
-               | erewrite lift_emp 
-               | apply lift_derives
-               ].
+Lemma MapsToSubst :
+  forall (θ : subst_t loc loc) h l x t,
+    (MapsTo l (x, t) (θ · h) ->
+    (exists (l' : loc) x' t', MapsTo (θ · l') (θ · x', θ · t') (θ · h))).
+Proof.
+  intros. apply MapsToSubst' in H. destruct H. destruct H.  destruct H. exists x0, x1, x2.
+  intuition.
+Qed.
+  
+Lemma nonunifying_closed :
+  forall (θ : subst_t var var)  (θ' : subst_t loc loc) h,
+    NonUnifyingSub θ h -> NonUnifyingSub θ' h -> NonUnifyingSub θ (θ θ' · h).
+Proof.
+  intros.
+  unfold NonUnifyingSub in *.
+  decompose [and] H. clear H.
+  decompose [and] H0. clear H0.
+  split. trivial.
+  intros l x t.
+  split.
+  intro M.
+  destruct (H3 l x t).
+  destruct (H2 l x t).
+  apply MapsToSubst in M.
+  destruct M as [l' M]. destruct M as [x' M]. destruct M as [t' M].
+  rewrite <- H3 in M.
+  rewrite H2 in M.
+**)
+Lemma subst_vv_fresh :
+  forall (s : subst_t var var),
+    wf_subst s ->
+    s · (var_e ν) = var_e ν.
+Proof.
+  intros.
+  unfold wf_subst in *.
+  destruct (H ν).
+  simpl subst in  *. simpl in *.
+  rewrite H1; reflexivity.
+Qed.
 
-Ltac fix_assert :=
-  let x := fresh "ρ" in
-  match goal with 
-    | |- appcontext[fun ρ : world  => _] => intro x; fix_assert_help; clear x
-    | _ => idtac
+Hint Resolve loc_sub_var2var var_sub_var2var loc_subst_vv_nonfv wf_subst_vv_nonfv subst_vv_fresh : subst.
+
+Instance Subst_list_ty_var_var : Subst (list reft_type) var var := Subst_list. 
+Instance Subst_list_ty_loc_loc : Subst (list reft_type) loc loc := Subst_list. 
+Instance Subst_list_env_var_var : Subst type_env var var := Subst_list. 
+Instance Subst_list_env_loc_loc : Subst type_env loc loc := Subst_list. 
+
+Definition unique_sub' P (s : subst_t var var) (x : var) :=
+  forall v, P v -> x <> v -> nonfv (subst s v) (subst s x).
+
+Goal forall s x, unique_sub' (fun _ => True) s x -> unique_sub s x.
+Proof.
+  firstorder.
+Qed.
+
+Ltac instantiate_ex :=
+  repeat match goal with
+    | H : exists _,_ |- _ => destruct H
   end.
-                
+
+Ltac decompose_all :=
+  repeat match goal with
+           | H : _ /\ _ |- _ => destruct H
+         end;
+  repeat match goal with
+           | H : _ \/ _ |- _ => destruct H
+         end.
+Lemma bind_in_empty_false :
+  forall (x : var) h,
+    bind_in x h -> ~ Empty h.
+Proof.
+  intros.
+  intro.
+  assert (elements h = []). apply HE_Props.elements_Empty. easy.
+  unfold bind_in in *.
+  instantiate_ex.
+  rewrite <- HE_Props.F.find_mapsto_iff in *.
+  rewrite HE_Props.F.elements_mapsto_iff in *.
+  unfold type_binding in *.
+  rewrite  H1 in *.
+  inversion H.
+Qed.
+
+Lemma wf_unique_binds :
+  forall (x : var) l l' t t' g h h',
+    l <> l' ->
+    wf_heap g h h' ->
+    MapsTo l (x,t) h' ->
+    MapsTo l' (x,t') h' ->
+    False.
+Proof.
+  intros until h'. intros neq H.
+  induction H; intro.
+  {
+    rewrite HE_Props.F.elements_mapsto_iff in *.
+    assert (elements Σ' = []).
+    apply HE_Props.elements_Empty. easy. unfold type_binding in *. rewrite H1 in H0. 
+    inversion H0.
+  }
+  {
+    assert (bind_not_in x0 Σ0).
+    apply fresh_var_nonmem_heap with (G := Γ). easy.
+    unfold HE_Props.Add in *.
+    rewrite HE_Props.F.find_mapsto_iff in *.
+    rewrite (H4 l) in *.
+    rewrite <- HE_Props.F.find_mapsto_iff in *.
+    rewrite HE_Props.F.add_mapsto_iff in H5.
+    destruct H5.
+    destruct H5. inv H7.
+    intro.
+    rewrite HE_Props.F.find_mapsto_iff in H5.
+    rewrite (H4 l') in H5.
+    rewrite <- HE_Props.F.find_mapsto_iff in H5.
+    rewrite HE_Props.F.add_mapsto_iff in H5.
+    destruct H5.
+    destruct H5. inv H7. 
+    congruence.
+    destruct H5.
+    unfold bind_not_in in *.
+    rewrite HE_Props.F.find_mapsto_iff in *.
+    specialize (H6 l' t').
+    rewrite <- H7 in *.
+    contradiction H6.
+    reflexivity.
+    destruct H5.
+    intro.
+    rewrite HE_Props.F.find_mapsto_iff in *.
+    rewrite (H4 l') in *.
+    rewrite <- HE_Props.F.find_mapsto_iff in *.
+    rewrite HE_Props.F.add_mapsto_iff in *.
+    destruct H8. destruct H8. inv H9. (* inv H8. *)
+    unfold bind_not_in in *.
+    rewrite HE_Props.F.find_mapsto_iff in *.
+    specialize (H6 l t0).
+    rewrite <- H7 in *. contradiction H6. reflexivity.
+    intuition.
+  }
+Qed.
+
+Lemma unique_binds_neq :
+  forall (x x': var) l t t' (h : heap_env),
+    MapsTo l (x, t) h ->
+    MapsTo l (x', t') h ->
+    x = x'.
+Proof.
+  intros. 
+  rewrite HE_Props.F.find_mapsto_iff in *.
+  rewrite H in H0.
+  inversion H0.
+  reflexivity.
+Qed.
+
+Ltac apply_in_env f :=
+  match goal with 
+    | H : _ |- _ => apply f in H
+  end.
+
+Lemma modvars_unique_sub :
+  forall (x : var) (s : subst_t var var) S,
+    NonUnifyingSub s (s_heap_out S) ->
+    NonUnifyingSub s (s_heap_in S) ->
+    List.In x (mod_vars S) ->
+    unique_sub s x.
+Proof.
+  intros.
+  exists (subst s x).
+  split. reflexivity.
+  intro x'. intro neq. unfold nonfv. simpl. intro.
+  destruct S as [xs ts hi ho xt]. simpl in *.
+  apply_in_env new_mod_vars_schema.
+  unfold NonUnifyingSub in *.
+  decompose_all.
+  unfold bind_in in *.
+  instantiate_ex.
+  rewrite <- HE_Props.F.find_mapsto_iff in *.
+  assert (MapsTo x0 (x', x1) ho).
+  rewrite H5. simpl subst at 2. rewrite H2. rewrite <- H5. assumption.
+  contradiction neq.
+  eapply unique_binds_neq; eauto.
+Qed.
+
+Lemma modlocs_unique_sub :
+  forall (l : loc) (s : subst_t loc loc) (s' : subst_t var var) S,
+    NonUnifyingSub s (subst s' (s_heap_out S)) ->
+    List.In l (mod_locs S) ->
+    unique_lsub s l.
+Proof.
+  intros.
+  repeat intro.
+  unfold NonUnifyingSub in *.
+  decompose_all.
+  apply H in H1.
+  congruence.
+Qed.
+
+Lemma locs_var_sub :
+  forall (s : subst_t var var) (L : list loc),
+    subst s L = L.
+Proof. 
+  induction L. reflexivity.
+  rewrite subst_cons.
+  rewrite IHL.
+  f_equal.
+Qed.
+
+(* Lemma wf_heap_bind_not_in_env : *)
+(*   forall x G H, *)
+(*     wf_heap G H H -> *)
+(*     bind_in x H ->  *)
+(*     ~ var_in x G. *)
+(* Proof. *)
+(*   intros. *)
+(*   intro. *)
+(*   induction H0. *)
+(*   + eapply bind_in_empty_false; eauto. *)
+(*   + unfold bind_in in *. *)
+(*     instantiate_ex. rewrite <- HE_Props.F.find_mapsto_iff in *. *)
+(*     rewrite HE_Props.F.add_mapsto_iff in *. *)
+(*     decompose_all; decompose_all. *)
+(*     inv H7. *)
+(*     apply_in_env fresh_var_not_in. intuition. *)
+(*     apply IHwf_heap. exists x1. exists x2. rewrite <- HE_Props.F.find_mapsto_iff. *)
+(*     easy. easy. *)
+(* Qed. *)
+
+Lemma fresh_loc_not_mem' :
+  forall G H (l : loc),
+    fresh_loc l G H -> forall xt, ~ MapsTo l xt H.
+Proof.
+  intros.
+  intro.
+  unfold fresh_loc in H0.
+  destruct H0.
+  simpl nonfv in *.
+  unfold nonfv_heap in *.
+  apply H2 in H1. intuition.
+Qed.
+
+
+Lemma fresh_loc_not_mem :
+  forall G H (l : loc),
+    fresh_loc l G H -> ~ In l H.
+Proof.
+  intros.
+  intro.
+  rewrite HE_Props.F.in_find_iff in *.
+  assert (exists xt, find l H = Some xt).
+  destruct (find l H). exists t0. reflexivity.
+  congruence.
+  instantiate_ex.
+  eapply fresh_loc_not_mem' in H0.
+  rewrite HE_Props.F.find_mapsto_iff in *.
+  apply H0.
+  apply H2.
+Qed.
+
+(* Lemma remove_add_inv : *)
+(*   forall (h : heap_env) l e, *)
+(*     ~ In l h ->  *)
+(*     Equal (remove l (add l e h)) h. *)
+(* Proof. *)
+(*   setoid_rewrite HE_Props.F.Equal_mapsto_iff. *)
+(*   intros. *)
+(*   symmetry. *)
+(*   rewrite HE_Props.F.find_mapsto_iff in *. *)
+(*   rewrite HE_Props.F.find_mapsto_iff in *. *)
+(*   compare l k. *)
+(*   intros.  *)
+(*   split. intro. rewrite HE_Props.F.not_find_in_iff in *. congruence. *)
+(*   intro.  *)
+(*   rewrite HE_Props.F.remove_eq_o in H0. congruence. assumption. *)
+(*   intros. *)
+(*   rewrite HE_Props.F.remove_neq_o. *)
+(*   rewrite HE_Props.F.add_neq_o. reflexivity. *)
+(*   assumption. *)
+(*   assumption. *)
+(*   apply eq_dec. *)
+(* Qed. *)
+
+Ltac solve_by_rewrite :=
+  match goal with 
+      | H : _ |- _ => (rewrite H; easy) || (rewrite <- H; easy)
+  end.
+
+Ltac solve_by_inversion :=
+  (** thanks jrw **)
+  match goal with 
+    | H : _ |- _ => solve [inversion H]
+    | H : _ |- _ => solve [inversion H]; easy
+  end.
+
+Instance Proper_add l x t (h : heap_env) :
+  Proper (Equal ==> iff) (HE_Props.Add l (x,t) h).
+Proof. 
+  unfold HE_Props.Add.
+  solve_proper.
+Qed.
+
+Lemma wf_Equal_heaps :
+  forall G H H',
+    wf_heap G H H' -> forall H'', Equal H' H'' -> wf_heap G H H''.
+Proof.
+  intros until H'. intro.
+  inv H0. intros.
+  apply wf_emp.
+  solve_by_rewrite.
+  intros.
+  setoid_rewrite H0 in H6.
+  eapply wf_heap_bind; eauto.
+Qed.
+
+Lemma wf_heap_split : 
+  forall G Ho H,
+    wf_heap G Ho H ->
+         forall H1 H2,
+           heap_split H1 H2 H -> (wf_heap G Ho H1 /\ wf_heap G Ho H2).
+Proof.
+  intros until H. intro. induction H0; intros.
+  + split; constructor; unfold heap_split in *;
+    apply_in_env HE_Props.Partition_Empty;
+    intuition.
+  + 
+    unfold heap_split in *.
+    assert (~ In l Σ0).
+    apply_in_env fresh_loc_not_mem; easy.
+    (* assert (HE_Props.Add l (x, t0) Σ0 (add l (x, t0) Σ0)) by firstorder. *)
+    pose (@HE_Props.Partition_Add type_binding Σ0 Σ0' l (x,t0) H8 H4 H5 H6 H7). 
+    instantiate_ex.
+    decompose_all; decompose_all.
+    split.
+    apply wf_heap_bind with (l := l) (x := x) (t := t0) (Σ0 := x0); eauto with heaps.
+    specialize (IHwf_heap x0 H6).
+    apply IHwf_heap. assumption.
+    apply (IHwf_heap x0 H6). assumption.
+    split.
+
+    apply IHwf_heap in H10. apply H10.
+    
+
+    assert (HE_Props.Partition Σ0 x0 H5). unfold HE_Props.Partition in *.
+    split.
+    apply HE_Props.Disjoint_sym.
+    easy. intros. split; intro. apply H10 in H11. destruct H11. right. easy. left. easy.
+    apply H10. destruct H11. right. easy. left. easy.
+   
+    apply wf_heap_bind with (l := l) (x := x) (t := t0) (Σ0 := x0); eauto with heaps.
+    apply IHwf_heap in H11. apply H11.
+Qed.
+
+Corollary wf_heap_split_1 :
+  forall G Ho H1 H2 H,
+    wf_heap G Ho H -> heap_split H1 H2 H -> wf_heap G Ho H1.
+Proof.
+  intros.
+  apply_in_env (wf_heap_split G Ho); eauto.
+  destruct H3. auto.
+Qed.
+
+Corollary wf_heap_split_2 :
+  forall G Ho H1 H2 H,
+    wf_heap G Ho H -> heap_split H1 H2 H -> wf_heap G Ho H2.
+Proof.
+  intros.
+  apply_in_env heap_split_comm.
+  eauto using wf_heap_split_1.
+Qed.
+
+Hint Resolve wf_heap_split_1 wf_heap_split_2 : heaps.
+
+Lemma nonfv_wf_cons :
+  forall (x : var) t g (h : heap_env),
+    wf_env h ((x,t) :: g) -> nonfv (sep_env g) x.
+Proof.
+  intros.
+  inv H.
+  eapply var_nonmem_free_ctx; eauto.
+Qed.
+
+Lemma subst_list_length : 
+  forall (s : subst_t var var) (l1 : list var) (l2 : list reft_type),
+    length l1 = length l2 -> 
+    length (subst s l1) = length (subst s l2).
+Proof.
+  intros until l1.
+  induction l1; intros; destruct l2; try easy.
+  simpl length.
+  simpl subst in IHl1. erewrite IHl1. reflexivity. 
+  inv H. reflexivity.
+Qed.
 
 Lemma sep_proof_proc_call :
-    forall Φ Γ Γ' Σ Σ' Ξ f xs r,
+    forall Φ Γ Γ' Σ Σ' Ξ f xs mxs mls r,
     wf_env Σ Γ ->
     wf_heap Γ Σ Σ ->
-    wf_guards Γ Σ Ξ ->
-    ((Φ ; Γ ; Σ ; Ξ) ⊢ proc_s f xs r [] [] ::: ( Γ' ; Σ')) ->
+    wf_guards Γ Ξ ->
+    ((Φ ; Γ ; Σ ; Ξ) ⊢ proc_s f xs r mxs mls ::: ( Γ' ; Σ')) ->
     (* ((Φ ; Γ ; Σ ; Ξ) *)
     (*    ⊢ proc_s f (subst θ (s_formals S)) (subst θ (fst (s_ret S))) [] ::: (Γ' ; Σ')) -> *)
     semax (sep_proc_env Φ)
           ((sep_env Γ && sep_guards Ξ) * sep_heap Σ)
-          (proc_s f xs r [] [])
+          (proc_s f xs r mxs mls)
           ((sep_env Γ' && sep_guards Ξ) * sep_heap Σ').
+
 Proof with (try assumption).
   (** Here we goo... **)
   intros.
@@ -1864,27 +2501,125 @@ Proof with (try assumption).
   fix_assert; apply subtype_args.
   (** Q' ==> Q **)
   fix_assert.
-  rewrite <- sepcon_pure_andp with (P := sep_ty (var_e (subst θ x)) (subst θl (subst θ t))).
+  (* rewrite <- sepcon_pure_andp with (P := sep_ty (isub θ θl (var_e x)) (isub θ θl t)). *)
   rewrite sepcon_comm.
   rewrite <- sepcon_assoc.
   apply sepcon_derives.
-  rewrite sepcon_pure_andp; try do_pure.
   rewrite sepcon_pure_andp; try do_pure.
   apply andp_right. apply andp_right. apply andp_right. apply andp_left2. apply derives_refl.
   do 2 apply andp_left1. apply derives_refl.
   do_pure.
   apply andp_left1. apply andp_left2. apply derives_refl.
   apply derives_refl.
-  do_pure.
-  do_pure.
   apply semax_frame with (R := sep_env Γ && sep_guards Ξ).
   unfold isub in *.
-  rewrite <- subst_combine.
-  rewrite <- subst_combine.
-  Admitted.
-  
+  setoid_rewrite <- subst_combine.
+  setoid_rewrite <- subst_combine.
+  assert (sep_heap (subst θl (subst θ hi)) = subst θl (sep_heap (subst θ hi))).
+  apply sep_heap_subst; eauto with subst. 
+  rewrite H2.
+  assert (sep_heap (subst θ hi) = subst θ (sep_heap  hi)).
+  apply sep_heap_subst; eauto with subst. 
+  rewrite H3.
+  assert (sep_heap (subst θl (subst θ ho)) = subst θl (sep_heap (subst θ ho))).
+  apply sep_heap_subst; eauto with subst.
+  rewrite H4.
+  assert (sep_heap (subst θ ho) = subst θ (sep_heap ho)).
+  apply sep_heap_subst; eauto with subst.
+  rewrite H5.
+  destruct t as [r P]. fold { ν : r | P }.
+  setoid_rewrite sep_ty_subst; try eauto with subst.
+  setoid_rewrite sep_ty_subst; try eauto with subst.
+  (* assert (sep_env (subst θl (subst θ (combine xs ts))) = subst ?θl (sep_env (subst θ (combine xs ts)))). *)
+  setoid_rewrite sep_env_subst; try eauto with subst.
+  setoid_rewrite sep_env_subst; try eauto with subst.
+  repeat rewrite <- subst_sepcon.
+  assert ( forall mxs0 mls0, subst θl (subst θ (proc_s f xs x mxs0 mls0)) = proc_s f (subst θl (subst θ xs))
+                                                              (subst θl (subst θ x))
+                                                              (subst θl (subst θ mxs0))
+                                                              (subst θl (subst θ mls0))).
+  reflexivity.
+  simpl subst in H6.
+  rewrite <- H6.
+  apply semax_subst_loc.
+  pose semax_subst.
+  simpl subst in s.
+  apply s.
+  set (S := mkSchema xs ts hi ho (x, { ν : r | P})).
+  set (foo := mkProc xs x (mod_vars S) (mod_locs S) p). 
+  assert (xs = p_args foo). reflexivity.
+  assert (x = p_ret foo). reflexivity.
+  assert (mod_vars S = p_mod foo). reflexivity.
+  assert (mod_locs S = p_modl foo). reflexivity.
+  rewrite H7. rewrite H20. rewrite H21. rewrite H22.
+  apply semax_proc.
+  match goal with
+    | H : _ |- _ => apply sep_schema_in_env in H; unfold sep_schema in H; apply H
+  end.
+  intro mv.
+  intro mvs.
+  inv mvs.
+  eapply modvars_unique_sub; eauto. eauto. eauto.
+  exists (subst θ mv). split. reflexivity. intro x'. intro neq.
+  simpl nonfv. simpl.
+  intro.
+  unfold subst_var_loc in *. 
+  rewrite H17 in H7. congruence.
+  intro ml.
+  intro mls.
+  inv mls.
+  set (S := mkSchema xs ts hi ho (x, { ν : r | P})).
+  apply modlocs_unique_sub with (s' := θ) (S := S); eauto.
+  assert (mod_locs S = subst θ (mod_locs S)).
+  rewrite locs_var_sub. reflexivity.
+  rewrite H7.
+  assumption.
+  inv H13. apply H2.
+  apply subst_list_length.
+  inv H13. apply H2.
+  unfold subset.
+  intros.
+  inv H2.
+  pose (nonfv_andp (D := var)). simpl nonfv in n. apply n.
+  split.
+  eapply var_nonmem_free_ctx; eauto.
+  apply H19.
+  apply H21.
+  eapply var_nonmem_free_grd.
+  apply H19.
+  apply H21.
+  auto.
+  auto.
+  pose (nonfv_andp (D := var)). simpl nonfv in n. apply n. split.
+  eapply nonfv_wf_cons; eauto.
+  inv H24.
+  eapply var_nonmem_free_grd; eauto with var.
+  unfold subset.
+  intros.
+  inv H2.
+  apply fv_var_sep_heap.
+  eapply heap_split_nonfv.
+  apply H15.
+  apply H19. apply H21.
+  apply fv_var_sep_heap.
+  eapply heap_split_nonfv.
+  apply H15.
+  apply H19.
+Qed.
     
-    
+Ltac solve_sub := match goal with
+                      | H : @nonfv _ _ _ _ _ ?v |- appcontext[@subst_one _ _ _ ?v _] =>
+                        simpl nonfv in H;
+                          unfold nonfv_assert in H;
+                          simpl; setoid_rewrite <- H;
+                          eauto using andp_left1, andp_left2, derives_refl
+                    end.
+Ltac nfv_env :=
+  match goal with
+    | |- context[@subst _ _ _ _ (subst_one ?v _) ?P] =>
+      assert (nonfv P v); eauto using var_nonmem_free_ctx, var_nonmem_free_grd
+      ; solve_sub
+  end.
   
 
 Lemma sep_proof_assign :
@@ -1905,7 +2640,7 @@ Proof.
   apply semax_frame.
   apply semax_pre_post with
      (P' := (EX v : value, eval_to e v)
-              && subst_pred (subst_one v e) (sep_env ((v, {ν : τ | (var_e ν) .= e}) :: Γ) && sep_guards Ξ))
+              && subst (subst_one v e) (sep_env ((v, {ν : τ | (var_e ν) .= e}) :: Γ) && sep_guards Ξ))
      (Q' := (sep_env ((v, {ν : τ | (var_e ν) .= e}) :: Γ) && sep_guards Ξ)).
   unfold sep_env at 2; fold sep_env.
   normalize.
@@ -1915,17 +2650,19 @@ Proof.
   eapply derives_trans.
   eapply expr_eval_ty' with (T := { ν : τ | φ}); eauto.
   eapply sep_base_eval.
-  repeat rewrite subst_dist_andp.
+  repeat rewrite subst_andp.
   repeat apply andp_right.
   apply derives_trans with (Q := sep_base e τ).
   apply andp_left1.
   eapply expr_eval_ty' with (T := { ν : τ | φ }); eauto.
   apply subst_assign_eq_true.
+  apply H10.
   eapply vv_not_fv; eauto.
   intro; eapply fresh_var_expr_fv; eauto.
   eapply expr_type_wf; eauto.
+  apply andp_left1.
   nfv_env.
-  rewrite subst_emp_id; apply andp_left1; apply sep_env_pure.
+  apply andp_left1. apply sep_env_pure.
   nfv_env.
   normalize.
   rewrite exp_andp1; apply semax_assign.
