Types.v
@@ -36,41 +36,21 @@ Inductive reft_prop : Set :=
   | and_r : reft_prop -> reft_prop -> reft_prop
   | or_r  : reft_prop -> reft_prop -> reft_prop.
 
-Fixpoint fv_prop φ :=
+Fixpoint nonfv_prop {D R : Type} {S: Subst expr D R} φ (x : D) :=
   match φ with 
-    | tt_r => []
-    | eq_r e1 e2 => fv_expr e1 ++ fv_expr e2
-    | not_r φ => fv_prop φ
-    | and_r φ1 φ2 => fv_prop φ1 ++ fv_prop φ2
-    | or_r φ1 φ2 => fv_prop φ1 ++ fv_prop φ2
-  end.
-
-Fixpoint fl_prop φ :=
-  match φ with
-    | tt_r => []
-    | eq_r e1 e2 => fl_expr e1 ++ fl_expr e2
-    | not_r φ => fl_prop φ
-    | and_r φ1 φ2 => fl_prop φ1 ++ fl_prop φ2
-    | or_r φ1 φ2 => fl_prop φ1 ++ fl_prop φ2
+    | tt_r => True
+    | eq_r e1 e2 => nonfv e1 x /\ nonfv e2 x
+    | not_r φ => nonfv_prop φ x
+    | and_r φ1 φ2 => nonfv_prop φ1 x /\ nonfv_prop φ2 x
+    | or_r φ1 φ2 => nonfv_prop φ1 x /\ nonfv_prop φ2 x
   end.
 
 Record reft_type : Set := 
   mkReft_type { reft_base: base_type;
                 reft_r: reft_prop } .
 
-Fixpoint subst_prop_var (s : subst_t var var) prop :=
-  match prop with
-    | tt_r        => tt_r
-    | eq_r e1 e2  => eq_r (subst s e1) (subst s e2)
-    | not_r p     => not_r (subst_prop_var s p)
-    | and_r p1 p2 => and_r (subst_prop_var s p1) (subst_prop_var s p2)
-    | or_r p1 p2  => or_r (subst_prop_var s p1) (subst_prop_var s p2)
-  end.
-
-Definition subst_prop_loc (s : subst_t loc loc) (p : reft_prop) := p.
-                                                       
-Fixpoint subst_prop (s : subst_t var expr) prop :=
-  match prop with
+Fixpoint subst_prop {D R : Type} {S: Subst expr D R} (s : subst_t D R) p :=
+  match p with
     | tt_r        => tt_r
     | eq_r e1 e2  => eq_r (subst s e1) (subst s e2)
     | not_r p     => not_r (subst_prop s p)
@@ -78,39 +58,188 @@ Fixpoint subst_prop (s : subst_t var expr) prop :=
     | or_r p1 p2  => or_r (subst_prop s p1) (subst_prop s p2)
   end.
 
-Instance Subst_prop_loc : Subst reft_prop loc loc := subst_prop_loc.
-Instance Subst_prop_var : Subst reft_prop var var := subst_prop_var.
-Instance Subst_prop : Subst reft_prop var expr := subst_prop.
+Fixpoint eq_prop {D R : Type} {S: Subst expr D R} p1 p2 :=
+  match (p1, p2) with
+    | (tt_r, tt_r) => True
+    | (eq_r e11 e12, eq_r e21 e22) => eq e11 e21 /\ eq e12 e22
+    | (not_r p1, not_r p2) => eq_prop p1 p2
+    | (and_r p11 p12, and_r p21 p22) => eq_prop p11 p21 /\ eq_prop p12 p22
+    | (or_r p11 p12, or_r p21 p22) => eq_prop p11 p21 /\ eq_prop p12 p22
+    | _ => False
+  end.
 
-Definition subst_r_var (s : subst_t var var) reft :=
-  mkReft_type (reft_base reft) (subst s (reft_r reft)).
+Instance Eq_eqProp {D R : Type} {S: Subst expr D R} {E: Equivalence (eq (A := expr) (D := D) (R := R))}
+: Equivalence eq_prop.
+Proof.
+  constructor; intro.
+  induction x; repeat constructor; try reflexivity; try assumption.
+  induction x; destruct y; intros; try inversion H; solve_instance.
+  induction x; destruct y; destruct z; solve_instance.
+Qed.
 
-Definition subst_base_loc (s : subst_t loc loc) b :=
+(* Definition subst_prop_loc (s : subst_t loc loc) (p : reft_prop) := p. *)
+                                                       
+(* Fixpoint subst_prop (s : subst_t var expr) prop := *)
+(*   match prop with *)
+(*     | tt_r        => tt_r *)
+(*     | eq_r e1 e2  => eq_r (subst s e1) (subst s e2) *)
+(*     | not_r p     => not_r (subst_prop s p) *)
+(*     | and_r p1 p2 => and_r (subst_prop s p1) (subst_prop s p2) *)
+(*     | or_r p1 p2  => or_r (subst_prop s p1) (subst_prop s p2) *)
+(*   end. *)
+
+
+(* Instance Subst_prop_loc : Subst reft_prop loc loc := subst_prop_loc. *)
+(* Instance Subst_prop_var : Subst reft_prop var var := subst_prop_var. *)
+Instance Subst_prop {D R : Type} {S: Subst expr D R} : Subst reft_prop D R := 
+  mkSubst _ _ _ (eq_prop (S := S)) nonfv_prop subst_prop.
+
+Instance FVSubst_prop
+         {D R : Type} 
+         `{S: SubstFV expr D R} 
+         {E : Equivalence (eq (A := expr) (D := D) (R := R))}
+         {P : Proper (Logic.eq ==> (eq (A := expr) (D := D) (R := R))
+                               ==> (eq (A := expr) (D := D) (R := R))) subst}
+         : SubstFV reft_prop D R _.
+Proof.
+  constructor.
+  intros; induction e; solve_instance. 
+Defined.
+
+(* Definition subst_r_var (s : subst_t var var) reft := *)
+(*   mkReft_type (reft_base reft) (subst s (reft_r reft)). *)
+
+(* Definition subst_base_loc (s : subst_t loc loc) b := *)
+(*   match b with *)
+(*     | ref_t l => ref_t (s l) *)
+(*     | _ => b *)
+(*   end. *)
+
+Definition subst_base {D R : Type} {S : Subst loc D R} s b :=
   match b with
-    | ref_t l => ref_t (s l)
+    | ref_t l => ref_t (subst s l)
     | _ => b
   end.
 
-Instance Subst_base_loc : Subst base_type loc loc := subst_base_loc.
+Definition nonfv_base {D R : Type} {S : Subst loc D R} b (x : D) :=
+  match b with
+    | ref_t l => nonfv l x
+    | _ => True
+  end.
 
-Definition subst_r_loc (s : subst_t loc loc) reft :=
-  mkReft_type (subst s (reft_base reft)) (reft_r reft).
+Definition eq_base {D R : Type} {S : Subst loc D R} {E : Equivalence (eq (A := loc))} (b1 b2 : base_type) := 
+  match (b1, b2) with
+    | (ref_t l, ref_t l') => (eq (D := D)) l l'
+    | _ => Logic.eq b1 b2
+  end.
 
-Definition subst_r s reft :=
-  mkReft_type (reft_base reft) (subst s (reft_r reft)).
+Instance Subst_base 
+         {D R : Type} 
+         `{S : Subst loc D R} 
+         {E : Equivalence (eq (A := loc))} : Subst base_type D R := 
+  mkSubst _ _ _ (@eq_base D R S E) nonfv_base subst_base.
 
-Instance Subst_reft_var : Subst reft_type var var := subst_r_var.
-Instance Subst_reft : Subst reft_type var expr := subst_r.
-Instance subst_reft_loc : Subst reft_type loc loc := subst_r_loc.
+Instance FVSubst_base 
+         {D R : Type} 
+         `{S : SubstFV loc D R} 
+         {E : Equivalence (eq (A := loc))} : SubstFV base_type D R _ := _.
+Proof. 
+  constructor; intros; destruct e; solve_instance.
+Defined.
+
+Instance Eq_eqBase 
+         {D R : Type}
+         {S : Subst loc D R}
+         {E : Equivalence (@eq loc D R S) } : Equivalence (@eq base_type D R Subst_base).
+Proof.
+  constructor. 
+  hnf; intros; destruct x; try reflexivity. unfold eq. simpl. unfold eq_base. reflexivity.
+
+  hnf; intros; destruct x; destruct y; try inversion H; try reflexivity.
+  unfold eq in *; simpl in *; unfold eq_base in *. symmetry. assumption.
+
+  hnf; intros; destruct x; destruct y; try inversion H; destruct z; try inversion H0.
+  assumption. assumption. unfold eq in *; simpl in *; unfold eq_base in *. eapply transitivity; eauto.
+Defined.
+
+Instance Subst_base_proper 
+    {D R : Type} 
+    {S : Subst loc D R}
+    {P : Proper (Logic.eq ==> (@eq _ _ _ S) ==> (@eq _ _ _ S)) subst}
+    {E : Equivalence (eq (A := loc))} :
+       Proper (Logic.eq ==> (@eq_base D R S E) ==> (@eq_base D R S E)) subst.
+Proof.
+  repeat (hnf; intros).
+  subst.
+  unfold eq_base in H0.
+  destruct x0; destruct y0; simpl; try reflexivity; try inversion H0.
+  rewrite H0. reflexivity.
+Qed.
+
+(* Definition subst_r_loc (s : subst_t loc loc) reft := *)
+(*   mkReft_type (subst s (reft_base reft)) (reft_r reft). *)
+
+Definition subst_r {D R : Type} {S : Subst base_type D R} {S' : Subst reft_prop D R} s reft :=
+  mkReft_type (subst s (reft_base reft)) (subst s (reft_r reft)).
+
+Definition nonfv_reft_t {D R : Type} {S : Subst base_type D R} {S' : Subst reft_prop D R} 
+           reft (x : D) := nonfv (reft_base reft) x /\ nonfv (reft_r reft) x.
+
+Definition eq_reft_r {D R : Type} {S : Subst base_type D R} {S' : Subst reft_prop D R}
+           r1 r2 := eq (reft_base r1) (reft_base r2) /\ eq (reft_r r1) (reft_r r2).
+
+(* Instance Subst_reft_var : Subst reft_type var var := subst_r_var. *)
+Instance Subst_reft {D R : Type} {S : Subst base_type D R} {S' : Subst reft_prop D R} : Subst reft_type D R
+:= (mkSubst _ _ _ eq_reft_r nonfv_reft_t subst_r).
+
+Instance Eq_eq_reft_r { D R : Type } 
+         {S : Subst base_type D R}
+         {S' : Subst reft_prop D R}
+         {E: Equivalence (@eq _ _ _ S)}
+         {E': Equivalence (@eq _ _ _ S')} : Equivalence (@eq _ _ _ Subst_reft).
+Proof.
+  constructor.
+  constructor; reflexivity.
+  constructor; symmetry; apply H. 
+  constructor; eapply transitivity. apply H. apply H0. apply H. apply H0.
+Qed.
+
+Instance Eq_eq_reft_r_list : Equivalence (@eq (list reft_type) var var Subst_list) := Eq_eqList.
+
+Instance Subst_reft_var : Subst reft_type var var := Subst_reft.
+Instance Subst_reft_expr : Subst reft_type var expr := Subst_reft.
+Instance Subst_reft_loc : Subst reft_type loc loc := Subst_reft.
+
+Instance FVSubst_reft
+{D R : Type} `{S : SubstFV base_type D R} `{S' : SubstFV reft_prop D R} : SubstFV reft_type D R _.
+Proof.
+  constructor; intros; solve_instance.
+Defined.
+
+Instance Eq_eqReft {D R : Type} {S : Subst base_type D R} {S' : Subst reft_prop D R}
+         {Eb : Equivalence (@eq base_type D R S)}
+         {Er : Equivalence (@eq reft_prop D R S')}
+         : Equivalence (@eq _ _ _ (@Subst_reft D R S S')).
+Proof.
+  unfold eq. simpl.
+  constructor; constructor. 
+  reflexivity. reflexivity.
+  inversion H; symmetry; assumption.
+  inversion H; symmetry; assumption. 
+  inversion H. inversion H0. eapply transitivity; eauto.
+  inversion H. inversion H0. eapply transitivity; eauto.
+Qed.
+
+(* Instance subst_reft_loc : Subst reft_type loc loc := subst_r_loc. *)
 
 Definition type_binding : Set := (var * reft_type)%type.
+Hint Transparent type_binding.
 
 Definition dummyt (v : var) t p := mkReft_type t p.
 
 Notation "x .= y" := (eq_r x y) (at level 70).
 (* Notation "{ vv : t | P }" := (mkReft_type t P%reft) (at level 0, no associativity). *)
 Notation "{ vv : t | P }" := (dummyt vv t P%reft) (at level 0, vv at level 99, no associativity).
-
 
 (** Environments **)
 (* Module Type Loc. *)
@@ -120,7 +249,7 @@ Notation "{ vv : t | P }" := (dummyt vv t P%reft) (at level 0, vv at level 99, n
 
 Module Loc_as_OT <: UsualOrderedType.
   Definition t := loc.
-  Definition eq := @eq loc.
+  Definition eq := @Logic.eq loc.
   Definition eq_refl := @eq_refl loc.
   Definition eq_sym := @eq_sym loc.
   Definition eq_trans := @eq_trans loc.
@@ -139,7 +268,7 @@ Module Loc_as_OT <: UsualOrderedType.
     apply l. apply H. apply H0.
   Qed.
 
-  Lemma lt_not_eq : forall l1 l2, lt l1 l2 -> ~ eq l1 l2.
+  Lemma lt_not_eq : forall (l1 l2 : loc), lt l1 l2 -> ~ @Logic.eq loc l1 l2.
   Proof.
     destruct l1 as [n1].
     destruct l2 as [n2].
@@ -176,29 +305,133 @@ Definition type_env : Type := bind_env var reft_type.
 Definition heap_env : Type := HE.t type_binding.
 Definition heap_emp := HE.empty type_binding.
 
-Definition subst_heap_var s (h : heap_env) : heap_env :=
-  HE.map (fun xt => subst s xt) h.
+Hint Transparent type_env bind_env.
 
-Instance Subst_heap_var : Subst heap_env var var := subst_heap_var.
-Instance Subst_binding_loc : Subst type_binding loc loc :=
-  fun s xt => (fst xt, subst s (snd xt)).
+Instance Subst_heap_bind {D R : Type} {S : Subst loc D R} {S' : Subst type_binding D R}
+: Subst (loc * type_binding) D R  := _.
 
-Definition subst_heap_loc (s : loc -> loc) (h : heap_env) : heap_env :=
-  HE_Props.of_list (subst s (HE_Props.to_list h)).
+(* Instance Subst_heap_bind_list {D R : Type} {S : Subst loc D R} {S' : Subst type_binding D R} *)
+(*          {E : Equivalence (@eq _ _ _ S)} {E' : Equivalence (@eq _ _ _ S')} *)
+(* : Subst (list (loc * type_binding)) D R := Subst_list. *)
 
-Definition subst_var_loc (s : loc -> loc) (x : var) : var := x.
+Definition subst_heap 
+           {D R : Type} {S : Subst loc D R} {S' : Subst type_binding D R}
+           {E : Equivalence (@eq _ _ _ S)} {E' : Equivalence (@eq _ _ _ S')}
+         s (h : heap_env) :=
+  HE.fold (fun l xt m => HE.add (subst s l) (subst s xt) m) h (heap_emp).
+  (* HE_Props.of_list (@subst (list (loc * type_binding)) D R Subst_list s (HE_Props.to_list h)). *)
 
-Fixpoint subst_expr_loc (s : loc -> loc) (x : expr) : expr := 
-  match x with
-    | locvar_e l => locvar_e (s l)
-    | fun_e p e1 e2 => fun_e p (subst_expr_loc s e1) (subst_expr_loc s e2)
-    | _ => x
-  end.
+Definition nonfv_heap {D R : Type} {S : Subst loc D R} {S : Subst type_binding D R}
+         (h : heap_env) (v : D) :=
+  forall l xt, HE.MapsTo l xt h -> (nonfv l v /\ nonfv xt v).
 
-Instance Subst_loc_var : Subst var loc loc := subst_var_loc.
-Instance Subst_loc_expr : Subst expr loc loc := subst_expr_loc.
+Import HE.
+Import HE_Facts.
+Import HE_Props.
 
-Instance Subst_heap_loc : Subst heap_env loc loc := subst_heap_loc.
+(* Lemma fv_heap_list : *)
+(*   forall (D R : Type) (S : Subst loc D R) (S' : Subst type_binding D R)  *)
+(*          {E : Equivalence (@eq _ _ _ S)} {E' : Equivalence (@eq _ _ _ S')} *)
+(*          (h : heap_env),  *)
+(*     (forall x:D, fv_heap h x <-> (@nonfv (list (loc * type_binding)) D R Subst_list (HE.elements h) x)). *)
+(* Proof. *)
+(*   constructor. { *)
+(*     intros. *)
+(*     unfold fv_heap in H. *)
+(*     destruct H as [l [[y t] [A B]]]. *)
+(*     destruct B. *)
+(*     simpl. *)
+(*     rewrite HE_Props.F.elements_mapsto_iff in A. *)
+(*     induction (HE.elements h) as [|[l' [y' t']]]. *)
+(*     inversion A. *)
+(*     simpl. inversion A. subst. inversion H1. inversion H2. simpl in *. subst. *)
+(*     left. left. assumption. *)
+(*     destruct y0. destruct t0. inversion H0. subst. *)
+(*     right. apply IHl0. assumption. *)
+ 
+(*     rewrite HE_Props.F.elements_mapsto_iff in A. *)
+(*     induction (HE.elements h) as [|[l' [y' t']]]. *)
+(*     inversion A. *)
+(*     simpl in *. inversion A. destruct y0. destruct t0. inversion H1. simpl in *. *)
+(*     inversion H0. subst. inversion H4. subst. left. right. assumption. *)
+(*     right. apply IHl0. assumption. *)
+(*   }  *)
+(*   { *)
+(*     intros. *)
+(*     (* pose (elements_3w h).  *) *)
+(*     (* pose (@elements_mapsto_iff _ h). *) *)
+(*     unfold fv_heap. *)
+(*     setoid_rewrite elements_mapsto_iff. *)
+(*     (* generalize i. *) *)
+(*     (* clear i. *) *)
+(*     induction (elements h). *)
+(*     intros. inversion H. *)
+(*     intros. *)
+(*     destruct a. *)
+(*     destruct H. *)
+(*     exists k. exists t0. constructor. left. reflexivity. destruct H. left. assumption. right. assumption. *)
+(*     apply IHl in H. destruct H. destruct H. *)
+(*     destruct H. *)
+(*     exists x0. exists x1. constructor. right. assumption. assumption. *)
+(*   } *)
+(* Qed. *)
+
+Lemma subst_list_step :
+  forall (A D R : Type) (S : Subst A D R) (E : Equivalence (@eq _ _ _ S))
+    (a : A) (l : list A) s,
+    eq (subst s (a :: l)) (subst s a :: subst s l).
+Proof.
+  intros.
+  simpl.
+  constructor; reflexivity.
+Qed.
+
+Hint Transparent key.
+Typeclasses Transparent key type_binding eq_base.
+
+Instance Subst_heap 
+           {D R : Type} 
+           {S : Subst key D R }
+           {S' : Subst type_binding D R }
+           {E : Equivalence (@eq _ _ _ S)}
+           {E' : Equivalence (@eq _ _ _ S')}
+           (* {P: Proper (@eq _ _ _ S ==> @eq _ _ _ S' ==> Equal ==> Equal) (add (elt := type_binding)) } *)
+  : Subst heap_env D R := mkSubst _ _ _ HE.Equal nonfv_heap subst_heap.
+
+Instance Subst_heap_var : Subst heap_env var var := Subst_heap.
+Instance Subst_heap_loc : Subst heap_env loc loc := Subst_heap.
+
+Instance FVSubst_heap 
+           {D R : Type} 
+          `{S : SubstFV key D R }
+          `{S': SubstFV type_binding D R }
+           {E : Equivalence (@eq key D R _)}
+           {E': Equivalence (@eq type_binding D R _)}
+           {P: Proper (@eq key _ _ _ ==> (@eq type_binding _ _ _) ==> Equal ==> Equal) (add (elt := type_binding)) }
+  : SubstFV heap_env D R _.
+Proof.
+  constructor.
+  intros.
+  unfold subst, Subst_heap, subst_heap.
+  assert (Equal (fold (fun l xt m => add (subst s l) (subst s xt) m) e heap_emp)
+                (fold (fun l xt m => add l xt m) e heap_emp)).
+  apply (fold_rel (R := Equal) 
+                  (f := fun l xt m => add (subst s l) (subst s xt) m)
+                  (g := fun l xt m => add l xt m)).
+  reflexivity.
+  intros.
+  unfold nonfv, Subst_heap, nonfv_heap in H. 
+  rewrite subst_nonfv.
+  rewrite subst_nonfv.
+  apply add_m; easy.
+  solve_instance.
+  solve_instance.
+  rewrite H0.
+  apply fold_identity.
+Defined.
+
+(* Instance Subst_binding_loc : Subst type_binding loc loc := *)
+(*   fun s xt => (fst xt, subst s (snd xt)). *)
 
 (** Procedures **)
 Record proc_schema : Type :=
@@ -208,28 +441,79 @@ Record proc_schema : Type :=
              s_heap_out: heap_env;
              s_ret: type_binding }.
 
-Definition subst_schema (s : var -> var) S :=
-  let subst_both s xt := (@subst _ _ _ Subst_var_var s (fst xt),
-                          @subst _ _ _ Subst_reft_var s (snd xt)) in
+Definition subst_schema 
+           {D R : Type} {Sv : Subst var D R } {St : Subst reft_type D R} {Sl : Subst key D R}
+           {E : Equivalence (@eq _ _ _ Sv)}
+           {E' : Equivalence (@eq _ _ _ St)}
+           {E'' : Equivalence (@eq _ _ _ Sl)}
+           {E''' : Equivalence (@eq type_binding _ _ _)}
+           (* {P : Proper ((@eq _ _ _ Sl) ==> (@eq type_binding _ _ _) ==> Equal ==> Equal) *)
+           (*             (add (elt := type_binding))} *)
+           (s : subst_t D R) S :=
   match S with
     | mkSchema xs ts hi ho xt =>
-      mkSchema (subst s xs) (subst s ts) (subst_heap_var s hi) (subst_heap_var s ho) (subst_both s xt)
+      mkSchema (subst s xs) (subst s ts) (subst s hi) (subst s ho) (subst s xt)
   end.
 
-Definition subst_schema_loc (s : loc -> loc) S :=
- match S with
-   | mkSchema xs ts hi ho (x, t) =>
-     mkSchema xs (subst s ts) (subst_heap_loc s hi)
-              (subst_heap_loc s ho) (x, subst s t)
- end.              
+Definition nonfv_schema
+           {D R : Type} {Sv : Subst var D R } {St : Subst reft_type D R} {Sl : Subst key D R}
+           {E : Equivalence (@eq _ _ _ Sv)}
+           {E' : Equivalence (@eq _ _ _ St)}
+           {E'' : Equivalence (@eq _ _ _ Sl)}
+           {E''' : Equivalence (@eq type_binding _ _ _)}
+           (* {P : Proper ((@eq _ _ _ Sl) ==> (@eq type_binding _ _ _) ==> Equal ==> Equal) *)
+           (*             (add (elt := type_binding))} *)
+           s x :=
+  match s with
+    | mkSchema xs ts hi ho xt =>
+     nonfv xs x /\ nonfv ts x /\ nonfv hi x /\ nonfv ho x /\ nonfv xt x
+  end.
 
-Instance Subst_proc_schema : Subst proc_schema var var := subst_schema.
-Instance Subst_proc_schema_loc : Subst proc_schema loc loc := subst_schema_loc.
+Definition eq_schema
+           {D R : Type} {Sv : Subst var D R } {St : Subst reft_type D R} {Sl : Subst key D R}
+           {E : Equivalence (@eq _ _ _ Sv)}
+           {E' : Equivalence (@eq _ _ _ St)}
+           {E'' : Equivalence (@eq _ _ _ Sl)}
+           {E''' : Equivalence (@eq type_binding _ _ _)}
+           (* {P : Proper ((@eq _ _ _ Sl) ==> (@eq type_binding _ _ _) ==> Equal ==> Equal) *)
+           (*             (add (elt := type_binding))} *)
+           (s1 s2 : proc_schema) :=
+  let (xs, ts, hi, ho, xt) := s1 in
+  let (xs', ts', hi', ho', xt') := s2 in
+  eq xs xs' /\ eq ts ts' /\ eq hi hi' /\ eq ho ho' /\ eq xt xt'.
+
+Instance Subst_schema
+           {D R : Type} {Sv : Subst var D R } {St : Subst reft_type D R} {Sl : Subst key D R}
+           {E : Equivalence (@eq _ _ _ Sv)}
+           {E' : Equivalence (@eq _ _ _ St)}
+           {E'' : Equivalence (@eq _ _ _ Sl)}
+           {E''' : Equivalence (@eq type_binding _ _ _)} :
+            Subst proc_schema D R := mkSubst _ _ _ eq_schema nonfv_schema subst_schema.
+Instance FVSubst_schema
+           {D R : Type} `{Sv : SubstFV var D R } `{St : SubstFV reft_type D R} `{Sl : SubstFV key D R}
+           {E : Equivalence (@eq var D R _)}
+           {E' : Equivalence (@eq reft_type D R _)}
+           {E'' : Equivalence (@eq key D R _)}
+           {E''' : Equivalence (@eq type_binding D R _)} 
+           {P : Proper ((@eq key _ _ _) ==> (@eq type_binding _ _ _) ==> Equal ==> Equal)
+                       (add (elt := type_binding))}
+         : SubstFV proc_schema D R Subst_schema := _.
+Proof.
+  constructor.
+  intros θ [xs ts hi ho xt].
+  intro.
+  unfold eq.
+  unfold subst.
+  unfold Subst_schema. unfold eq_schema. unfold subst_schema.
+  unfold nonfv in H. unfold Subst_schema in H. unfold nonfv_schema in H.
+  repeat rewrite subst_nonfv;
+  first [repeat constructor; reflexivity | apply H].
+Defined.
 
 Definition proc_env : Type := bind_env pname (stmt * proc_schema)%type.
 
 Definition var_in : var -> type_env -> Prop := 
-  fun x Γ => exists t, In (x, t) Γ.
+  fun x Γ => exists t, List.In (x, t) Γ.
 
 Definition var_not_in : var -> type_env -> Prop :=
   fun x Γ => Forall (fun xt => (fst xt <> x)) Γ.
@@ -254,15 +538,15 @@ Definition ty_loc (T : reft_type) :=
   end.
 
 Definition loc_not_in_ctx : loc -> type_env -> Prop :=
-  fun l Γ => Forall (fun xt => ~ In l (ty_loc (snd xt))) Γ.
+  fun l Γ => Forall (fun xt => ~ List.In l (ty_loc (snd xt))) Γ.
 
 Definition fun_in : (pname * (stmt * proc_schema)) -> proc_env -> Prop :=
-  fun ft Φ => In ft Φ.
+  fun ft Φ => List.In ft Φ.
 
 Definition fun_not_in : pname  -> proc_env -> Prop :=
   fun f Φ => Forall (fun ft => fst ft <> f) Φ.
 
-Notation "X ∈ Y" := (In X Y) (at level 40).
+Notation "X ∈ Y" := (List.In X Y) (at level 40).
 
 Definition disjoint (Σ1 Σ2 : heap_env) :=
      forall l, (HE.In l Σ1 -> ~ HE.In l Σ2)
@@ -287,23 +571,58 @@ Definition guards := list reft_prop.
 (** Ugh Equality **)
 Instance EqDec_base_t : EqDec base_type := _.
 Proof.
-  hnf. decide equality; apply eq_dec.
+  hnf. decide equality; apply eq_dec.eq_dec.
 Qed.
 
 Instance EqDec_reft_prop : EqDec reft_prop := _.
 Proof.
-  hnf. decide equality; try apply eq_dec. 
+  hnf. decide equality; try apply eq_dec.eq_dec.
 Qed.
 
 Instance EqDec_reft_type : EqDec reft_type := _.
 Proof.
-  hnf. decide equality; try apply eq_dec.
+  hnf. decide equality; try apply eq_dec.eq_dec.
 Qed.
 
-(* Instance EqDec_proc_schema : EqDec proc_schema := _. *)
-(* Proof. *)
-(*   hnf. decide equality; try apply eq_dec. *)
-(* Qed. *)
+Class SubstReft (D R : Type) `{SubstFV expr D R} `{ SubstFV reft_prop D R} : Type := 
+  mkSubstReft {
+      subst_tt_r : 
+        forall (s : subst_t D R), 
+          subst s tt_r = tt_r
+      ;
+      subst_rel_r : 
+        forall (s : subst_t D R) e1 e2, 
+          subst s (e1 .= e2) = (subst s e1 .= subst s e2)
+      ;
+      subst_not_r :
+        forall (s : subst_t D R) p,
+          subst s (not_r p) = not_r (subst s p)
+      ;
+      subst_and_r :
+        forall (s : subst_t D R) p1 p2, 
+          subst s (and_r p1 p2) = (and_r (subst s p1) (subst s p2))
+      ;
+      subst_or_r :
+        forall (s : subst_t D R) p1 p2, 
+          subst s (or_r p1 p2) = (or_r (subst s p1) (subst s p2))
+    }.
+
+Ltac rw_subst_reft :=
+  repeat first [ setoid_rewrite subst_tt_r
+               | setoid_rewrite subst_rel_r
+               | setoid_rewrite subst_not_r
+               | setoid_rewrite subst_or_r
+               | setoid_rewrite subst_and_r
+               ].
+
+Instance SubstReft_var_var : SubstReft var var. 
+Proof. solve_instance. Qed.
+
+Instance SubstReft_var_expr : SubstReft var expr. 
+Proof. solve_instance. Qed.
+
+Instance SubstReft_loc_loc : SubstReft loc loc. 
+Proof. solve_instance. Qed.
 
 Definition ν := vv.
 
@@ -351,10 +670,6 @@ Proof.
   apply HE_Props.Partition_sym.
   assumption.
 Qed.
-
-Import HE.
-Import HE_Facts.
-Import HE_Props.
 
 Lemma heap_split_loc_not_in :
   forall l Σ1 Σ2 Σ,
